new code for demands analysis

meta-theory/pure_demandScript.sml
@@ -7,39 +7,521 @@ open arithmeticTheory listTheory stringTheory alistTheory dep_rewrite
      optionTheory pairTheory ltreeTheory llistTheory bagTheory
      BasicProvers pred_setTheory relationTheory rich_listTheory finite_mapTheory;
 open pure_expTheory pure_valueTheory pure_evalTheory pure_eval_lemmasTheory
-     pure_exp_lemmasTheory pure_miscTheory pure_exp_relTheory pure_congruenceTheory;
+     pure_exp_lemmasTheory pure_miscTheory pure_exp_relTheory pure_congruenceTheory
+     pure_alpha_equivTheory pure_alpha_equivTheory;
 
 val _ = new_theory "pure_demand";
 
-Definition Projs_def:
-  Projs [] e = e ∧
-  Projs ((x,i)::ps) e = Projs ps (Proj x i e)
+(** begin ctxt **)
+
+(* Definitions *)
+
+Datatype:
+  ctxt = Nil
+       | IsFree string ctxt
+       | Bind string exp ctxt
+       | RecBind ((string # exp) list) ctxt
 End
 
-Theorem demands_proj_end:
-  ∀ ps x i e. Projs (ps++[(x,i)]) e = Proj x i (Projs ps e)
+Definition unfold_ctxt_def:
+  unfold_ctxt Nil e = e ∧
+  unfold_ctxt (IsFree v c) e = Lam v (unfold_ctxt c e) ∧
+  unfold_ctxt (Bind v e c) e2 = Let v e (unfold_ctxt c e2) ∧
+  unfold_ctxt (RecBind bL c) e = Letrec bL (unfold_ctxt c e)
+End
+
+Definition concat_rev_ctxt_def:
+  concat_rev_ctxt Nil c = c ∧
+  concat_rev_ctxt (IsFree v c1) c2 = concat_rev_ctxt c1 (IsFree v c2) ∧
+  concat_rev_ctxt (Bind v e c1) c2 = concat_rev_ctxt c1 (Bind v e c2) ∧
+  concat_rev_ctxt (RecBind bL c1) c2 = concat_rev_ctxt c1 (RecBind bL c2)
+End
+
+Definition concat_ctxt_def:
+  concat_ctxt Nil c = c ∧
+  concat_ctxt (IsFree v c1) c2 = IsFree v (concat_ctxt c1 c2) ∧
+  concat_ctxt (Bind v e c1) c2 = Bind v e (concat_ctxt c1 c2) ∧
+  concat_ctxt (RecBind bL c1) c2 = RecBind bL (concat_ctxt c1 c2)
+End
+
+Definition not_bound_in_ctxt_def:
+  not_bound_in_ctxt Nil v = T ∧
+  not_bound_in_ctxt (IsFree v1 c) v2 = (v1 ≠ v2 ∧ not_bound_in_ctxt c v2) ∧
+  not_bound_in_ctxt (Bind v1 e c) v2 = (v1 ≠ v2 ∧ not_bound_in_ctxt c v2) ∧
+  not_bound_in_ctxt (RecBind bL c) v = (not_bound_in_ctxt c v ∧ ¬MEM v (MAP FST bL))
+End
+
+Definition eq_when_applied_def:
+  (eq_when_applied Nil e1 e2 len = ∀l. len = LENGTH l ⇒ (Apps e1 l) ≈ (Apps e2 l)) ∧
+  eq_when_applied (Bind v e c) e1 e2 len = eq_when_applied c (Let v e e1) (Let v e e2) len ∧
+  eq_when_applied (IsFree v c) e1 e2 len = (∀e. closed e ⇒ eq_when_applied c (Let v e e1) (Let v e e2) len) ∧
+  eq_when_applied (RecBind b c) e1 e2 len = eq_when_applied c (Letrec b e1) (Letrec b e2) len
+End
+
+Definition exp_eq_in_ctxt_def:
+  exp_eq_in_ctxt Nil = (λe1 e2. e1 ≈ e2) ∧
+  exp_eq_in_ctxt (IsFree s c) e1 e2 = (∀e3. closed e3 ⇒ exp_eq_in_ctxt c (Let s e3 e1) (Let s e3 e2)) ∧
+  exp_eq_in_ctxt (Bind s e3 c) e1 e2 = exp_eq_in_ctxt c (Let s e3 e1) (Let s e3 e2) ∧
+  exp_eq_in_ctxt (RecBind l c) e1 e2 = exp_eq_in_ctxt c (Letrec l e1) (Letrec l e2)
+End
+
+Theorem exp_eq_l_refl:
+  ∀b l. LIST_REL (λx y. (x ≅? y) b) l l
 Proof
-  Induct THEN1 rw [Projs_def]
-  \\ gen_tac \\ rename1 ‘hd::ps’
-  \\ PairCases_on ‘hd’
-  \\ rw [Projs_def]
+  gen_tac
+  \\ Induct
+  \\ fs [exp_eq_refl]
 QED
 
-Theorem double_Projs:
-  ∀ps' ps e. Projs (ps' ++ ps) e = Projs ps (Projs ps' e)
+Theorem exp_eq_unfold_cong:
+  ∀c e1 e2 b. (e1 ≅? e2) b ⇒ (unfold_ctxt c e1 ≅? unfold_ctxt c e2) b
 Proof
-  Induct >- rw [Projs_def]
-  \\ gen_tac \\ rename1 ‘hd::ps'’
-  \\ PairCases_on ‘hd’
-  \\ rw [Projs_def]
+  Induct >> rw [unfold_ctxt_def] >> last_x_assum $ dxrule_then assume_tac >>
+  gvs [exp_eq_App_cong, exp_eq_refl, exp_eq_Lam_cong, exp_eq_Letrec_cong, exp_eq_l_refl]
 QED
 
-Theorem Seq_App:
+Theorem eq_when_applied_0:
+  ∀c e1 e2. exp_eq_in_ctxt c e1 e2 = eq_when_applied c e1 e2 0
+Proof
+  Induct >>
+  gvs [exp_eq_in_ctxt_def, eq_when_applied_def, Apps_def]
+QED
+
+Definition ctxt_size_def:
+  ctxt_size Nil = 0n ∧
+  ctxt_size (IsFree s ctxt) = 1 + ctxt_size ctxt ∧
+  ctxt_size (Bind s e ctxt) = 1 + list_size char_size s +  exp_size e + ctxt_size ctxt ∧
+  ctxt_size (RecBind sel ctxt) = 1 + exp1_size sel + ctxt_size ctxt
+End
+
+(* Preliminaries *)
+
+Theorem exp_eq_Apps_cong:
+  ∀l l' b e e'. LIST_REL (λx y. (x ≅? y) b) l l' ⇒ (e ≅? e') b ⇒ (Apps e l ≅? Apps e' l') b
+Proof
+  Induct
+  \\ fs [Apps_def]
+  \\ rw [Apps_def]
+  \\ fs [Apps_def]
+  \\ first_x_assum $ irule
+  \\ fs [exp_eq_App_cong]
+QED
+
+Theorem exp_eq_Lams_cong:
+  ∀l e e' b. (e ≅? e') b ⇒ (Lams l e ≅? Lams l e') b
+Proof
+  Induct
+  \\ rw [Lams_def]
+  \\ fs [exp_eq_Lam_cong]
+QED
+
+Theorem eval_Prim:
+  ∀ope eL eL'. LIST_REL (λe1 e2. eval e1 = eval e2) eL eL' ⇒ eval (Prim ope eL) = eval (Prim ope eL')
+Proof
+  Cases
+  \\ rw [eval_thm]
+  >~[‘MAP _ _ = MAP _ _’]
+  >- (irule LIST_EQ
+      \\ gvs [LIST_REL_EL_EQN, EL_MAP])
+  >~[‘AtomOp’]
+  >- (fs [eval_def]
+      \\ once_rewrite_tac [v_unfold]
+      \\ fs [eval_wh_Prim]
+      \\ qsuff_tac ‘get_atoms (MAP eval_wh eL') = get_atoms (MAP eval_wh eL)’
+      >- (CASE_TAC \\ fs [])
+      \\ fs [get_atoms_def]
+      \\ qsuff_tac ‘EXISTS error_Atom (MAP eval_wh eL) ⇔ EXISTS error_Atom (MAP eval_wh eL')’
+      >- (strip_tac
+          \\ IF_CASES_TAC
+          \\ simp []
+          \\ qsuff_tac ‘MEM wh_Diverge (MAP eval_wh eL) ⇔ MEM wh_Diverge (MAP eval_wh eL')’
+          >- (strip_tac
+              \\ IF_CASES_TAC
+              \\ simp []
+              \\ irule LIST_EQ
+              \\ rw []
+              \\ gvs [LIST_REL_EL_EQN, EL_MAP, EVERY_EL]
+              \\ rpt $ first_x_assum drule
+              \\ once_rewrite_tac [v_unfold]
+              \\ rpt FULL_CASE_TAC
+              \\ rw [dest_Atom_def, error_Atom_def])
+          \\ eq_tac
+          \\ strip_tac
+          \\ gvs [MEM_EL, LIST_REL_EL_EQN]
+          \\ first_assum $ irule_at Any
+          \\ first_assum drule
+          \\ once_rewrite_tac [v_unfold]
+          \\ rpt FULL_CASE_TAC
+          \\ gvs [EL_MAP])
+      \\ eq_tac
+      \\ strip_tac
+      \\ gvs [EXISTS_MEM, MEM_EL, EL_MAP, LIST_REL_EL_EQN]
+      \\ rename1 ‘MAP eval_wh eL2’
+      \\ qexists_tac ‘eval_wh (EL n eL2)’
+      \\ first_x_assum drule
+      \\ once_rewrite_tac [v_unfold]
+      \\ rpt FULL_CASE_TAC
+      \\ fs [error_Atom_def]
+      \\ rw []
+      \\ first_assum $ irule_at Any
+      \\ fs [EL_MAP])
+  \\ Cases_on ‘eL’ \\ Cases_on ‘eL'’ \\ fs []
+  \\ rename1 ‘LIST_REL _ t1 t2’
+  \\ Cases_on ‘t1’ \\ Cases_on ‘t2’ \\ gvs [eval_thm]
+  >~[‘Prim Seq (_::_::_)’]
+  >- (rename1 ‘LIST_REL _ t1 t2’
+      \\ Cases_on ‘t1’ \\ Cases_on ‘t2’
+      \\ gvs [eval_thm, eval_def]
+      \\ once_rewrite_tac [v_unfold]
+      \\ fs [eval_wh_Prim])
+  >~[‘Prim If (_::_::_)’]
+  >- (rename1 ‘LIST_REL _ t1 t2’
+      \\ Cases_on ‘t1’ \\ Cases_on ‘t2’ \\ gvs []
+      >~[‘_::_::_::_’]
+      >- (rename1 ‘LIST_REL _ t1 t2’
+          \\ Cases_on ‘t1’ \\ Cases_on ‘t2’
+          \\ gvs [eval_thm, eval_def]
+          \\ once_rewrite_tac [v_unfold]
+          \\ rw [eval_wh_Prim])
+      \\ rw [eval_def]
+      \\ once_rewrite_tac [v_unfold]
+      \\ rw [eval_wh_Prim])
+  \\ rw [eval_def]
+  \\ once_rewrite_tac [v_unfold]
+  \\ rw [eval_wh_Prim]
+QED
+
+Theorem FLOOKUP_LUPDATE:
+  ∀l f n v. FLOOKUP (f |++ l) n = SOME v ⇒ MEM (n, v) l ∨ FLOOKUP f n = SOME v
+Proof
+  Induct
+  \\ fs [FUPDATE_LIST_THM]
+  \\ PairCases \\ rw []
+  \\ first_x_assum $ dxrule_then assume_tac
+  \\ gvs [FLOOKUP_UPDATE]
+  \\ FULL_CASE_TAC \\ fs []
+QED
+
+Theorem Letrec_Prim:
+  ∀l ope eL b. (Letrec l (Prim ope eL) ≅? Prim ope (MAP (Letrec l) eL)) b
+Proof
+  rw []
+  \\ irule eval_IMP_exp_eq
+  \\ rw [subst_def, eval_thm, subst_funs_def, bind_def]
+  >- (irule eval_Prim
+      \\ rw [LIST_REL_EL_EQN, EL_MAP, subst_def, eval_thm, subst_funs_def]
+      \\ gvs [bind_def]
+      \\ IF_CASES_TAC \\ fs []
+      \\ first_x_assum dxrule
+      \\ strip_tac
+      \\ fs [])
+  \\ fs [MAP_MAP_o]
+  \\ dxrule_then assume_tac FLOOKUP_LUPDATE
+  \\ gvs [FLOOKUP_EMPTY, MEM_EL, EL_MAP]
+  \\ qsuff_tac ‘F’ \\ fs []
+  \\ first_x_assum irule
+  \\ rename1 ‘EL k l’
+  \\ qabbrev_tac ‘p = EL k l’
+  \\ PairCases_on ‘p’
+  \\ gvs [EVERY_EL, EL_MAP]
+  \\ rw []
+  \\ rename1 ‘EL k2 l’
+  \\ qabbrev_tac ‘p' = EL k2 l’
+  \\ PairCases_on ‘p'’
+  \\ gvs []
+  \\ ‘∀v. v ∈ FRANGE (FDIFF f (set (MAP FST l))) ⇒ closed v’
+    by (rw []
+        \\ first_x_assum irule
+        \\ gvs [FRANGE_FLOOKUP, FLOOKUP_FDIFF]
+        \\ pop_assum $ irule_at Any)
+  \\ gvs [freevars_subst, SUBSET_DEF, IN_DIFF, FDOM_FDIFF]
+  \\ rw [MEM_EL]
+  >>~[‘EL _ (MAP FST _) = EL _ (MAP FST _)’]
+  >- (first_assum $ irule_at Any
+      \\ gvs [EL_MAP]
+      \\ rename1 ‘FST p = FST _’
+      \\ PairCases_on ‘p’
+      \\ fs [])
+  >- (first_assum $ irule_at Any
+      \\ gvs [EL_MAP]
+      \\ rename1 ‘FST p = FST _’
+      \\ PairCases_on ‘p’
+      \\ fs [])
+  \\ first_x_assum $ qspecl_then [‘x’] assume_tac
+  \\ pop_assum kall_tac
+  \\ first_x_assum $ qspecl_then [‘x’] assume_tac
+  \\ gvs [] >>~[‘MEM x (MAP FST l)’]
+  >- (gvs [MEM_EL]
+      \\ first_assum $ irule_at Any
+      \\ fs [EL_MAP]
+      \\ rename1 ‘FST p = FST _’
+      \\ PairCases_on ‘p’ \\ fs [])
+  >- (gvs [MEM_EL]
+      \\ first_assum $ irule_at Any
+      \\ fs [EL_MAP]
+      \\ rename1 ‘FST p = FST _’
+      \\ PairCases_on ‘p’ \\ fs [])
+  \\ first_x_assum $ qspecl_then [‘freevars p'1’] assume_tac
+  \\ gvs [MEM_MAP]
+  \\ pop_assum $ qspecl_then [‘EL k2 l’] assume_tac
+  \\ gvs [EL_MEM]
+QED
+
+Theorem Let_Lam:
+  ∀v w e1 e2 b. closed e1 ∧ v ≠ w ⇒ (Let v e1 (Lam w e2) ≅? Lam w (Let v e1 e2)) b
+Proof
+  rw []
+  \\ irule exp_eq_trans
+  \\ irule_at Any beta_equality
+  \\ gvs [subst1_def]
+  \\ irule exp_eq_Lam_cong
+  \\ irule $ iffLR exp_eq_sym
+  \\ irule beta_equality
+  \\ gvs []
+QED
+
+Theorem Let_Lam_weak:
+  ∀v w e1 e2 b. v ≠ w ⇒ w ∉ freevars e1 ⇒ (Let v e1 (Lam w e2) ≅? Lam w (Let v e1 e2)) b
+Proof
+  rw [exp_eq_def, bind_def] >> IF_CASES_TAC >>
+  gvs [app_bisimilarity_eq, exp_eq_refl] >>
+  rpt (irule_at Any IMP_closed_subst) >>
+  drule_then assume_tac $ GSYM subst_fdomsub >>
+  gvs [subst_def, DOMSUB_COMMUTES] >>
+  irule_at Any Let_Lam >>
+  irule_at Any IMP_closed_subst >>
+  rw [FRANGE_FLOOKUP]
+QED
+
+Theorem FDIFF_DOMSUB:
+  ∀f v s. FDIFF (f \\ s) v = (FDIFF f v) \\ s
+Proof
+  rw [FDIFF_def, fmap_domsub, INTER_COMM]
+QED
+
+Theorem MAP_subst_fdomsub:
+  ∀v l f. EVERY (λe. v ∉ freevars e) (MAP SND l) ⇒
+          MAP (λ(s, e). (s, subst (FDIFF f (set (MAP FST l)) \\ v) e)) l
+          = MAP (λ(s, e). (s, subst (FDIFF f (set (MAP FST l))) e)) l
+Proof
+  rw [EVERY_EL] >> irule LIST_EQ >>
+  rw [EL_MAP] >> first_x_assum $ drule_then assume_tac >>
+  rename1 ‘EL x l’ >> qabbrev_tac ‘p = EL x l’ >> PairCases_on ‘p’ >>
+  gvs [subst_fdomsub, EL_MAP]
+QED
+
+Theorem Letrec_Lam:
+  ∀l w e b. EVERY (λe. freevars e ⊆ set (MAP FST l)) (MAP SND l) ∧ ¬MEM w (MAP FST l)
+          ⇒ (Letrec l (Lam w e) ≅? Lam w (Letrec l e)) b
+Proof
+  rw []
+  \\ irule exp_eq_trans
+  \\ irule_at Any beta_equality_Letrec
+  \\ gvs [subst_funs_eq_subst, subst_def]
+  \\ irule exp_eq_Lam_cong
+  \\ irule $ iffLR exp_eq_sym
+  \\ irule exp_eq_trans
+  \\ irule_at Any beta_equality_Letrec
+  \\ gvs [subst_funs_eq_subst]
+  \\ irule eval_IMP_exp_eq
+  \\ rw []
+  \\ rpt AP_TERM_TAC \\ AP_THM_TAC \\ AP_TERM_TAC
+  \\ irule $ GSYM DOMSUB_NOT_IN_DOM
+  \\ gvs [FDOM_FUPDATE_LIST]
+  \\ strip_tac \\ last_x_assum irule
+  \\ gvs [MEM_EL]
+  \\ first_assum $ irule_at Any
+  \\ gvs [EL_MAP]
+  \\ rename1 ‘FST (_ p)’
+  \\ PairCases_on ‘p’
+  \\ fs []
+QED
+
+Theorem Letrec_Lam_weak:
+  ∀l v e b. EVERY (λe. v ∉ freevars e) (MAP SND l) ∧ ¬ MEM v (MAP FST l)
+            ⇒ (Letrec l (Lam v e) ≅? Lam v (Letrec l e)) b
+Proof
+  rw [exp_eq_def, bind_def] >> IF_CASES_TAC >>
+  gvs [app_bisimilarity_eq, exp_eq_refl] >>
+  rpt $ irule_at Any IMP_closed_subst >>
+  gvs [subst_def, FDIFF_DOMSUB, MAP_subst_fdomsub] >>
+  irule_at Any Letrec_Lam >>
+  gvs [MAP_MAP_o, combinTheory.o_DEF, LAMBDA_PROD, EVERY_EL, EL_MAP] >>
+  rw [FRANGE_FLOOKUP]
+  >- (rename1 ‘EL n l’ >> qabbrev_tac ‘p = EL n l’ >>
+      PairCases_on ‘p’ >>
+      ‘∀v. v ∈ FRANGE (FDIFF f (set (MAP FST l))) ⇒ closed v’
+        by (rw [FRANGE_FLOOKUP, FLOOKUP_FDIFF] >>
+            first_x_assum irule >>
+            pop_assum $ irule_at Any) >>
+      gvs [freevars_subst, SUBSET_DEF, IN_DIFF, FDOM_FDIFF] >>
+      gen_tac >> rename1 ‘MEM x _’ >>
+      last_x_assum $ qspecl_then [‘x’] assume_tac >>
+      last_x_assum $ qspecl_then [‘x’] assume_tac >>
+      rw [] >> gvs []
+      >- (last_x_assum $ qspecl_then [‘freevars p1’] assume_tac >>
+          gvs [MEM_MAP] >> pop_assum $ qspecl_then [‘EL n l’] assume_tac >>
+          gvs [EL_MEM])
+      >- (last_x_assum $ qspecl_then [‘freevars p1’] assume_tac >>
+          gvs [MEM_MAP] >> pop_assum $ qspecl_then [‘EL n l’] assume_tac >>
+          gvs [EL_MEM]) >>
+      gvs [MEM_EL] >>
+      first_assum $ irule_at Any >>
+      rw [EL_MAP] >>
+      rename1 ‘FST p2’ >> PairCases_on ‘p2’ >> fs [])
+  >- (strip_tac >> last_x_assum irule >>
+      gvs [MEM_EL] >> first_assum $ irule_at Any >>
+      gvs [EL_MAP] >> rename1 ‘FST p’ >> PairCases_on ‘p’ >>
+      fs [])
+QED
+
+Theorem Let_not_in_freevars:
+  ∀v e e2 b. v ∉ freevars e2 ⇒ (Let v e e2 ≅? e2) b
+Proof
+  rw [] >>
+  irule eval_IMP_exp_eq >>
+  dxrule_then assume_tac $ GSYM subst_fdomsub >>
+  rw [subst_def, eval_thm, bind1_def, FRANGE_FLOOKUP, IMP_closed_subst]
+QED
+
+Theorem Letrec_not_in_freevars:
+  ∀l e b. EVERY (λv. v ∉ freevars e) (MAP FST l) ⇒ (Letrec l e ≅? e) b
+Proof
+  rw [exp_eq_def, bind_def] >> IF_CASES_TAC >>
+  gvs [app_bisimilarity_eq, exp_eq_refl] >>
+  rpt $ irule_at Any IMP_closed_subst >>
+  gvs [subst_def, FRANGE_FLOOKUP] >>
+  irule exp_eq_trans >>
+  irule_at Any beta_equality_Letrec >>
+  conj_asm1_tac
+  >- (rw [EVERY_EL, EL_MAP, MAP_MAP_o, combinTheory.o_DEF, LAMBDA_PROD] >>
+      rename1 ‘EL n l’ >> qabbrev_tac ‘p = EL n l’ >> PairCases_on ‘p’ >>
+      ‘∀v. v ∈ FRANGE (FDIFF f (set (MAP FST l))) ⇒ closed v’
+        by (rw [FRANGE_FLOOKUP, FLOOKUP_FDIFF] >>
+            first_x_assum irule >>
+            pop_assum $ irule_at Any) >>
+      gvs [freevars_subst, SUBSET_DEF, IN_DIFF, FDOM_FDIFF] >>
+      gen_tac >> rename1 ‘MEM x _’ >>
+      last_x_assum $ qspecl_then [‘x’] assume_tac >>
+      rw [] >> gvs []
+      >- (first_x_assum $ qspecl_then [‘freevars p1’] assume_tac >>
+          gvs [MEM_MAP] >> pop_assum $ qspecl_then [‘EL n l’] assume_tac >>
+          gvs [EL_MEM]) >>
+      gvs [MEM_EL] >>
+      first_assum $ irule_at Any >> rw [EL_MAP] >>
+      rename1 ‘FST p2’ >> PairCases_on ‘p2’ >> fs []) >>
+  dxrule_then assume_tac subst_funs_eq_subst >>
+  qspecl_then [‘f’, ‘e’, ‘set (MAP FST l)’] assume_tac $ GSYM subst_FDIFF' >>
+  gvs [EVERY_MEM] >>
+  rw [exp_eq_refl, IMP_closed_subst, FRANGE_FLOOKUP]
+QED
+
+Theorem Let_Letrec:
+  ∀s l e1 e2 b. EVERY (λe. s ∉ freevars e) (MAP SND l) ∧ ¬MEM s (MAP FST l)
+                ∧ EVERY (λv. v ∉ freevars e1) (MAP FST l)
+                ⇒ (Let s e1 (Letrec l e2) ≅? Letrec l (Let s e1 e2)) b
+Proof
+  rw [] >>
+  irule exp_eq_trans >>
+  irule_at (Pos hd) exp_eq_App_cong >>
+  irule_at (Pos hd) $ iffLR exp_eq_sym >>
+  irule_at Any Letrec_Lam_weak >> fs [] >>
+  irule_at Any exp_eq_refl >>
+  irule $ iffLR exp_eq_sym >>
+  irule exp_eq_trans >>
+  irule_at Any Letrec_App >>
+  irule exp_eq_App_cong >>
+  gvs [exp_eq_refl, Letrec_not_in_freevars]
+QED
+
+Theorem Let_Letrec2:
+  ∀s l e1 e2 b. ¬MEM s (MAP FST l)
+                ∧ EVERY (λv. v ∉ freevars e1) (MAP FST l)
+                ⇒ (Let s e1 (Letrec l e2) ≅? Letrec (MAP (λ(v, e). (v, Let s e1 e)) l)  (Let s e1 e2)) b
+Proof
+  rw [exp_eq_def, bind_def] >> IF_CASES_TAC >>
+  gvs [app_bisimilarity_eq, exp_eq_refl] >>
+  rpt $ irule_at Any IMP_closed_subst >>
+  gvs [subst_def, FRANGE_FLOOKUP] >>
+  irule exp_eq_trans >>
+  irule_at Any beta_equality >>
+  irule_at Any IMP_closed_subst >>
+  gvs [FRANGE_FLOOKUP, subst1_def, MAP_MAP_o] >>
+  rename1 ‘MEM s (MAP (FST o (λ(f', e). (f', subst (FDIFF (f \\ s) (set (MAP FST l))) e))) l)’ >>
+  ‘¬MEM s (MAP (FST o (λ(f', e). (f', subst (FDIFF (f \\ s) (set (MAP FST l))) e))) l)’
+    by (strip_tac >> first_x_assum irule >>
+        gvs [MEM_EL] >> first_assum $ irule_at Any >> gvs [EL_MAP] >>
+        rename1 ‘EL n l’ >> qabbrev_tac ‘p = EL n l’ >> PairCases_on ‘p’ >> fs []) >>
+  gvs [] >> irule exp_eq_Letrec_cong2 >>
+  irule_at Any fmap_rel_FUPDATE_LIST_same >> irule_at Any LIST_EQ >>
+  rw [EL_MAP, fmap_rel_FEMPTY, LIST_REL_EL_EQN]
+  >~[‘FST (_ (_ p)) = FST (_ (_ p))’]
+  >- (PairCases_on ‘p’ >> fs [])
+  >~[‘SND (_ (_ p)) ≅? SND (_ (_ p))’]
+  >- (PairCases_on ‘p’ >> gvs [subst_def] >>
+      gvs [EVERY_MEM] >> drule_then assume_tac $ GSYM subst_FDIFF' >>
+      ‘MAP (FST o (λ(v, e). (v, Let s e1 e))) l = MAP FST l’
+        by (irule LIST_EQ >> rw [EL_MAP] >> rename1 ‘FST (_ p)’ >> PairCases_on ‘p’ >> fs []) >>
+      gvs [FDIFF_def, fmap_domsub, INTER_COMM, Once exp_eq_sym] >>
+      irule beta_equality >>
+      gvs [IMP_closed_subst, FRANGE_FLOOKUP])
+  >- (‘MAP (FST o (λ(v, e). (v, Let s e1 e))) l = MAP FST l’
+        by (irule LIST_EQ >> rw [EL_MAP] >> rename1 ‘FST (_ p)’ >> PairCases_on ‘p’ >> fs []) >>
+      gvs [EVERY_MEM] >> drule_then assume_tac $ GSYM subst_FDIFF' >>
+      gvs [FDIFF_def, fmap_domsub, INTER_COMM, Once exp_eq_sym] >>
+      irule beta_equality >> gvs [IMP_closed_subst, FRANGE_FLOOKUP])
+QED
+
+Theorem Let_Let:
+  ∀v w e1 e2 e3 b. v ≠ w ∧ v ∉ freevars e2 ∧ w ∉ freevars e1 ⇒
+                   (Let v e1 (Let w e2 e3) ≅? Let w e2 (Let v e1 e3)) b
+Proof
+  rw []
+  \\ irule eval_IMP_exp_eq
+  \\ rw [subst_def]
+  \\ rename1 ‘subst (f \\ _ \\ _)’
+  \\ ‘∀v. v ∈ FRANGE f ⇒ closed v’ by (rw [FRANGE_FLOOKUP])
+  \\ drule $ GSYM subst_fdomsub
+  \\ last_x_assum assume_tac
+  \\ last_x_assum assume_tac
+  \\ drule $ GSYM subst_fdomsub
+  \\ rw [eval_Let, subst_def, bind1_def, IMP_closed_subst, DOMSUB_COMMUTES]
+  \\ AP_TERM_TAC
+  \\ rw [fmap_domsub, COMPL_UNION]
+  \\ irule subst1_subst1
+  \\ gvs [IMP_closed_subst]
+QED
+
+Theorem Let_Apps:
+  ∀eL v e1 e2 b. (Let v e1 (Apps e2 eL) ≅? Apps (Let v e1 e2) (MAP (Let v e1) eL)) b
+Proof
+  Induct >> rw [Apps_def, exp_eq_refl] >>
+  irule exp_eq_trans >> pop_assum $ irule_at Any >>
+  irule exp_eq_Apps_cong >> gvs [Let_App, exp_eq_l_refl]
+QED
+
+Theorem Letrec_Apps:
+  ∀eL bL e b. (Letrec bL (Apps e eL) ≅? Apps (Letrec bL e) (MAP (Letrec bL) eL)) b
+Proof
+  Induct >> rw [Apps_def, exp_eq_refl] >>
+  irule exp_eq_trans >> pop_assum $ irule_at Any >>
+  irule exp_eq_Apps_cong >> gvs [exp_eq_l_refl, Letrec_App]
+QED
+
+Theorem App_Seq:
   ∀b. (App (Seq p f) e ≅? Seq p (App f e)) b
 Proof
   irule eval_wh_IMP_exp_eq
   \\ rw [subst_def, eval_wh_App, eval_wh_Seq]
   \\ fs []
+QED
+
+Theorem Apps_Seq:
+  ∀eL e e' b. (Apps (Seq e e') eL ≅? Seq e (Apps e' eL)) b
+Proof
+  Induct >> rw [Apps_def, exp_eq_refl] >>
+  irule exp_eq_trans >> pop_assum $ irule_at Any >>
+  irule exp_eq_Apps_cong >> gvs [exp_eq_l_refl, App_Seq]
 QED
 
 Theorem Proj_Seq2:
@@ -80,7 +562,7 @@ Proof
 QED
 
 Theorem IsEq_Seq:
-  ∀b e e' n i. (IsEq n i (Seq e e') ≅? Seq e (IsEq n i e')) b
+  ∀b b2 e e' n i. (IsEq n i b2 (Seq e e') ≅? Seq e (IsEq n i b2 e')) b
 Proof
   rpt gen_tac
   \\ irule eval_wh_IMP_exp_eq
@@ -88,11 +570,10 @@ Proof
   \\ fs []
 QED
 
-
 Definition well_written_def:
   well_written (Cons s) l = T ∧
   well_written (Proj s i) [e] = T ∧
-  well_written (IsEq s i) [e] = T ∧
+  well_written (IsEq s i b) [e] = T ∧
   well_written If [e; e'; e''] = T ∧
   well_written Seq [e; e'] = T ∧
   well_written (AtomOp op) l = T ∧
@@ -136,12 +617,905 @@ Proof
   \\ fs [subst_def, eval_wh_def, eval_wh_to_def]
 QED
 
-Theorem exp_eq_l_refl:
-  ∀b l. LIST_REL (λx y. (x ≅? y) b) l l
+(* Part on context *)
+
+Theorem eq_when_applied_refl:
+  ∀c e len. eq_when_applied c e e len
+Proof
+  Induct
+  \\ gvs [eq_when_applied_def, exp_eq_refl]
+QED
+
+Theorem eq_when_applied_l_refl:
+  ∀c l len. LIST_REL (λe1 e2. eq_when_applied c e1 e2 len) l l
 Proof
   gen_tac
   \\ Induct
-  \\ fs [exp_eq_refl]
+  \\ fs [eq_when_applied_refl]
+QED
+
+Theorem eq_when_applied_sym:
+  ∀c e1 e2 len. eq_when_applied c e1 e2 len ⇔ eq_when_applied c e2 e1 len
+Proof
+  Induct
+  \\ rw [] \\ eq_tac
+  \\ gvs [eq_when_applied_def, exp_eq_sym]
+QED
+
+Theorem eq_when_applied_trans:
+  ∀c e1 e2 e3 len. eq_when_applied c e1 e2 len
+                   ∧ eq_when_applied c e2 e3 len
+                   ⇒ eq_when_applied c e1 e3 len
+Proof
+  Induct
+  \\ rw []
+  \\ gvs [eq_when_applied_def] \\ rw []
+  >- (irule exp_eq_trans
+      \\ pop_assum $ irule_at Any \\ fs [])
+  \\ last_x_assum irule
+  \\ first_x_assum $ irule_at Any
+  \\ gvs []
+QED
+
+Theorem exp_eq_in_ctxt_refl:
+  ∀c e. exp_eq_in_ctxt c e e
+Proof
+  Induct
+  \\ gvs [exp_eq_in_ctxt_def, exp_eq_refl]
+QED
+
+Theorem exp_eq_in_ctxt_l_refl:
+  ∀c l. LIST_REL (exp_eq_in_ctxt c) l l
+Proof
+  gen_tac
+  \\ Induct
+  \\ fs [exp_eq_in_ctxt_refl]
+QED
+
+Theorem exp_eq_in_ctxt_sym:
+  ∀c e1 e2. exp_eq_in_ctxt c e1 e2 ⇔ exp_eq_in_ctxt c e2 e1
+Proof
+  gvs [eq_when_applied_0, eq_when_applied_sym]
+QED
+
+Theorem exp_eq_in_ctxt_trans:
+  ∀c e1 e2 e3. exp_eq_in_ctxt c e1 e2 ∧ exp_eq_in_ctxt c e2 e3 ⇒ exp_eq_in_ctxt c e1 e3
+Proof
+  rw [eq_when_applied_0] >>
+  dxrule_then (dxrule_then irule) eq_when_applied_trans
+QED
+
+Theorem last_exists:
+  ∀l. LENGTH l > 0 ⇒ ∃x t. l = SNOC x t
+Proof
+  Induct
+  \\ fs []
+  \\ rw []
+  \\ rename1 ‘hd::tl’
+  \\ Cases_on ‘tl’
+  \\ fs []
+QED
+
+Theorem last_Apps:
+  ∀l x e. Apps e (l ++ [x]) = App (Apps e l) x
+Proof
+  Induct
+  \\ fs [Apps_def]
+QED
+
+Theorem eq_when_applied_SUC:
+  ∀c e1 e2 len. eq_when_applied c e1 e2 len
+                ⇒ eq_when_applied c e1 e2 (SUC len)
+Proof
+  Induct >> gvs [eq_when_applied_def] >>
+  rpt gen_tac >> strip_tac >> rw [] >>
+  qspecl_then [‘l’] assume_tac last_exists >> gvs [last_Apps] >>
+  irule exp_eq_App_cong >>
+  last_x_assum $ irule_at Any >>
+  gvs [exp_eq_refl]
+QED
+
+Theorem eq_when_applied_bigger:
+  ∀len2 len1 c e1 e2. eq_when_applied c e1 e2 len1 ∧ len1 ≤ len2
+                      ⇒ eq_when_applied c e1 e2 len2
+Proof
+  Induct >> gvs [] >> gen_tac >>
+  rename1 ‘len1 ≤ SUC len2’ >> Cases_on ‘len1 = SUC len2’ >> rw [] >>
+  irule eq_when_applied_SUC >> last_x_assum $ dxrule_then irule >>
+  gvs []
+QED
+
+Theorem exp_eq_in_ctxt_IMP_eq_when_applied:
+  ∀c e1 e2 len. exp_eq_in_ctxt c e1 e2 ⇒ eq_when_applied c e1 e2 len
+Proof
+  Induct >>
+  gvs [exp_eq_in_ctxt_def, eq_when_applied_def, exp_eq_Apps_cong, exp_eq_l_refl]
+QED
+
+Theorem exp_eq_IMP_exp_eq_in_ctxt:
+  ∀c e e'. e ≈ e' ⇒ exp_eq_in_ctxt c e e'
+Proof
+  Induct
+  \\ gvs [exp_eq_in_ctxt_def]
+  \\ rw []
+  \\ first_x_assum irule
+  \\ gvs [exp_eq_Letrec_cong, exp_eq_App_cong, exp_eq_Lam_cong, exp_eq_refl, exp_eq_l_refl]
+QED
+
+Theorem exp_eq_IMP_eq_when_applied:
+  ∀c e e' len. e ≈ e' ⇒ eq_when_applied c e e' len
+Proof
+  rw [] \\ irule exp_eq_in_ctxt_IMP_eq_when_applied
+  \\ gvs [exp_eq_IMP_exp_eq_in_ctxt]
+QED
+
+Theorem exp_eq_in_ctxt_Prim:
+  ∀c eL eL' ope. LIST_REL (exp_eq_in_ctxt c) eL eL'
+                 ⇒ exp_eq_in_ctxt c (Prim ope eL) (Prim ope eL')
+Proof
+  Induct
+  \\ gvs [exp_eq_in_ctxt_def, exp_eq_refl, exp_eq_Prim_cong]
+  \\ rw []
+  \\ irule exp_eq_in_ctxt_trans
+  \\ irule_at Any exp_eq_in_ctxt_trans
+  \\ last_x_assum $ irule_at Any
+  \\ irule_at (Pos last) exp_eq_IMP_exp_eq_in_ctxt
+  \\ irule_at (Pos last) exp_eq_IMP_exp_eq_in_ctxt
+  >~[‘Letrec’]
+  >- (irule_at Any Letrec_Prim
+      \\ irule_at Any $ iffLR exp_eq_sym
+      \\ irule_at Any Letrec_Prim
+      \\ gvs [LIST_REL_EL_EQN, EL_MAP, exp_eq_in_ctxt_def])
+  \\ irule_at Any Let_Prim
+  \\ irule_at Any $ iffLR exp_eq_sym
+  \\ irule_at Any Let_Prim
+  \\ gvs [LIST_REL_EL_EQN, EL_MAP, exp_eq_in_ctxt_def]
+QED
+
+Theorem Let_App_w_app:
+  ∀c s e1 e2 e3 len. eq_when_applied c (Let s e1 (App e2 e3)) (App (Let s e1 e2) (Let s e1 e3)) len
+Proof
+  rpt gen_tac
+  \\ irule exp_eq_IMP_eq_when_applied
+  \\ gvs [Let_App]
+QED
+
+Theorem Let_App_in_ctxt:
+  ∀c s e1 e2 e3. exp_eq_in_ctxt c (Let s e1 (App e2 e3)) (App (Let s e1 e2) (Let s e1 e3))
+Proof
+  gvs [eq_when_applied_0, Let_App_w_app]
+QED
+
+Theorem exp_eq_in_ctxt_App:
+  ∀c f1 f2 e1 e2. exp_eq_in_ctxt c f1 f2 ∧ exp_eq_in_ctxt c e1 e2
+                  ⇒ exp_eq_in_ctxt c (App f1 e1) (App f2 e2)
+Proof
+  Induct
+  \\ gvs [exp_eq_in_ctxt_def,exp_eq_App_cong]
+  \\ rw []
+  \\ irule exp_eq_in_ctxt_trans
+  \\ irule_at Any exp_eq_in_ctxt_trans
+  \\ last_x_assum $ irule_at (Pos $ el 2)
+  \\ first_x_assum $ irule_at (Pos $ el 2)
+  \\ rpt $ last_assum $ irule_at Any
+  \\ irule_at (Pos last) $ iffLR exp_eq_in_ctxt_sym
+  \\ rpt $ irule_at Any Let_App_in_ctxt
+  \\ fs [Letrec_App, exp_eq_IMP_exp_eq_in_ctxt]
+QED
+
+Theorem eq_when_applied_App:
+  ∀c f1 f2 e1 e2 len. eq_when_applied c f1 f2 (SUC len) ∧ exp_eq_in_ctxt c e1 e2
+                  ⇒ eq_when_applied c (App f1 e1) (App f2 e2) len
+Proof
+  Induct
+  \\ gvs [eq_when_applied_def,exp_eq_App_cong, GSYM Apps_def, exp_eq_in_ctxt_def]
+  \\ rw []
+  >- (irule exp_eq_trans >> last_x_assum $ irule_at Any >>
+      gvs [exp_eq_Apps_cong, exp_eq_l_refl, exp_eq_App_cong, exp_eq_refl])
+  \\ irule eq_when_applied_trans
+  \\ irule_at Any eq_when_applied_trans
+  \\ last_x_assum $ irule_at (Pos $ el 2)
+  \\ first_x_assum $ irule_at (Pos $ el 2)
+  \\ rpt $ last_assum $ irule_at Any
+  \\ irule_at (Pos last) $ iffLR eq_when_applied_sym
+  \\ rpt $ irule_at Any Let_App_w_app
+  \\ fs [Letrec_App, exp_eq_IMP_eq_when_applied]
+QED
+
+Theorem SUC_ADD:
+  ∀n m. SUC (n + m) = n + SUC m
+Proof
+  gvs []
+QED
+
+Theorem eq_when_applied_Apps:
+  ∀eL eL' e e' c len. LIST_REL (exp_eq_in_ctxt c) eL eL' ⇒ eq_when_applied c e e' (len + LENGTH eL)
+                  ⇒ eq_when_applied c (Apps e eL) (Apps e' eL') len
+Proof
+  Induct
+  >- (Cases
+      \\ fs [Apps_def])
+  \\ gen_tac
+  \\ Cases
+  \\ rw [Apps_def]
+  \\ first_x_assum irule
+  \\ fs []
+  \\ irule eq_when_applied_App
+  \\ gvs [SUC_ADD]
+QED
+
+Theorem exp_eq_in_ctxt_Apps:
+  ∀eL eL' e e' c. LIST_REL (exp_eq_in_ctxt c) eL eL' ⇒ exp_eq_in_ctxt c e e'
+                  ⇒ exp_eq_in_ctxt c (Apps e eL) (Apps e' eL')
+Proof
+  Induct
+  >- (Cases
+      \\ fs [Apps_def])
+  \\ gen_tac
+  \\ Cases
+  \\ rw [Apps_def]
+  \\ first_x_assum irule
+  \\ fs []
+  \\ irule exp_eq_in_ctxt_App
+  \\ gvs [SUC_ADD]
+QED
+
+Theorem Let_freevars_in_ctxt:
+  ∀c v e e'. v ∉ freevars e' ⇒ exp_eq_in_ctxt c (Let v e e') e'
+Proof
+  rw []
+  \\ irule exp_eq_IMP_exp_eq_in_ctxt
+  \\ irule eval_wh_IMP_exp_eq
+  \\ rw [subst_def, eval_wh_thm, bind1_def, GSYM subst_fdomsub]
+  >- (AP_TERM_TAC
+      \\ irule subst1_ignore
+      \\ rename1 ‘subst f e2’
+      \\ qsuff_tac ‘closed (subst f e2)’
+      >- rw [closed_def]
+      \\ irule IMP_closed_subst
+      \\ rw []
+      \\ first_x_assum $ irule_at Any
+      \\ fs [FRANGE_FLOOKUP]
+      \\ pop_assum $ irule_at Any)
+  \\ gvs [IMP_closed_subst, FRANGE_FLOOKUP]
+QED
+
+Theorem Let_freevars_w_app:
+  ∀c v e e' len. v ∉ freevars e' ⇒ eq_when_applied c (Let v e e') e' len
+Proof
+  rw [] >>
+  irule exp_eq_in_ctxt_IMP_eq_when_applied >>
+  gvs [Let_freevars_in_ctxt]
+QED
+
+Theorem Let_Let_in_ctxt:
+  ∀v w e1 e2 e3 c. v ≠ w ∧ v ∉ freevars e2 ∧ w ∉ freevars e1 ⇒
+                   exp_eq_in_ctxt c (Let v e1 (Let w e2 e3)) (Let w e2 (Let v e1 e3))
+Proof
+  rw []
+  \\ irule exp_eq_IMP_exp_eq_in_ctxt
+  \\ gvs [Let_Let]
+QED
+
+Theorem Let_Let_eq_w_app:
+  ∀v w e1 e2 e3 c len. v ≠ w ∧ v ∉ freevars e2 ∧ w ∉ freevars e1 ⇒
+                   eq_when_applied c (Let v e1 (Let w e2 e3)) (Let w e2 (Let v e1 e3)) len
+Proof
+  rw []
+  \\ irule exp_eq_IMP_eq_when_applied
+  \\ gvs [Let_Let]
+QED
+
+Theorem exp_eq_in_ctxt_Lam:
+  ∀c s e1 e2. exp_eq_in_ctxt (IsFree s c) e1 e2
+              ⇒ exp_eq_in_ctxt c (Lam s e1) (Lam s e2)
+Proof
+  Induct
+  \\ fs[exp_eq_in_ctxt_def] \\ rw [exp_eq_in_ctxt_def]
+  >- (rw [exp_eq_Lam_strong]
+      \\ irule exp_eq_trans
+      \\ irule_at Any beta_equality
+      \\ fs []
+      \\ irule $ iffLR exp_eq_sym
+      \\ irule exp_eq_trans
+      \\ irule_at (Pos last) beta_equality
+      \\ fs [exp_eq_sym])
+  >>~ [‘Letrec l (Lam w _)’]
+  >- (‘∃s. s ∉ {w} ∪ set (MAP FST l) ∪ BIGUNION (set (MAP (freevars o SND) l))
+             ∪ freevars e1 ∪ freevars e2’
+        by  (‘INFINITE 𝕌(:string)’ by simp [] \\ dxrule_then assume_tac $ iffLR NOT_IN_FINITE
+             \\ pop_assum $ irule_at Any \\ rw [FINITE_UNION, FINITE_BIGUNION, MEM_EL]
+             \\ gvs [EL_MAP])
+      \\ irule exp_eq_in_ctxt_trans
+      \\ irule_at (Pos hd) exp_eq_IMP_exp_eq_in_ctxt
+      \\ irule_at Any exp_eq_Letrec_cong
+      \\ irule_at Any exp_eq_l_refl
+      \\ irule_at Any exp_alpha_exp_eq
+      \\ irule_at Any exp_alpha_Alpha
+      \\ fs [] \\ first_assum $ irule_at Any
+      \\ fs []
+      \\ irule exp_eq_in_ctxt_trans
+      \\ irule_at (Pos hd) exp_eq_IMP_exp_eq_in_ctxt
+      \\ irule_at Any Letrec_Lam_weak
+      \\ fs [] \\ conj_tac
+      >- (rw [EVERY_MEM]
+          \\ rename1 ‘MEM e _’ \\ last_x_assum $ qspecl_then [‘freevars e’] assume_tac
+          \\ fs [MEM_MAP]
+          \\ rename1 ‘e = SND pair’ \\ pop_assum $ qspecl_then [‘pair’] assume_tac
+          \\ rw [])
+      \\ irule exp_eq_in_ctxt_trans
+      \\ irule_at (Pos last) exp_eq_IMP_exp_eq_in_ctxt
+      \\ irule_at Any $ iffLR exp_eq_sym
+      \\ irule_at Any exp_eq_Letrec_cong
+      \\ irule_at Any exp_alpha_exp_eq
+      \\ irule_at Any exp_alpha_Alpha
+      \\ irule_at Any exp_eq_l_refl
+      \\ first_assum $ irule_at Any \\ fs []
+      \\ irule exp_eq_in_ctxt_trans
+      \\ irule_at (Pos last) exp_eq_IMP_exp_eq_in_ctxt
+      \\ irule_at Any $ iffLR exp_eq_sym
+      \\ irule_at Any Letrec_Lam_weak
+      \\ fs []
+      \\ conj_tac
+      >- (rw [EVERY_MEM]
+          \\ rename1 ‘MEM e _’ \\ last_x_assum $ qspecl_then [‘freevars e’] assume_tac
+          \\ fs [MEM_MAP]
+          \\ rename1 ‘e = SND pair’ \\ pop_assum $ qspecl_then [‘pair’] assume_tac
+          \\ rw [])
+      \\ last_x_assum irule \\ rw []
+      \\ irule exp_eq_in_ctxt_trans
+      \\ irule_at Any exp_eq_in_ctxt_trans
+      \\ last_x_assum $ irule_at Any
+      \\ irule_at (Pos last) $ iffLR exp_eq_in_ctxt_sym
+      \\ rename1 ‘Let s e3 _’ \\ qexists_tac ‘e3’ \\ fs []
+      \\ conj_tac
+      \\ irule exp_eq_IMP_exp_eq_in_ctxt
+      \\ irule exp_eq_trans
+      \\ irule_at Any Let_Letrec
+      \\ fs []
+      \\ irule_at Any exp_eq_Letrec_cong
+      \\ irule_at Any $ iffLR exp_eq_sym
+      \\ irule_at Any exp_eq_App_cong
+      \\ irule_at Any exp_alpha_exp_eq
+      \\ irule_at Any exp_alpha_Alpha
+      \\ rw [EVERY_MEM, exp_eq_refl, exp_eq_l_refl] \\ fs [closed_def]
+      \\ rename1 ‘MEM e _’
+      \\ last_x_assum $ qspecl_then [‘freevars e’] assume_tac
+      \\ fs [MEM_MAP]
+      \\ rename1 ‘e = SND pair’ \\ pop_assum $ qspecl_then [‘pair’] assume_tac
+      \\ rw [])
+  \\ rename1 ‘Let v e3 (Lam w _)’
+  \\ ‘∃s. s ∉ {v} ∪ {w} ∪ freevars e3 ∪ freevars e1 ∪ freevars e2’
+    by (‘INFINITE 𝕌(:string)’ by simp []
+        \\ gvs [NOT_IN_FINITE])
+  \\ irule exp_eq_in_ctxt_trans
+  \\ irule_at (Pos hd) exp_eq_IMP_exp_eq_in_ctxt
+  \\ irule_at Any exp_eq_App_cong \\ irule_at Any exp_eq_Lam_cong
+  \\ irule_at Any exp_alpha_exp_eq
+  \\ irule_at Any exp_alpha_Alpha
+  \\ fs [] \\ first_assum $ irule_at Any
+  \\ irule_at Any exp_eq_refl \\ fs []
+  \\ irule exp_eq_in_ctxt_trans
+  \\ irule_at (Pos hd) exp_eq_IMP_exp_eq_in_ctxt
+  \\ irule_at Any Let_Lam_weak \\ fs []
+  \\ irule exp_eq_in_ctxt_trans
+  \\ irule_at (Pos last) exp_eq_IMP_exp_eq_in_ctxt
+  \\ irule_at Any $ iffLR exp_eq_sym
+  \\ irule_at Any exp_eq_App_cong \\ irule_at Any exp_eq_Lam_cong
+  \\ irule_at Any exp_alpha_exp_eq
+  \\ irule_at Any exp_alpha_Alpha
+  \\ first_assum $ irule_at Any
+  \\ irule_at Any exp_eq_refl \\ fs []
+  \\ irule exp_eq_in_ctxt_trans
+  \\ irule_at (Pos last) exp_eq_IMP_exp_eq_in_ctxt
+  \\ irule_at Any $ iffLR exp_eq_sym
+  \\ irule_at Any Let_Lam_weak \\ fs []
+  \\ last_x_assum $ irule_at Any
+  \\ rw []
+  \\ irule exp_eq_in_ctxt_trans \\ irule_at Any exp_eq_in_ctxt_trans
+  \\ last_x_assum $ irule_at Any
+  \\ rpt $ irule_at Any exp_eq_IMP_exp_eq_in_ctxt
+  \\ irule_at (Pos $ el 2) $ iffLR exp_eq_sym
+  \\ irule_at (Pos $ el 2) exp_eq_trans \\ irule_at (Pos $ el 3) exp_eq_trans
+  \\ irule_at (Pos $ el 2) Let_Let \\ irule_at (Pos $ el 6) Let_Let
+  \\ rpt $ irule_at Any exp_eq_App_cong
+  \\ rpt $ irule_at Any exp_eq_refl
+  \\ rpt $ irule_at Any exp_eq_Lam_cong
+  \\ rpt $ irule_at Any exp_eq_App_cong
+  \\ rpt $ irule_at Any exp_eq_refl
+  \\ fs [closed_def] \\ conj_tac
+  \\ irule exp_alpha_exp_eq
+  \\ irule exp_alpha_Alpha
+  \\ fs []
+QED
+
+Theorem exp_eq_in_ctxt_Lams:
+  ∀vl c e e'. exp_eq_in_ctxt (FOLDL (λc n. IsFree n c) c vl) e e' ⇒
+              exp_eq_in_ctxt c (Lams vl e) (Lams vl e')
+Proof
+  Induct
+  \\ rw [Lams_def]
+  \\ irule exp_eq_in_ctxt_Lam
+  \\ last_x_assum $ irule_at Any
+  \\ fs []
+QED
+
+Theorem eq_when_applied_Lam:
+  ∀c s e1 e2 len. eq_when_applied (IsFree s c) e1 e2 len
+              ⇒ eq_when_applied c (Lam s e1) (Lam s e2) (SUC len)
+Proof
+  Induct
+  \\ fs[eq_when_applied_def] \\ rw [eq_when_applied_def]
+  >~[‘Apps (Lam s e1) l ≈ Apps (Lam s e2) l’]
+  >- (‘∃v. v ∉ BIGUNION (set (MAP freevars l)) ∪ {s} ∪ freevars e1 ∪ freevars e2 ’
+        by  (‘INFINITE 𝕌(:string)’ by simp [] \\ dxrule_then assume_tac $ iffLR NOT_IN_FINITE
+             \\ pop_assum $ irule_at Any \\ rw [FINITE_UNION, FINITE_BIGUNION, MEM_EL]
+             \\ gvs [EL_MAP])
+      \\ irule exp_eq_trans \\ irule_at (Pos hd) exp_eq_Apps_cong
+      \\ irule_at Any exp_eq_l_refl
+      \\ irule_at (Pos hd) exp_alpha_exp_eq \\ irule_at Any exp_alpha_Alpha
+      \\ fs [] \\ first_assum $ irule_at Any \\ fs [Once exp_eq_sym]
+      \\ irule exp_eq_trans \\ irule_at (Pos hd) exp_eq_Apps_cong
+      \\ irule_at Any exp_eq_l_refl
+      \\ irule_at (Pos hd) exp_alpha_exp_eq \\ irule_at Any exp_alpha_Alpha
+      \\ fs [] \\ first_assum $ irule_at Any \\ fs [Once exp_eq_sym]
+      \\ Cases_on ‘l’ \\ gvs [Apps_def]
+      \\ irule exp_eq_trans \\ irule_at (Pos last) exp_eq_trans
+      \\ irule_at (Pos hd) Let_Apps \\ irule_at Any exp_eq_Apps_cong
+      \\ irule_at Any $ iffRL LIST_REL_EL_EQN \\ irule_at Any LENGTH_MAP
+      \\ irule_at (Pos $ el 2) exp_eq_refl
+      \\ conj_asm1_tac
+      >- (rw [EL_MAP] \\ irule eval_IMP_exp_eq
+          \\ rw [subst_def, eval_thm, IMP_closed_subst, FRANGE_FLOOKUP, bind1_def]
+          \\ rename1 ‘EL n t’ \\ first_x_assum $ qspecl_then [‘freevars (EL n t)’] assume_tac
+          \\ gvs [GSYM subst_fdomsub, subst1_ignore, closed_def, IMP_closed_subst, FRANGE_FLOOKUP, MEM_MAP]
+          \\ pop_assum $ qspecl_then [‘EL n t’] assume_tac
+          \\ gvs [MEM_EL])
+      \\ once_rewrite_tac [exp_eq_sym]
+      \\ irule exp_eq_trans \\ irule_at (Pos last) exp_eq_trans
+      \\ irule_at (Pos hd) Let_Apps \\ irule_at Any exp_eq_Apps_cong
+      \\ irule_at Any $ iffRL LIST_REL_EL_EQN \\ irule_at Any LENGTH_MAP
+      \\ irule_at (Pos $ el 2) exp_eq_refl \\ fs []
+      \\ irule_at Any exp_eq_App_cong \\ rw [exp_eq_Lam_strong, exp_eq_refl]
+      \\ irule exp_eq_trans \\ irule_at Any beta_equality \\ fs []
+      \\ irule $ iffLR exp_eq_sym
+      \\ irule exp_eq_trans \\ irule_at (Pos last) beta_equality \\ fs []
+      \\ irule exp_eq_trans \\ irule_at Any Let_Apps
+      \\ irule exp_eq_trans \\ irule_at Any exp_eq_Apps_cong
+      \\ irule_at Any $ iffRL LIST_REL_EL_EQN \\ irule_at Any LENGTH_MAP
+      \\ irule_at (Pos $ el 2) $ iffLR exp_eq_sym \\ irule_at Any exp_eq_App_cong
+      \\ irule_at (Pos hd) exp_alpha_exp_eq \\ irule_at Any exp_alpha_Alpha \\ fs []
+      \\ irule_at (Pos hd) exp_eq_refl
+      \\ conj_asm1_tac
+      >- (rw [EL_MAP] \\ irule eval_IMP_exp_eq
+          \\ rw [subst_def, eval_thm, IMP_closed_subst, FRANGE_FLOOKUP, bind1_def]
+          \\ rename1 ‘EL n t’ \\ first_x_assum $ qspecl_then [‘freevars (EL n t)’] assume_tac
+          \\ gvs [GSYM subst_fdomsub, subst1_ignore, closed_def, IMP_closed_subst, FRANGE_FLOOKUP, MEM_MAP]
+          \\ pop_assum $ qspecl_then [‘EL n t’] assume_tac
+          \\ gvs [MEM_EL])
+      \\ irule exp_eq_trans \\ last_x_assum $ irule_at Any \\ fs [Once exp_eq_sym]
+      \\ irule exp_eq_trans \\ irule_at Any Let_Apps \\ irule exp_eq_Apps_cong
+      \\ gvs [LIST_REL_EL_EQN, exp_eq_sym]
+      \\ irule exp_eq_App_cong \\ fs [exp_eq_refl]
+      \\ irule exp_alpha_exp_eq \\ irule exp_alpha_Alpha \\ fs [])
+  >>~ [‘Letrec l (Lam w _)’]
+  >- (‘∃s. s ∉ {w} ∪ set (MAP FST l) ∪ BIGUNION (set (MAP (freevars o SND) l))
+             ∪ freevars e1 ∪ freevars e2’
+        by  (‘INFINITE 𝕌(:string)’ by simp [] \\ dxrule_then assume_tac $ iffLR NOT_IN_FINITE
+             \\ pop_assum $ irule_at Any \\ rw [FINITE_UNION, FINITE_BIGUNION, MEM_EL]
+             \\ gvs [EL_MAP])
+      \\ irule eq_when_applied_trans
+      \\ irule_at (Pos hd) exp_eq_IMP_eq_when_applied
+      \\ irule_at Any exp_eq_Letrec_cong
+      \\ irule_at Any exp_eq_l_refl
+      \\ irule_at Any exp_alpha_exp_eq
+      \\ irule_at Any exp_alpha_Alpha
+      \\ fs [] \\ first_assum $ irule_at Any
+      \\ fs []
+      \\ irule eq_when_applied_trans
+      \\ irule_at (Pos hd) exp_eq_IMP_eq_when_applied
+      \\ irule_at Any Letrec_Lam_weak
+      \\ fs [] \\ conj_tac
+      >- (rw [EVERY_MEM]
+          \\ rename1 ‘MEM e _’ \\ last_x_assum $ qspecl_then [‘freevars e’] assume_tac
+          \\ fs [MEM_MAP]
+          \\ rename1 ‘e = SND pair’ \\ pop_assum $ qspecl_then [‘pair’] assume_tac
+          \\ rw [])
+      \\ irule eq_when_applied_trans
+      \\ irule_at (Pos last) exp_eq_IMP_eq_when_applied
+      \\ irule_at Any $ iffLR exp_eq_sym
+      \\ irule_at Any exp_eq_Letrec_cong
+      \\ irule_at Any exp_alpha_exp_eq
+      \\ irule_at Any exp_alpha_Alpha
+      \\ irule_at Any exp_eq_l_refl
+      \\ first_assum $ irule_at Any \\ fs []
+      \\ irule eq_when_applied_trans
+      \\ irule_at (Pos last) exp_eq_IMP_eq_when_applied
+      \\ irule_at Any $ iffLR exp_eq_sym
+      \\ irule_at Any Letrec_Lam_weak
+      \\ fs []
+      \\ conj_tac
+      >- (rw [EVERY_MEM]
+          \\ rename1 ‘MEM e _’ \\ last_x_assum $ qspecl_then [‘freevars e’] assume_tac
+          \\ fs [MEM_MAP]
+          \\ rename1 ‘e = SND pair’ \\ pop_assum $ qspecl_then [‘pair’] assume_tac
+          \\ rw [])
+      \\ last_x_assum irule \\ rw []
+      \\ irule eq_when_applied_trans
+      \\ irule_at Any eq_when_applied_trans
+      \\ last_x_assum $ irule_at Any
+      \\ irule_at (Pos last) $ iffLR eq_when_applied_sym
+      \\ rename1 ‘Let s e3 _’ \\ qexists_tac ‘e3’ \\ fs []
+      \\ conj_tac
+      \\ irule exp_eq_IMP_eq_when_applied
+      \\ irule exp_eq_trans
+      \\ irule_at Any Let_Letrec
+      \\ fs []
+      \\ irule_at Any exp_eq_Letrec_cong
+      \\ irule_at Any $ iffLR exp_eq_sym
+      \\ irule_at Any exp_eq_App_cong
+      \\ irule_at Any exp_alpha_exp_eq
+      \\ irule_at Any exp_alpha_Alpha
+      \\ rw [EVERY_MEM, exp_eq_refl, exp_eq_l_refl] \\ fs [closed_def]
+      \\ rename1 ‘MEM e _’
+      \\ last_x_assum $ qspecl_then [‘freevars e’] assume_tac
+      \\ fs [MEM_MAP]
+      \\ rename1 ‘e = SND pair’ \\ pop_assum $ qspecl_then [‘pair’] assume_tac
+      \\ rw [])
+  \\ rename1 ‘Let v e3 (Lam w _)’
+  \\ ‘∃s. s ∉ {v} ∪ {w} ∪ freevars e3 ∪ freevars e1 ∪ freevars e2’
+    by (‘INFINITE 𝕌(:string)’ by simp []
+        \\ gvs [NOT_IN_FINITE])
+  \\ irule eq_when_applied_trans
+  \\ irule_at (Pos hd) exp_eq_IMP_eq_when_applied
+  \\ irule_at Any exp_eq_App_cong \\ irule_at Any exp_eq_Lam_cong
+  \\ irule_at Any exp_alpha_exp_eq
+  \\ irule_at Any exp_alpha_Alpha
+  \\ fs [] \\ first_assum $ irule_at Any
+  \\ irule_at Any exp_eq_refl \\ fs []
+  \\ irule eq_when_applied_trans
+  \\ irule_at (Pos hd) exp_eq_IMP_eq_when_applied
+  \\ irule_at Any Let_Lam_weak \\ fs []
+  \\ irule eq_when_applied_trans
+  \\ irule_at (Pos last) exp_eq_IMP_eq_when_applied
+  \\ irule_at Any $ iffLR exp_eq_sym
+  \\ irule_at Any exp_eq_App_cong \\ irule_at Any exp_eq_Lam_cong
+  \\ irule_at Any exp_alpha_exp_eq
+  \\ irule_at Any exp_alpha_Alpha
+  \\ first_assum $ irule_at Any
+  \\ irule_at Any exp_eq_refl \\ fs []
+  \\ irule eq_when_applied_trans
+  \\ irule_at (Pos last) exp_eq_IMP_eq_when_applied
+  \\ irule_at Any $ iffLR exp_eq_sym
+  \\ irule_at Any Let_Lam_weak \\ fs []
+  \\ last_x_assum $ irule_at Any
+  \\ rw []
+  \\ irule eq_when_applied_trans \\ irule_at Any eq_when_applied_trans
+  \\ last_x_assum $ irule_at Any
+  \\ rpt $ irule_at Any exp_eq_IMP_eq_when_applied
+  \\ irule_at (Pos $ el 2) $ iffLR exp_eq_sym
+  \\ irule_at (Pos $ el 2) exp_eq_trans \\ irule_at (Pos $ el 3) exp_eq_trans
+  \\ irule_at (Pos $ el 2) Let_Let \\ irule_at (Pos $ el 6) Let_Let
+  \\ rpt $ irule_at Any exp_eq_App_cong
+  \\ rpt $ irule_at Any exp_eq_refl
+  \\ rpt $ irule_at Any exp_eq_Lam_cong
+  \\ rpt $ irule_at Any exp_eq_App_cong
+  \\ rpt $ irule_at Any exp_eq_refl
+  \\ fs [closed_def] \\ conj_tac
+  \\ irule exp_alpha_exp_eq
+  \\ irule exp_alpha_Alpha
+  \\ fs []
+QED
+
+Theorem eq_when_applied_Lams:
+  ∀vl c e e' len. eq_when_applied (FOLDL (λc n. IsFree n c) c vl) e e' len ⇒
+              eq_when_applied c (Lams vl e) (Lams vl e') (len + LENGTH vl)
+Proof
+  Induct
+  \\ rw [Lams_def, GSYM SUC_ADD]
+  \\ irule eq_when_applied_Lam
+  \\ last_x_assum $ irule_at Any
+  \\ fs []
+QED
+
+Theorem exp_eq_in_IsFree_Bind:
+  ∀e1 e2 e3 c v. exp_eq_in_ctxt (IsFree v c) e1 e2 ⇒ exp_eq_in_ctxt (Bind v e3 c) e1 e2
+Proof
+  rpt strip_tac >>
+  gvs [exp_eq_in_ctxt_def, exp_eq_in_ctxt_App, exp_eq_in_ctxt_Lam, exp_eq_in_ctxt_refl]
+QED
+
+Theorem Apps_Seq_in_ctxt:
+  ∀e e2 eL c. exp_eq_in_ctxt c (Apps (Seq e e2) eL) (Seq e (Apps e2 eL))
+Proof
+  rw [exp_eq_IMP_exp_eq_in_ctxt, Apps_Seq]
+QED
+
+Theorem Let_Apps_in_ctxt:
+  ∀v e1 e2 eL c. exp_eq_in_ctxt c (Let v e1 (Apps e2 eL)) (Apps (Let v e1 e2) (MAP (Let v e1) eL))
+Proof
+  rw [Let_Apps, exp_eq_IMP_exp_eq_in_ctxt]
+QED
+
+Theorem Letrec_Apps:
+  ∀l bL b e. (Letrec bL (Apps e l) ≅? Apps (Letrec bL e) (MAP (Letrec bL) l)) b
+Proof
+  Induct >> gvs [exp_eq_refl, Apps_def] >>
+  rpt gen_tac >>
+  irule exp_eq_trans >> pop_assum $ irule_at Any >>
+  irule exp_eq_Apps_cong >>
+  fs [exp_eq_l_refl, Letrec_App]
+QED
+
+Theorem Letrec_Apps_in_ctxt:
+  ∀l b e c. exp_eq_in_ctxt c (Letrec b (Apps e l)) (Apps (Letrec b e) (MAP (Letrec b) l))
+Proof
+  gvs [exp_eq_IMP_exp_eq_in_ctxt, Letrec_Apps]
+QED
+
+Theorem Let_stay:
+  ∀v e b. v ∉ freevars e ⇒ (Let v e (Var v) ≅? Let v e e) b
+Proof
+  rw [] >> irule exp_eq_trans >>
+  irule_at Any Let_Var >>
+  irule eval_IMP_exp_eq >>
+  rw [eval_thm, subst_def, GSYM subst_fdomsub, bind1_def, subst1_ignore,
+      closed_def, IMP_closed_subst, FRANGE_FLOOKUP]
+QED
+
+Theorem concat_rev_ctxt_size:
+  ∀c1 c2. ctxt_size (concat_rev_ctxt c1 c2) = ctxt_size c1 + ctxt_size c2
+Proof
+  Induct >> gvs [ctxt_size_def, concat_rev_ctxt_def]
+QED
+
+Theorem exp_eq_in_ctxt_unfold:
+  ∀c2 w e' c1. not_bound_in_ctxt c2 w
+               ∧ (∀v. v ∈ freevars e' ⇒ not_bound_in_ctxt c2 v) ∧ w ∉ freevars e'
+              ⇒ exp_eq_in_ctxt (Bind w e' c1) (unfold_ctxt c2 (Var w)) (unfold_ctxt c2 e')
+Proof
+  Induct >> rw [not_bound_in_ctxt_def, exp_eq_in_ctxt_def, unfold_ctxt_def]
+  >- gvs [exp_eq_in_ctxt_def, exp_eq_IMP_exp_eq_in_ctxt, Let_stay] >>
+  irule exp_eq_in_ctxt_trans >> irule_at Any exp_eq_in_ctxt_trans >>
+  irule_at (Pos hd) exp_eq_IMP_exp_eq_in_ctxt >> irule_at (Pos last) exp_eq_IMP_exp_eq_in_ctxt >>
+  irule_at (Pos hd) $ iffLR exp_eq_sym
+  >~[‘Letrec’]
+  >- (rpt $ irule_at Any Let_Letrec2 >>
+      gvs [GSYM exp_eq_in_ctxt_def, EVERY_MEM] >>
+      rw [] >> strip_tac >> first_x_assum $ dxrule_then assume_tac >>
+      gvs [])
+  >- (rpt $ irule_at Any Let_Lam_weak >>
+      irule_at Any exp_eq_in_ctxt_Lam >>
+      gvs [GSYM exp_eq_in_ctxt_def] >>
+      strip_tac >> first_x_assum $ dxrule_then assume_tac >> fs [])
+  >- (rpt $ irule_at Any Let_App >> irule exp_eq_in_ctxt_App >> fs [exp_eq_in_ctxt_refl] >>
+      irule exp_eq_in_ctxt_trans >> irule_at Any exp_eq_in_ctxt_trans >>
+      irule_at (Pos hd) exp_eq_IMP_exp_eq_in_ctxt >> irule_at (Pos last) exp_eq_IMP_exp_eq_in_ctxt >>
+      irule_at (Pos hd) $ iffLR exp_eq_sym >>
+      rpt $ irule_at Any Let_Lam_weak >>
+      irule_at Any exp_eq_in_ctxt_Lam >>
+      gvs [GSYM exp_eq_in_ctxt_def] >>
+      strip_tac >> first_x_assum $ dxrule_then assume_tac >> fs [])
+QED
+
+Theorem concat_rev_unfold:
+  ∀c2 c1 e1 e2 len. exp_eq_in_ctxt (concat_rev_ctxt c2 c1) e1 e2
+                    = exp_eq_in_ctxt c1 (unfold_ctxt c2 e1) (unfold_ctxt c2 e2)
+Proof
+  Induct >> gvs [exp_eq_in_ctxt_def, concat_rev_ctxt_def, unfold_ctxt_def] >>
+  rw [] >> eq_tac >> rw []
+  >- (irule exp_eq_in_ctxt_Lam >> gvs [exp_eq_in_ctxt_def])
+  >- gvs [exp_eq_in_ctxt_App, exp_eq_in_ctxt_refl]
+QED
+
+Theorem exp_eq_in_ctxt_concat:
+  ∀c2 w e' c1. not_bound_in_ctxt c2 w ∧
+               (∀v. v ∈ freevars e' ⇒ not_bound_in_ctxt c2 v) ∧ w ∉ freevars e'
+               ⇒ exp_eq_in_ctxt (concat_rev_ctxt c2 (Bind w e' c1)) (Var w) e'
+Proof
+  gvs [exp_eq_in_ctxt_unfold, concat_rev_unfold]
+QED
+
+Theorem exp_eq_concat_rev_still_eq:
+  ∀c_top c_bot e e'.
+    exp_eq_in_ctxt (concat_rev_ctxt c_top Nil) e e'
+      ⇒ exp_eq_in_ctxt (concat_rev_ctxt c_top c_bot) e e'
+Proof
+  Induct >> gvs [concat_ctxt_def, concat_rev_unfold, unfold_ctxt_def, exp_eq_in_ctxt_def] >>
+  rw [exp_eq_IMP_exp_eq_in_ctxt]
+QED
+
+Theorem exp_eq_concat_still_eq:
+  ∀c_top c_bot e e'.
+    exp_eq_in_ctxt c_top e e'
+      ⇒ exp_eq_in_ctxt (concat_ctxt c_top c_bot) e e'
+Proof
+  Induct >> gvs [concat_ctxt_def, exp_eq_IMP_exp_eq_in_ctxt, exp_eq_in_ctxt_def]
+QED
+
+Theorem eq_when_applied_unfold:
+  ∀c2 w e' c1 len. not_bound_in_ctxt c2 w ∧ (∀v. v ∈ freevars e' ⇒ not_bound_in_ctxt c2 v) ∧ w ∉ freevars e'
+              ⇒ eq_when_applied (Bind w e' c1) (unfold_ctxt c2 (Var w)) (unfold_ctxt c2 e') len
+Proof
+  gvs [exp_eq_in_ctxt_IMP_eq_when_applied, exp_eq_in_ctxt_unfold]
+QED
+
+Theorem MAP_FST_no_change:
+  ∀l f. MAP FST l = MAP FST (MAP (λ(v, e). (v, f e)) l)
+Proof
+  Induct >> gvs [FORALL_PROD]
+QED
+
+Theorem ALL_DISTINCT_FST_MAP:
+  ∀l f. ALL_DISTINCT (MAP FST l) ⇒ ALL_DISTINCT (MAP FST (MAP (λ(v,e). (v, f e)) l))
+Proof
+  gvs [GSYM MAP_FST_no_change]
+QED
+
+Theorem fmap_FOLDL_FOLDR:
+  ∀l f f2. ALL_DISTINCT (MAP FST l) ⇒
+           FOLDR (flip $|+) f l = FOLDL $|+ f l
+Proof
+  Induct >> gvs [FORALL_PROD] >> rw [] >>
+  dxrule_then assume_tac FUPDATE_FUPDATE_LIST_COMMUTES >>
+  gvs [FUPDATE_LIST]
+QED
+
+Theorem subst_exp_eq:
+  ∀l1 l2 b e e'.
+    LIST_REL (λ(v1, e1) (v2, e2). v1 = v2 ∧ (e1 ≅? e2) b ∧ closed e1 ∧ closed e2) l1 l2
+    ∧ (e ≅? e') b
+    ⇒ (subst (FEMPTY |++ l1) e ≅? subst (FEMPTY |++ l2) e') b
+Proof
+  Induct using SNOC_INDUCT >> gvs [FUPDATE_LIST, subst_FEMPTY] >> PairCases >>
+  Induct using SNOC_INDUCT >> gvs [] >> PairCases >>
+  gvs [LIST_REL_SNOC, FUPDATE_LIST, FOLDL_SNOC] >>
+  rw [Once subst_subst1_UPDATE] >>
+  irule exp_eq_trans >> last_x_assum $ dxrule_then $ irule_at Any >>
+  irule_at (Pos hd) exp_eq_trans >> dxrule_then (irule_at $ Pos hd) $ iffLR exp_eq_forall_subst >>
+  irule_at Any exp_eq_subst >> first_x_assum $ irule_at (Pos hd) >>
+  gvs [GSYM subst_subst1_UPDATE, exp_eq_refl]
+QED
+
+(*Theorem exp_eq_Letrec_cong3_lemma:
+  ∀bL bL' e e' b.
+    LIST_REL (λ(v1, e1) (v2, e2). ((Letrec bL e1) ≅? (Letrec bL e2)) b) bL bL'
+    ∧ MAP FST bL = MAP FST bL'
+    ∧ EVERY (λe. freevars e ⊆ set (MAP FST bL)) (MAP SND bL)
+    ∧ EVERY (λe. freevars e ⊆ set (MAP FST bL)) (MAP SND bL')
+    ∧ ((Letrec bL e) ≅? (Letrec bL e')) b
+    ∧ ALL_DISTINCT (MAP FST bL)
+    ⇒ ((Letrec bL e) ≅? (Letrec bL' e')) b
+Proof
+  rw [] >>
+  irule exp_eq_trans >> first_x_assum $ irule_at Any >>
+  irule exp_eq_trans >> irule_at Any beta_equality_Letrec >>
+  irule_at Any $ iffLR exp_eq_sym >>
+  irule_at Any exp_eq_trans >> irule_at Any beta_equality_Letrec >>
+  gvs [subst_funs_def, bind_def] >>
+  rename1 ‘MAP FST bL = MAP FST bL2’ >>
+  rpt $ FULL_CASE_TAC >> gvs [exp_eq_refl]
+  >~[‘subst _ _ ≅? subst _ _’]
+  >- (irule subst_exp_eq >>
+      gvs [exp_eq_refl, LIST_REL_EL_EQN, EL_MAP, LIST_REL_eq] >> rw [] >>
+      last_x_assum $ dxrule_then assume_tac >>
+      rename1 ‘EL n _’ >>
+      qabbrev_tac ‘p1 = EL n bL’ >> PairCases_on ‘p1’ >>
+      qabbrev_tac ‘p2 = EL n bL2’ >> PairCases_on ‘p2’ >>
+      ‘∀(l1 : string list) l2. l1 = l2 ⇒ ∀i. i < LENGTH l1 ⇒ EL i l1 = EL i l2’ by gvs [] >>
+      pop_assum $ dxrule_then assume_tac >>
+      gvs [EL_MAP] >> cheat) >>
+  qspecl_then [‘bL’, ‘Letrec bL’] assume_tac ALL_DISTINCT_FST_MAP >>
+  qspecl_then [‘bL2’, ‘Letrec bL2’] assume_tac ALL_DISTINCT_FST_MAP >>
+  gvs [] >>
+  drule_then assume_tac fmap_FOLDL_FOLDR >> dxrule_then assume_tac FLOOKUP_FOLDR_UPDATE >>
+  drule_then assume_tac fmap_FOLDL_FOLDR >> dxrule_then assume_tac FLOOKUP_FOLDR_UPDATE >>
+  rpt $ FULL_CASE_TAC >> gvs [exp_eq_refl, FUPDATE_LIST]
+  >-
+  cheat
+QED*)
+
+(*Theorem exp_eq_test1:
+  ∀vL eL e b.
+    LENGTH vL = LENGTH eL ∧ EVERY (λv. EVERY (λe. v ∉ freevars e) eL) vL ∧ ALL_DISTINCT vL
+    ⇒ (Apps (Lams vL e) eL ≅? Letrec (ZIP (vL, eL)) e) b
+Proof
+  Induct >> gvs [Lams_def, Apps_def]
+  >- (rw [] >> irule eval_wh_IMP_exp_eq >>
+      simp [subst_def, eval_wh_thm, subst_funs_def, FUPDATE_LIST_THM]) >>
+  gen_tac >> Cases >> rw [Apps_def] >>
+  irule $ iffLR exp_eq_sym >> irule exp_eq_trans >> irule_at Any exp_eq_Apps_cong >>
+  gvs [LIST_REL_EL_EQN] >> irule_at Any LENGTH_MAP >> gvs [EL_MAP] >>
+  irule_at (Pos $ el 2) exp_eq_refl >>
+  rename1 ‘(v, e1)::ZIP _’ >> qexists_tac ‘Let v e1’ >>
+  rw [] >> gvs [EL_MAP, EVERY_EL, Let_not_in_freevars] >>
+  first_assum $ irule_at Any >> gvs []
+      irule exp_eq_Tick_cong >>
+      gvs [exp_eq_refl]) >>
+  cheat
+QED
+
+Theorem exp_eq_in_Letrec_test:
+  ∀e e' bL c.
+    exp_eq_in_ctxt c (Lams (MAP FST bL) e) (Lams (MAP FST bL) e')
+    ⇒ exp_eq_in_ctxt c (Letrec bL e) (Letrec bL e')
+Proof
+
+QED*)
+
+(*Theorem exp_eq_in_ctxt_Letrec:
+  ∀e b e1 e2 v c.
+    exp_eq_in_ctxt (RecBind ((v, e1)::b) c) e1 e2
+    ⇒ exp_eq_in_ctxt c (Letrec ((v, e1)::b) e) (Letrec ((v, e2)::b) e)
+Proof
+  Induct using freevars_ind
+  >- (rw [exp_eq_in_ctxt_def] >>
+      irule exp_eq_in_ctxt_trans >> irule_at (Pos hd) exp_eq_IMP_exp_eq_in_ctxt >>
+      rename1 ‘Letrec ((v, _)::_) (Var w)’ >> Cases_on ‘v = w’ >> cheat)
+  >> cheat
+QED*)
+
+(*Theorem exp_eq_in_ctxt_Letrec:
+  ∀c b b' e e'.
+    LIST_REL (λ(v1, e1) (v2, e2). v1 = v2 ∧ exp_eq_in_ctxt c (Letrec b e1) (Letrec b e2)) b b'
+    ∧ exp_eq_in_ctxt c (Letrec b e) (Letrec b e')
+    ⇒ exp_eq_in_ctxt c (Letrec b e) (Letrec b' e')
+Proof
+  Induct >> gvs [exp_eq_in_ctxt_def]
+  >- gvs [exp_eq_Letrec_cong3]
+
+  cheat
+QED*)
+
+(** end ctxt **)
+
+Definition is_bot_def:
+  is_bot e = (e = wh_Diverge ∨ e = wh_Error)
+End
+
+Theorem is_bot_continuous:
+  ∀e k k2. k2 ≤ k ∧ is_bot (eval_wh_to k e) ⇒ is_bot (eval_wh_to k2 e)
+Proof
+  rw [is_bot_def]
+  \\ Cases_on ‘eval_wh_to k2 e = wh_Diverge’
+  \\ fs []
+  \\ qspecl_then [‘k’, ‘e’, ‘k2’] assume_tac eval_wh_inc
+  \\ gvs []
+QED
+
+Definition Projs_def:
+  Projs [] e = e ∧
+  Projs ((x,i)::ps) e = Projs ps (Proj x i e)
+End
+
+Theorem freevars_Projs:
+  ∀ps e. freevars (Projs ps e) = freevars e
+Proof
+  Induct >> gvs [freevars_def, Projs_def, FORALL_PROD]
+QED
+
+Theorem perm_exp_Projs:
+  ∀ps v w e. perm_exp v w (Projs ps e) = Projs ps (perm_exp v w e)
+Proof
+  Induct >> gvs [perm_exp_def, Projs_def, FORALL_PROD]
+QED
+
+Theorem demands_Projs_end:
+  ∀ ps x i e. Projs (ps++[(x,i)]) e = Proj x i (Projs ps e)
+Proof
+  Induct THEN1 rw [Projs_def]
+  \\ gen_tac \\ rename1 ‘hd::ps’
+  \\ PairCases_on ‘hd’
+  \\ rw [Projs_def]
+QED
+
+Theorem double_Projs:
+  ∀ps' ps e. Projs (ps' ++ ps) e = Projs ps (Projs ps' e)
+Proof
+  Induct >- rw [Projs_def]
+  \\ gen_tac \\ rename1 ‘hd::ps'’
+  \\ PairCases_on ‘hd’
+  \\ rw [Projs_def]
 QED
 
 Theorem exp_eq_Projs_cong:
@@ -176,6 +1550,19 @@ Proof
   \\ fs [Let_Prim_alt]
 QED
 
+Theorem Letrec_Projs:
+  ∀ps x bL b. (Letrec bL (Projs ps x) ≅? Projs ps (Letrec bL x)) b
+Proof
+  Induct \\ fs [Projs_def,exp_eq_refl,FORALL_PROD] \\ rw []
+  \\ irule exp_eq_trans
+  \\ qexists_tac ‘Projs ps (Letrec bL (Proj p_1 p_2 x))’
+  \\ conj_tac THEN1 fs []
+  \\ irule exp_eq_Projs_cong
+  \\ irule exp_eq_trans
+  \\ irule_at Any Letrec_Prim
+  \\ gvs [exp_eq_refl]
+QED
+
 Theorem Projs_subst:
   ∀ps f e. subst f (Projs ps e) = Projs ps (subst f e)
 Proof
@@ -189,29 +1576,94 @@ QED
 val _ = set_fixity "demands" (Infixl 480);
 
 Definition demands_def:
-  (e demands (p,v)) = (e ≈ Seq (Projs p (Var v)) e)
+  (e demands ((p,v), c)) = (exp_eq_in_ctxt c e (Seq (Projs p (Var v)) e))
 End
 
 val _ = set_fixity "needs" (Infixl 480);
 Definition needs_def:
-  (e needs (ps, e')) = (e ≈ Seq (Projs ps e') e)
+  (e needs ((ps, e'), c)) = (exp_eq_in_ctxt c e (Seq (Projs ps e') e))
 End
 
+Theorem is_bot_IMP_IMP_needs:
+  ∀e ps e' c. (∀f. is_bot (eval_wh (subst f (Projs ps e'))) ⇒ is_bot (eval_wh (subst f e))) ⇒ e needs ((ps, e'), c)
+Proof
+  rw [needs_def]
+  \\ irule exp_eq_IMP_exp_eq_in_ctxt
+  \\ irule no_err_eval_wh_IMP_exp_eq
+  \\ rw [no_err_eval_wh_def, subst_def, eval_wh_thm]
+  \\ first_x_assum $ qspecl_then [‘f’] assume_tac
+  \\ gvs [is_bot_def]
+QED
+
 Theorem needs_Var_is_demands:
-  e needs (ps, Var v) ⇔ e demands (ps, v)
+  e needs ((ps, Var v), c) ⇔ e demands ((ps, v), c)
 Proof
   rw [needs_def, demands_def] \\ fs []
 QED
 
+Theorem needs_in_IsFree_Bind:
+  e needs (d, IsFree v c) ⇒ e needs (d, Bind v e2 c)
+Proof
+  PairCases_on ‘d’
+  \\ rw [needs_def, exp_eq_in_IsFree_Bind]
+QED
+
+Theorem needs_IsFree_List_lemma:
+  ∀d e c v e'.
+    e needs (d, FOLDL (λc v. IsFree v c) (IsFree v c) l)
+    ⇒ e needs (d, FOLDL (λc v. IsFree v c) (Bind v e' c) l)
+Proof
+  Induct_on ‘LENGTH l’ >> rw [needs_in_IsFree_Bind] >>
+  qspecl_then [‘l’] assume_tac last_exists >>
+  rename1 ‘e needs (d, _)’ >> PairCases_on ‘d’ >>
+  gvs [FOLDL_APPEND, FORALL_PROD, needs_def, exp_eq_in_ctxt_def] >>
+  rpt strip_tac >>
+  irule exp_eq_in_ctxt_trans >> irule_at (Pos last) exp_eq_IMP_exp_eq_in_ctxt >>
+  once_rewrite_tac [exp_eq_sym] >> irule_at Any exp_eq_trans >>
+  irule_at (Pos hd) Let_Seq >>
+  last_x_assum $ irule_at Any >> irule_at Any exp_eq_Prim_cong >>
+  fs [exp_eq_refl] >> irule_at Any Let_Projs >>
+  irule_at Any exp_eq_in_ctxt_trans >>
+  first_x_assum $ irule_at Any >> fs [] >>
+  irule exp_eq_IMP_exp_eq_in_ctxt >>
+  irule exp_eq_trans >> irule_at Any Let_Seq >>
+  gvs [Let_Projs, exp_eq_Prim_cong, exp_eq_refl]
+QED
+
+Theorem needs_IsFree_List:
+  ∀l e c d. e needs (d, FOLDL (λc v. IsFree v c) c (MAP FST l))
+            ⇒ e needs (d, FOLDL (λc (v, e). Bind v e c) c l)
+Proof
+  Induct >> rw [] >>
+  last_x_assum $ irule_at Any >>
+  rename1 ‘IsFree (FST h) c’ >> PairCases_on ‘h’ >>
+  gvs [needs_IsFree_List_lemma]
+QED
+
+Theorem demands_in_IsFree_Bind:
+  e demands (d, IsFree v c) ⇒ e demands (d, Bind v e2 c)
+Proof
+  PairCases_on ‘d’
+  \\ rw [demands_def, exp_eq_in_IsFree_Bind]
+QED
+
+Theorem demands_IsFree_List:
+  ∀d l e c. e demands (d, FOLDL (λc v. IsFree v c) c (MAP FST l))
+            ⇒ e demands (d, FOLDL (λc (v, e). Bind v e c) c l)
+Proof
+  PairCases
+  \\ metis_tac [needs_IsFree_List, needs_Var_is_demands]
+QED
+
 Theorem needs_refl:
-  ∀e. e needs ([],e)
+  ∀e c. e needs (([],e), c)
 Proof
   rw [needs_def, Projs_def]
-  \\ metis_tac [Seq_id, exp_eq_sym]
+  \\ metis_tac [Seq_id, exp_eq_sym, exp_eq_IMP_exp_eq_in_ctxt]
 QED
 
 Theorem needs_Var:
-  (Var v) needs ([], Var v)
+  (Var v) needs (([], Var v), c)
 Proof
   fs [needs_refl]
 QED
@@ -220,21 +1672,21 @@ Theorem needs_Proj:
   e needs d ⇒ (Proj n i e) needs d
 Proof
   PairCases_on ‘d’
-  \\ rename1 ‘(ps, e')’
+  \\ rename1 ‘((ps, e'), _)’
   \\ rw [needs_def, Projs_def]
-  \\ irule exp_eq_trans
+  \\ irule exp_eq_in_ctxt_trans
   \\ qexists_tac ‘Seq e (Proj n i e)’
-  \\ conj_tac >- fs [Proj_Seq]
+  \\ conj_tac >- fs [Proj_Seq, exp_eq_IMP_exp_eq_in_ctxt]
   \\ qabbrev_tac ‘p = Projs ps e'’
-  \\ irule exp_eq_trans
+  \\ irule exp_eq_in_ctxt_trans
   \\ qexists_tac ‘Seq (Seq p e) (Proj n i e)’
   \\ conj_tac
-  >- (irule exp_eq_Prim_cong \\ fs [exp_eq_refl])
-  \\ irule exp_eq_trans
+  >- (irule exp_eq_in_ctxt_Prim \\ fs [exp_eq_in_ctxt_refl])
+  \\ irule exp_eq_in_ctxt_trans
   \\ qexists_tac ‘Seq p (Seq e (Proj n i e))’
-  \\ conj_tac >- fs [Seq_assoc]
-  \\ irule exp_eq_Prim_cong \\ fs [exp_eq_refl, Let_Var]
-  \\ metis_tac [Proj_Seq, exp_eq_sym]
+  \\ conj_tac >- fs [exp_eq_IMP_exp_eq_in_ctxt, Seq_assoc]
+  \\ irule exp_eq_in_ctxt_Prim \\ fs [exp_eq_IMP_exp_eq_in_ctxt, exp_eq_refl, Let_Var]
+  \\ metis_tac [exp_eq_IMP_exp_eq_in_ctxt, Proj_Seq, exp_eq_sym]
 QED
 
 Theorem needs_Projs:
@@ -250,28 +1702,28 @@ Proof
 QED
 
 Theorem needs_trans:
-  e needs (ps,e') ∧ e' needs (ps',e'') ⇒ e needs (ps',e'')
+  e needs ((ps,e'), c) ∧ e' needs ((ps',e''), c) ⇒ e needs ((ps',e''), c)
 Proof
   rw [needs_def]
-  \\ irule exp_eq_trans
+  \\ irule exp_eq_in_ctxt_trans
   \\ first_assum $ irule_at Any
-  \\ irule exp_eq_trans
+  \\ irule exp_eq_in_ctxt_trans
   \\ qexists_tac ‘Seq (Seq (Projs ps' e'') (Projs ps e')) e’
   \\ conj_tac >-
-   (irule exp_eq_Prim_cong \\ fs [exp_eq_refl]
+   (irule exp_eq_in_ctxt_Prim \\ fs [exp_eq_in_ctxt_refl]
     \\ assume_tac needs_Projs \\ metis_tac [needs_def])
-  \\ irule exp_eq_trans
+  \\ irule exp_eq_in_ctxt_trans
   \\ qexists_tac ‘Seq (Projs ps' e'') (Seq (Projs ps e') e)’
-  \\ conj_tac >- fs [Seq_assoc]
-  \\ irule exp_eq_Prim_cong
-  \\ fs [exp_eq_refl, exp_eq_sym]
+  \\ conj_tac >- fs [exp_eq_IMP_exp_eq_in_ctxt, Seq_assoc]
+  \\ irule exp_eq_in_ctxt_Prim
+  \\ fs [exp_eq_in_ctxt_refl, exp_eq_in_ctxt_sym]
 QED
 
 Theorem needs_Projs_Var:
-  (Proj s i (Var v)) needs ([(s,i)], Var v)
+  (Proj s i (Var v)) needs (([(s,i)], Var v), c)
 Proof
   rw [needs_def, Projs_def]
-  \\ metis_tac [Seq_id, exp_eq_sym]
+  \\ metis_tac [exp_eq_IMP_exp_eq_in_ctxt, Seq_id, exp_eq_sym]
 QED
 
 Theorem needs_Seq:
@@ -279,61 +1731,57 @@ Theorem needs_Seq:
 Proof
   PairCases_on ‘d’
   \\ rw [needs_def]
-  \\ irule exp_eq_trans
+  \\ irule exp_eq_in_ctxt_trans
   \\ qexists_tac ‘Seq (Seq (Projs d0 d1) e) e'’
   \\ conj_tac >-
-   (irule exp_eq_Prim_cong \\ fs [exp_eq_refl])
-  \\ fs [Seq_assoc]
+   (irule exp_eq_in_ctxt_Prim \\ fs [exp_eq_in_ctxt_refl])
+  \\ fs [exp_eq_IMP_exp_eq_in_ctxt, Seq_assoc]
 QED
-
 
 Theorem needs_Seq2:
   e' needs d ⇒ (Seq e e') needs d
 Proof
   PairCases_on ‘d’
   \\ rw [needs_def]
-  \\ irule exp_eq_trans
+  \\ irule exp_eq_in_ctxt_trans
   \\ qexists_tac ‘Seq e (Seq (Projs d0 d1) e')’
-  \\ fs [exp_eq_Prim_cong, exp_eq_refl]
-  \\ irule exp_eq_trans
+  \\ fs [exp_eq_in_ctxt_Prim, exp_eq_in_ctxt_refl]
+  \\ irule exp_eq_in_ctxt_trans
+  \\ irule_at (Pos last) exp_eq_IMP_exp_eq_in_ctxt
   \\ irule_at Any Seq_assoc
-  \\ irule exp_eq_trans
+  \\ irule exp_eq_in_ctxt_trans
+  \\ irule_at (Pos last) exp_eq_IMP_exp_eq_in_ctxt
   \\ irule_at Any Seq_comm
-  \\ metis_tac [Seq_assoc, exp_eq_sym]
+  \\ metis_tac [exp_eq_IMP_exp_eq_in_ctxt, Seq_assoc, exp_eq_sym]
 QED
 
 Theorem needs_Let1:
-  e needs d ∧ e' demands ([],w) ⇒ (Let w e e') needs d
+  e needs (d, c) ∧ e' demands (([],w), Bind w e c) ⇒ (Let w e e') needs (d, c)
 Proof
   PairCases_on ‘d’
-  \\ rw [demands_def,needs_def,Projs_def]
-  \\ irule exp_eq_trans
+  \\ rw [demands_def,needs_def,Projs_def, exp_eq_in_ctxt_def]
+  \\ irule exp_eq_in_ctxt_trans
   \\ qabbrev_tac ‘p = (Projs d0 d1)’
-  \\ qexists_tac ‘Let w e (Seq (Var w) e')’
-  \\ conj_tac THEN1
-   (irule exp_eq_App_cong \\ fs [exp_eq_refl]
-    \\ irule exp_eq_Lam_cong \\ fs [exp_eq_refl])
-  \\ irule exp_eq_trans
+  \\ first_assum $ irule_at Any
+  \\ irule exp_eq_in_ctxt_trans
   \\ qexists_tac ‘Seq (Let w e (Var w)) (Let w e e')’
-  \\ conj_tac THEN1 fs [Let_Seq]
-  \\ irule exp_eq_trans
+  \\ conj_tac THEN1 fs [exp_eq_IMP_exp_eq_in_ctxt, Let_Seq]
+  \\ irule exp_eq_in_ctxt_trans
   \\ qexists_tac ‘Seq e (Let w e e')’
   \\ conj_tac
-  THEN1 (irule exp_eq_Prim_cong \\ fs [exp_eq_refl,Let_Var])
-  \\ irule exp_eq_trans
+  THEN1 (irule exp_eq_in_ctxt_Prim \\ fs [exp_eq_IMP_exp_eq_in_ctxt, exp_eq_refl,Let_Var])
+  \\ irule exp_eq_in_ctxt_trans
   \\ qexists_tac ‘Seq (Seq p e) (Let w e e')’
   \\ conj_tac THEN1
-   (irule exp_eq_Prim_cong \\ fs [exp_eq_refl])
-  \\ irule exp_eq_trans
+   (irule exp_eq_in_ctxt_Prim \\ fs [exp_eq_in_ctxt_refl])
+  \\ irule exp_eq_in_ctxt_trans
   \\ qexists_tac ‘Seq p (Seq e (Let w e e'))’
-  \\ conj_tac THEN1 fs [Seq_assoc]
-  \\ irule exp_eq_Prim_cong \\ fs [exp_eq_refl]
-  \\ once_rewrite_tac [exp_eq_sym]
-  \\ irule exp_eq_trans
-  \\ irule_at Any exp_eq_App_cong
-  \\ irule_at Any exp_eq_Lam_cong
-  \\ irule_at (Pos $ el 2) exp_eq_refl
-  \\ first_x_assum $ irule_at Any
+  \\ conj_tac THEN1 fs [exp_eq_IMP_exp_eq_in_ctxt, Seq_assoc]
+  \\ irule exp_eq_in_ctxt_Prim \\ fs [exp_eq_in_ctxt_refl]
+  \\ once_rewrite_tac [exp_eq_in_ctxt_sym]
+  \\ irule exp_eq_in_ctxt_trans
+  \\ first_assum $ irule_at Any
+  \\ irule exp_eq_IMP_exp_eq_in_ctxt
   \\ irule exp_eq_trans
   \\ irule_at Any Let_Seq
   \\ irule exp_eq_Prim_cong
@@ -341,23 +1789,23 @@ Proof
 QED
 
 Theorem needs_Let_Cons: (* expects program to be in ANF *)
-  e demands ((s,LENGTH xs)::ps,w) ⇒
-  (Let w (Cons s (xs ++ e'::ys)) e) needs (ps,e')
+  e demands (((s,LENGTH xs)::ps,w), Bind w (Cons s (xs ++ e' ::ys)) c) ⇒
+  (Let w (Cons s (xs ++ e'::ys)) e) needs ((ps,e'), c)
 Proof
-  rw [demands_def,needs_def,Projs_def]
+  rw [demands_def,needs_def,Projs_def, exp_eq_in_ctxt_def]
   \\ qabbrev_tac ‘cons = (Cons s (xs ++ e'::ys))’
-  \\ irule exp_eq_trans
-  \\ qexists_tac ‘Let w cons (Seq (Projs ps (Proj s (LENGTH xs) (Var w))) e)’
-  \\ conj_tac THEN1
-   (irule exp_eq_App_cong \\ fs [exp_eq_refl]
-    \\ irule exp_eq_Lam_cong \\ fs [exp_eq_refl])
-  \\ irule exp_eq_trans
+  \\ irule exp_eq_in_ctxt_trans
+  \\ last_assum $ irule_at Any
+  \\ irule exp_eq_in_ctxt_trans
+  \\ irule_at (Pos hd) exp_eq_IMP_exp_eq_in_ctxt
   \\ irule_at Any Let_Seq
-  \\ irule exp_eq_Prim_cong \\ fs [exp_eq_refl,Let_Var]
+  \\ irule exp_eq_in_ctxt_Prim \\ fs [exp_eq_IMP_exp_eq_in_ctxt, exp_eq_in_ctxt_refl,Let_Var]
   \\ fs [GSYM Projs_def]
-  \\ irule exp_eq_trans
+  \\ irule exp_eq_in_ctxt_trans
+  \\ irule_at (Pos hd) exp_eq_IMP_exp_eq_in_ctxt
   \\ irule_at Any Let_Projs
   \\ fs [Projs_def]
+  \\ irule exp_eq_IMP_exp_eq_in_ctxt
   \\ irule exp_eq_Projs_cong \\ fs [exp_eq_refl,Let_Var]
   \\ irule exp_eq_trans
   \\ irule_at Any exp_eq_Prim_cong \\ fs [PULL_EXISTS]
@@ -367,20 +1815,18 @@ Proof
 QED
 
 Theorem needs_Let_Proj: (* expects program to be in ANF *)
-  e demands (ps,w) ⇒
-  (Let w (Proj s i e') e) needs ((s,i)::ps,e')
+  e demands ((ps,w), Bind w (Proj s i e') c) ⇒
+  (Let w (Proj s i e') e) needs (((s,i)::ps,e'), c)
 Proof
-  rw [demands_def,needs_def,Projs_def]
-  \\ irule exp_eq_trans
-  \\ qexists_tac ‘Let w (Proj s i e') (Seq (Projs ps (Var w)) e)’
-  \\ conj_tac THEN1
-   (irule exp_eq_App_cong \\ fs [exp_eq_refl]
-    \\ irule exp_eq_Lam_cong \\ fs [exp_eq_refl])
-  \\ irule exp_eq_trans
+  rw [demands_def,needs_def,Projs_def, exp_eq_in_ctxt_def]
+  \\ irule exp_eq_in_ctxt_trans
+  \\ last_assum $ irule_at Any
+  \\ irule exp_eq_in_ctxt_trans
   \\ qexists_tac ‘Seq (Let w (Proj s i e') (Projs ps (Var w)))
                       (Let w (Proj s i e') e)’
-  \\ conj_tac THEN1 fs [Let_Seq]
-  \\ irule exp_eq_Prim_cong \\ fs [exp_eq_refl,Let_Var]
+  \\ conj_tac THEN1 fs [exp_eq_IMP_exp_eq_in_ctxt, Let_Seq]
+  \\ irule exp_eq_in_ctxt_Prim \\ fs [exp_eq_IMP_exp_eq_in_ctxt, exp_eq_refl,Let_Var]
+  \\ irule exp_eq_IMP_exp_eq_in_ctxt
   \\ irule exp_eq_trans
   \\ qexists_tac ‘Projs ps (Let w (Proj s i e') (Var w))’
   \\ conj_tac THEN1 fs [Let_Projs]
@@ -391,14 +1837,14 @@ QED
 Theorem needs_App:
   f needs d ⇒ (App f e) needs d
 Proof
-  PairCases_on ‘d’ \\ rename1 ‘(ps,e')’
+  PairCases_on ‘d’ \\ rename1 ‘((ps,e'), c)’
   \\ rw [needs_def]
   \\ qabbrev_tac ‘proj = Projs ps e'’
-  \\ irule exp_eq_trans
+  \\ irule exp_eq_in_ctxt_trans
   \\ qexists_tac ‘App (Seq proj f) e’
   \\ conj_tac THEN1
-   (irule exp_eq_App_cong \\ rw [exp_eq_refl])
-  \\ fs [Seq_App]
+   (irule exp_eq_in_ctxt_App \\ rw [exp_eq_in_ctxt_refl])
+  \\ fs [exp_eq_IMP_exp_eq_in_ctxt, App_Seq]
 QED
 
 Theorem needs_If:
@@ -406,11 +1852,11 @@ Theorem needs_If:
 Proof
   PairCases_on ‘d’
   \\ rw [needs_def]
-  \\ qabbrev_tac ‘p = Projs d0 d1’
-  \\ irule exp_eq_trans
+  \\ irule exp_eq_in_ctxt_trans
+  \\ irule_at (Pos last) exp_eq_IMP_exp_eq_in_ctxt
   \\ irule_at Any If_Seq
-  \\ irule exp_eq_Prim_cong
-  \\ fs [exp_eq_refl, exp_eq_sym]
+  \\ irule exp_eq_in_ctxt_Prim
+  \\ fs [exp_eq_in_ctxt_refl, exp_eq_in_ctxt_sym]
 QED
 
 Theorem needs_If2:
@@ -418,16 +1864,30 @@ Theorem needs_If2:
 Proof
   PairCases_on ‘d’
   \\ rw [needs_def]
-  \\ irule exp_eq_trans
+  \\ irule exp_eq_in_ctxt_trans
+  \\ irule_at (Pos last) exp_eq_IMP_exp_eq_in_ctxt
   \\ irule_at Any If_Seq2
-  \\ irule exp_eq_Prim_cong
-  \\ fs [exp_eq_refl, exp_eq_sym]
+  \\ irule exp_eq_in_ctxt_Prim
+  \\ fs [exp_eq_in_ctxt_refl, exp_eq_in_ctxt_sym]
+QED
+
+Theorem needs_exp_eq:
+  ∀d c e e'. exp_eq_in_ctxt c e e' ⇒ e needs (d, c) ⇒ e' needs (d, c)
+Proof
+  PairCases
+  \\ rw [needs_def]
+  \\ irule exp_eq_in_ctxt_trans
+  \\ irule_at Any $ iffLR exp_eq_in_ctxt_sym
+  \\ first_assum $ irule_at Any
+  \\ irule exp_eq_in_ctxt_trans
+  \\ pop_assum $ irule_at Any
+  \\ fs [exp_eq_in_ctxt_Prim, exp_eq_in_ctxt_refl]
 QED
 
         (********************************************)
 
 Theorem demands_Var:
-  (Var v) demands ([],v)
+  (Var v) demands (([],v), c)
 Proof
   metis_tac [needs_Var_is_demands, needs_Var]
 QED
@@ -449,10 +1909,10 @@ Proof
 QED
 
 Theorem demands_Proj_Var:
-  (Proj s i (Var v)) demands ([(s,i)],v)
+  (Proj s i (Var v)) demands (([(s,i)],v), c)
 Proof
   rw [demands_def,Projs_def]
-  \\ metis_tac [Seq_id,exp_eq_sym]
+  \\ metis_tac [Seq_id,exp_eq_sym, exp_eq_IMP_exp_eq_in_ctxt]
 QED
 
 Theorem demands_Seq:
@@ -470,29 +1930,27 @@ Proof
 QED
 
 Theorem demands_Let1:
-  e demands d ∧ e' demands ([],w) ⇒ (Let w e e') demands d
+  e demands (d, c) ∧ e' demands (([],w), Bind w e c) ⇒ (Let w e e') demands (d, c)
 Proof
   PairCases_on ‘d’
   \\ metis_tac [needs_def, needs_Var_is_demands, needs_Let1]
 QED
 
 Theorem demands_Let2:
-  e' demands (p,v) ∧ v ≠ w ⇒ (Let w e e') demands (p,v)
+  e' demands ((p,v), Bind w e c) ∧ v ≠ w ⇒ (Let w e e') demands ((p,v), c)
 Proof
-  rw [demands_def,Projs_def]
-  \\ irule exp_eq_trans
-  \\ qexists_tac ‘Let w e (Seq (Projs p (Var v)) e')’
-  \\ conj_tac THEN1
-   (irule exp_eq_App_cong \\ fs [exp_eq_refl]
-    \\ irule exp_eq_Lam_cong \\ fs [exp_eq_refl])
-  \\ irule exp_eq_trans
+  rw [demands_def,Projs_def, exp_eq_in_ctxt_def]
+  \\ irule exp_eq_in_ctxt_trans
+  \\ last_assum $ irule_at Any
+  \\ irule exp_eq_in_ctxt_trans
   \\ qexists_tac ‘Seq (Let w e (Projs p (Var v))) (Let w e e')’
-  \\ conj_tac THEN1 fs [Let_Seq]
-  \\ irule exp_eq_Prim_cong \\ fs [exp_eq_refl,Let_Var]
+  \\ conj_tac THEN1 fs [exp_eq_IMP_exp_eq_in_ctxt, Let_Seq]
+  \\ irule exp_eq_in_ctxt_Prim \\ fs [exp_eq_IMP_exp_eq_in_ctxt, exp_eq_refl,Let_Var]
   \\ qid_spec_tac ‘p’ \\ Induct
-  THEN1 fs [Projs_def,Let_Var2]
+  THEN1 fs [exp_eq_IMP_exp_eq_in_ctxt, Projs_def,Let_Var2]
   \\ fs [FORALL_PROD,Projs_def] \\ rw []
   \\ fs [GSYM Projs_def]
+  \\ irule exp_eq_IMP_exp_eq_in_ctxt
   \\ irule exp_eq_trans
   \\ qexists_tac ‘Projs ((p_1,p_2)::p') (Let w e (Var v))’
   \\ conj_tac THEN1 fs [Let_Projs]
@@ -500,16 +1958,32 @@ Proof
   \\ fs [Let_Var2]
 QED
 
+Theorem demands_Let3:
+  ∀e v h ps c. e demands ((ps, v), Bind v (Var h) c) ⇒ (Let v (Var h) e) demands ((ps, h), c)
+Proof
+  rw [demands_def, exp_eq_in_ctxt_def]
+  \\ irule exp_eq_in_ctxt_trans
+  \\ last_assum $ irule_at Any
+  \\ irule exp_eq_IMP_exp_eq_in_ctxt
+  \\ irule exp_eq_trans
+  \\ irule_at Any Let_Seq
+  \\ irule exp_eq_Prim_cong \\ fs [exp_eq_refl]
+  \\ irule exp_eq_trans
+  \\ irule_at Any Let_Projs
+  \\ irule exp_eq_Projs_cong
+  \\ fs [Let_Var]
+QED
+
 Theorem demands_Let_Proj: (* expects program to be in ANF *)
-  e demands (ps,w) ⇒
-  (Let w (Proj s i (Var v)) e) demands ((s,i)::ps,v)
+  e demands ((ps,w), Bind w (Proj s i (Var v)) c) ⇒
+  (Let w (Proj s i (Var v)) e) demands (((s,i)::ps,v), c)
 Proof
   metis_tac [needs_Let_Proj, needs_Var_is_demands]
 QED
 
 Theorem demands_Let_Cons: (* expects program to be in ANF *)
-  e demands ((s,LENGTH xs)::ps,w) ⇒
-  (Let w (Cons s (xs ++ (Var v)::ys)) e) demands (ps,v)
+  e demands (((s,LENGTH xs)::ps,w), Bind w (Cons s (xs ++ (Var v)::ys)) c) ⇒
+  (Let w (Cons s (xs ++ (Var v)::ys)) e) demands ((ps,v), c)
 Proof
   metis_tac [needs_Let_Cons, needs_Var_is_demands]
 QED
@@ -535,10 +2009,16 @@ Proof
   \\ metis_tac [needs_If2, needs_Var_is_demands]
 QED
 
+Theorem demands_concat:
+  ∀c1 c2 d e. e demands (d, c1) ⇒ e demands (d, concat_ctxt c1 c2)
+Proof
+  gvs [FORALL_PROD, demands_def, exp_eq_concat_still_eq]
+QED
+
 Definition well_formed_def:
   well_formed (Cons s) l = (s ≠ s) ∧
   well_formed (Proj s i) l = (∃ e. l = [e]) ∧
-  well_formed (IsEq s i) l = (∃e. l = [e]) ∧
+  well_formed (IsEq s i b) l = (∃e. l = [e]) ∧
   well_formed If (l: exp list) = (∃e e' e''. l = e::e'::e''::[]) ∧
   well_formed Seq l = (∃e e'. l = e::e'::[]) ∧
   well_formed (AtomOp op) l = (op ≠ op)
@@ -550,166 +2030,79 @@ Proof
   PairCases_on ‘d’
   \\ rw [demands_def]
   \\ qabbrev_tac ‘p = Projs d0 (Var d1)’
-  \\ irule exp_eq_trans \\ qexists_tac ‘Prim ope ((Seq p e)::l)’
+  \\ irule exp_eq_in_ctxt_trans \\ qexists_tac ‘Prim ope ((Seq p e)::l)’
   \\ conj_tac
-  >- (irule exp_eq_Prim_cong \\ fs [exp_eq_l_refl])
+  >- (irule exp_eq_in_ctxt_Prim
+      \\ gvs [exp_eq_in_ctxt_refl, LIST_REL_EL_EQN])
   \\ Cases_on ‘ope’ \\ fs [well_formed_def]
+  \\ irule exp_eq_IMP_exp_eq_in_ctxt
   \\ fs [If_Seq, IsEq_Seq, Proj_Seq2, Seq_assoc]
 QED
 
 Theorem demands_IsEq:
-  e demands d ⇒ (IsEq n i e) demands d
+  e demands d ⇒ (IsEq n i b e) demands d
 Proof
   strip_tac
   \\ irule demands_Prim
   \\ fs [well_formed_def]
 QED
 
-(*
-Definition is_good_def:
-  is_good e = (eval_wh e ≠ wh_Error ∧ eval_wh e ≠ wh_Diverge ∧ closed e)
-End
-
-
-Definition can_commute_def:
-  can_commute  e e' = ∀f.
-                           ¬ (eval_wh (subst f e) = wh_Diverge ∧ eval_wh (subst f e') = wh_Error) ∧
-                           ¬ (eval_wh (subst f e) = wh_Error ∧ eval_wh (subst f e') = wh_Diverge)
-End
-
-Theorem can_commute_sym:
-  can_commute e e' ⇒ can_commute e' e
+Theorem demands_Letrec:
+  ∀d b e c. e demands (d, RecBind b c) ∧ ¬MEM (SND d) (MAP FST b) ⇒ Letrec b e demands (d, c)
 Proof
-  metis_tac [can_commute_def]
+  PairCases >> rw [demands_def, exp_eq_in_ctxt_def] >>
+  irule exp_eq_in_ctxt_trans >> last_x_assum $ irule_at Any >>
+  irule exp_eq_IMP_exp_eq_in_ctxt >> irule exp_eq_trans >>
+  irule_at Any Letrec_Prim >> irule exp_eq_Prim_cong >>
+  gvs [exp_eq_refl] >>
+  irule Letrec_not_in_freevars >>
+  gvs [freevars_Projs, EVERY_MEM]
 QED
 
-Theorem can_commute_Seq_com:
-  ∀e e'. can_commute e e' ⇒ ∀e''. Seq (Seq e e') e'' ≈ Seq (Seq e' e) e''
-Proof
-  rw [can_commute_def]
-  \\ irule eval_wh_IMP_exp_eq
-  \\ gen_tac
-  \\ ‘eval_wh (subst f e) = wh_Diverge ∨ eval_wh (subst f e) = wh_Error ∨ (eval_wh (subst f e) ≠ wh_Diverge ∧ eval_wh (subst f e) ≠ wh_Error)’ by rw [DISJ_EQ_IMP]
-  \\ ‘eval_wh (subst f e') = wh_Diverge ∨ eval_wh (subst f e') = wh_Error ∨ (eval_wh (subst f e') ≠ wh_Diverge ∧ eval_wh (subst f e') ≠ wh_Error)’ by rw [DISJ_EQ_IMP]
-  \\ rw [subst_def, eval_wh_Seq]
-  \\ fs []
-  \\ metis_tac []
-QED
-
-Theorem is_good_means_can_commute:
-  ∀e e'. is_good e ⇒ can_commute e e'
-Proof
-  fs [is_good_def, can_commute_def]
-QED
-
-Theorem demands_Seq_com:
-  ∀e e'. is_good e ∨ is_good e' ⇒ ∀e''. Seq (Seq e e') e'' ∼ Seq (Seq e' e) e''
-Proof
-  rw [is_good_means_can_commute]
-  \\ irule can_commute_Seq_com
-  \\ fs [is_good_means_can_commute, can_commute_sym]
-QED
-
-Theorem needs_Seq2:
-  (can_commute e (Projs ps e'')) ∧ e' needs (ps, e'')
-  ⇒ (Seq e e') needs (ps, e'')
-Proof
-  rw [DISJ_EQ_IMP]
-  \\ fs [needs_def, Projs_def]
-  \\ qabbrev_tac ‘p = Projs ps e''’
-  \\ irule exp_eq_trans \\ qexists_tac ‘Seq e (Seq p e')’
-  \\ conj_tac
-  >- (irule exp_eq_Prim_cong \\ fs [exp_eq_refl])
-  \\ irule exp_eq_trans \\ qexists_tac ‘Seq (Seq e p) e'’
-  \\ conj_tac
-  >- (‘Seq (Seq e p) e' ∼ Seq e (Seq p e')’ by fs [Seq_assoc]
-      \\ fs [exp_eq_sym])
-  \\ irule exp_eq_trans \\ qexists_tac ‘Seq (Seq p e) e'’
-  \\ fs [Seq_assoc]
-  \\ irule can_commute_Seq_com
-  \\ fs [DISJ_EQ_IMP]
-QED
-
-Theorem demands_Seq2:
-  is_good e ∧ e' demands (ps, v)
-   ⇒ (Seq e e') demands (ps, v)
-Proof
-  metis_tac [is_good_means_can_commute,needs_Var_is_demands, needs_Seq2]
-QED
-
-Theorem needs_If2_no_Diverge:
-  (∀f. eval_wh (subst f ce) ≠ wh_Diverge ∧ eval_wh (subst f e) ≠ wh_Diverge)
-  ∧ te ∼ Seq e te' ∧ ee ∼ Seq e ee'
-  ⇒ If ce te ee ∼ Seq e (If ce te' ee')
-Proof
-  rw []
-  \\ irule exp_eq_trans
-  \\ qexists_tac ‘If ce (Seq e te') (Seq e ee')’
-  \\ conj_tac
-  >- (irule exp_eq_Prim_cong \\ fs [exp_eq_refl])
-  \\ irule eval_wh_IMP_expeq
-  \\ rw [subst_def, eval_wh_Seq, eval_wh_If]
-  \\ fs []
-QED
-
-Theorem needs_If2:
-  ((is_good ce ∧ (eval_wh ce = wh_True ∨ eval_wh ce = wh_False)) ∨ is_good e') ∧ te needs ([], e') ∧ ee needs ([], e') ⇒ (If ce te ee) needs ([], e')
-Proof
-  rw [is_good_def, needs_def, Projs_def]
-  \\ irule exp_eq_trans
-  \\ qexists_tac ‘If ce (Seq e' te) (Seq e' ee)’
-  \\ conj_tac
-  \\ TRY (irule exp_eq_Prim_cong \\ fs [exp_eq_refl])
-  \\ irule eval_wh_IMP_exp_eq
-  \\ rw [subst_def, eval_wh_Seq, eval_wh_If]
-  \\ fs []
-QED
-*)
-
-Theorem needs_projs_reduce:
-  ∀ps ps' e e'. e needs (ps ++ ps', e') ⇒ e needs (ps, e')
+Theorem needs_Projs_reduce:
+  ∀ps ps' e e' c. e needs ((ps ++ ps', e'), c) ⇒ e needs ((ps, e'), c)
 Proof
   rw [needs_def, double_Projs]
   \\ qabbrev_tac ‘p = Projs ps e'’
-  \\ irule exp_eq_trans \\ qexists_tac ‘Seq (Seq p (Projs ps' p)) e’
+  \\ irule exp_eq_in_ctxt_trans \\ qexists_tac ‘Seq (Seq p (Projs ps' p)) e’
   \\ conj_tac
-  >- (irule exp_eq_trans \\ first_assum $ irule_at Any
-      \\ irule exp_eq_Prim_cong
-      \\ fs [exp_eq_refl]
-      \\ ‘p needs ([], p)’ by fs [needs_refl]
+  >- (irule exp_eq_in_ctxt_trans \\ first_assum $ irule_at Any
+      \\ irule exp_eq_in_ctxt_Prim
+      \\ fs [exp_eq_in_ctxt_refl]
+      \\ ‘p needs (([], p), c)’ by fs [needs_refl]
       \\ drule needs_Projs
       \\ rw [needs_def, Projs_def])
-  \\ irule exp_eq_trans \\ qexists_tac ‘Seq p (Seq (Projs ps' p) e)’
-  \\ fs [Seq_assoc]
-  \\ irule exp_eq_Prim_cong
-  \\ fs [exp_eq_refl, exp_eq_sym]
+  \\ irule exp_eq_in_ctxt_trans \\ qexists_tac ‘Seq p (Seq (Projs ps' p) e)’
+  \\ fs [exp_eq_IMP_exp_eq_in_ctxt, Seq_assoc]
+  \\ irule exp_eq_in_ctxt_Prim
+  \\ fs [exp_eq_in_ctxt_refl, exp_eq_in_ctxt_sym]
 QED
 
-
 Theorem demands_Projs_empty:
-  ∀ps v. (Projs ps (Var v)) demands ([], v)
+  ∀ps v c. (Projs ps (Var v)) demands (([], v), c)
 Proof
   rpt gen_tac
-  \\ ‘(Projs ps (Var v)) demands (ps, v)’ by metis_tac [Projs_def, demands_def, Seq_id, exp_eq_sym]
+  \\ ‘(Projs ps (Var v)) demands ((ps, v), c)’
+    by metis_tac [exp_eq_IMP_exp_eq_in_ctxt, Projs_def, demands_def, Seq_id, exp_eq_sym]
   \\ irule $ iffLR needs_Var_is_demands
-  \\ irule needs_projs_reduce
+  \\ irule needs_Projs_reduce
   \\ fs []
   \\ rw [needs_Var_is_demands]
   \\ first_assum $ irule_at Any
 QED
 
-Theorem demands_empty_proj:
-  e demands (ps, v) ⇒ e demands ([], v)
+Theorem demands_empty_Projs:
+  e demands ((ps, v), c) ⇒ e demands (([], v), c)
 Proof
   ‘ps = [] ++ ps’ by rw []
   \\ rw []
-  \\ metis_tac [needs_projs_reduce, needs_Var_is_demands]
+  \\ metis_tac [needs_Projs_reduce, needs_Var_is_demands]
 QED
 
-Theorem demands_projs_reduce:
-  e demands (ps ++ ps', v) ⇒ e demands (ps, v)
+Theorem demands_Projs_reduce:
+  e demands ((ps ++ ps', v), c) ⇒ e demands ((ps, v), c)
 Proof
-  metis_tac [needs_projs_reduce, needs_Var_is_demands]
+  metis_tac [needs_Projs_reduce, needs_Var_is_demands]
 QED
 
 Theorem EXISTS_EL:
@@ -733,16 +2126,16 @@ Proof
   gen_tac
   \\ PairCases_on ‘d’
   \\ rw [eval_wh_def, eval_wh_to_def, demands_def]
-  \\ irule exp_eq_trans
-  \\ irule_at Any exp_eq_Prim_cong
+  \\ irule exp_eq_in_ctxt_trans
+  \\ irule_at Any exp_eq_in_ctxt_Prim
   \\ drule EXISTS_EL
   \\ rw []
-  \\ rename1 ‘EL n l ≈ Seq p _’
+  \\ rename1 ‘exp_eq_in_ctxt c (EL n l) (Seq p _)’
   \\ qexists_tac ‘LUPDATE (Seq p (EL n l)) n l’
-(*  \\ qexists_tac ‘GENLIST (λ i. if i = n then Seq p (EL i l) else EL i l) (LENGTH l)’ *)
   \\ rw [LIST_REL_EL_EQN, EL_LUPDATE]
   >- (IF_CASES_TAC
-      \\ fs [exp_eq_refl])
+      \\ fs [exp_eq_in_ctxt_refl])
+  \\ irule exp_eq_IMP_exp_eq_in_ctxt
   \\ irule no_err_eval_wh_IMP_exp_eq
   \\ rw [no_err_eval_wh_def, subst_def, eval_wh_Prim_alt, MAP_MAP_o]
   \\ qabbrev_tac ‘l2 = LUPDATE (Seq p (EL n l)) n l’
@@ -821,95 +2214,6 @@ Proof
       \\ rw [LENGTH_MAP, LENGTH_LUPDATE, EL_MAP, EL_LUPDATE, eval_wh_Seq, subst_def])
 QED
 
-(*
-Definition fun_demands2_def:
-  f fun_demands (ps,(k:num),(n:num)) ⇒ ∀l hd v. LENGTH l = n ∧ LENGTH hd = k ∧ (l = hd++v::tl) ⇒ Apps f (MAP Var l) demands ([],v)
-End
-*)
-Definition fun_demands_pre_def:
-  fun_demands_pre (k:num) f ps = if k = 0
-                        then ∀n. n ∉ freevars f ⇒ (App f (Var n)) demands (ps, n)
-                        else ∀e. fun_demands_pre (k - 1) (App f e) ps
-End
-
-val _ = set_fixity "fun_demands" (Infixl 478);
-
-Definition fun_demands_def:
-  f fun_demands (ps, k) = fun_demands_pre k f ps
-End
-(*
-Theorem Let_Var_eq:
-  ∀e v. Let v (Var v) e ∼ e
-Proof
-  Induct \\ rw []
-  THEN1 (qsuff_tac ‘v = s ∨ v ≠ s’
-         THEN1 (DISCH_TAC \\ pop_assum DISJ_CASES_TAC
-                THEN1 (rw [] \\ fs [Let_Var])
-                \\ fs [Let_Var2])
-         \\ rw [])
-  THEN1 (irule exp_eq_trans \\ qexists_tac ‘Prim o' (MAP (Let v (Var v)) l)’
-         \\ conj_tac
-         THEN1 fs [Let_Prim]
-QED
-*)
-(*
-Theorem fun_demands_Lam:
-  e demands (ps, v) ⇒ (Lam v e) fun_demands (ps, 0)
-Proof
-  rw [fun_demands_def, fun_demands_pre_def, demands_def]
-  \\ irule exp_eq_trans
-  THEN1 (qexists_tac ‘Let v (Var n) (Seq (Projs ps (Var v)) e)’
-         \\ conj_tac
-         THEN1 (irule exp_eq_App_cong \\ fs [exp_eq_refl]
-                \\ irule exp_eq_Lam_cong \\ fs [])
-         \\ irule exp_eq_trans \\ qexists_tac ‘Seq (Let v (Var n) (Projs ps (Var v))) (Let v (Var n) e)’
-         \\ conj_tac
-         THEN1 fs [Let_Seq]
-         \\ irule exp_eq_Prim_cong
-         \\ fs [exp_eq_refl]
-         \\ irule exp_eq_trans \\ qexists_tac ‘Projs ps (Let v (Var n) (Var v))’
-         \\ conj_tac
-         THEN1 fs [Let_Projs]
-         \\ irule exp_eq_Projs_cong \\ fs [Let_Var])
-  \\ qexists_tac ‘e’ \\ conj_tac
-  THEN1 fs [Let_Var_eq]
-  \\ irule exp_eq_trans \\ qexists_tac ‘Seq (Projs ps (Var n)) e’
-  THEN1 fs []
-  \\ irule exp_eq_Prim_cong \\ fs [exp_eq_refl]
-QED
-
-Theorem fun_demands_Let:
-  ∀f. (f fun_demands (ps, k) ⇒ ∀e v. (App (Lam v f) e) fun_demands (ps, k))
-Proof
-  rw [fun_demands_def, Once fun_demands_pre_def, demands_def]
-  THEN1 (rw [fun_demands_pre_def]
-   \\ rw [demands_def]
-   \\ irule exp_eq_trans \\ qexists_tac ‘Let v e (App f (Var n))’
-   \\ conj_tac
-   THEN1 (irule exp_eq_trans \\ qexists_tac ‘App (Let v e f) (Let v e (Var n))’
-    \\ conj_tac
-    THEN1 (irule exp_eq_App_cong \\ fs [exp_eq_refl])
-*)
-
-Theorem exp_eq_Apps_cong:
-  ∀l l' b e e'. LIST_REL (λx y. (x ≅? y) b) l l' ⇒ (e ≅? e') b ⇒ (Apps e l ≅? Apps e' l') b
-Proof
-  Induct
-  \\ fs [Apps_def]
-  \\ rw [Apps_def]
-  \\ fs [Apps_def]
-  \\ first_x_assum $ irule
-  \\ fs [exp_eq_App_cong]
-QED
-
-Theorem exp_eq_Lams_cong:
-  ∀l e e' b. (e ≅? e') b ⇒ (Lams l e ≅? Lams l e') b
-Proof
-  Induct
-  \\ rw [Lams_def]
-  \\ fs [exp_eq_Lam_cong]
-QED
-
 Theorem Apps_demands:
   ∀el d e. e demands d ⇒ Apps e el demands d
 Proof
@@ -921,171 +2225,2021 @@ Proof
   \\ fs [demands_App]
 QED
 
-Datatype:
-  ctxt = Nil
-       | IsFree string ctxt
-       | Bind string exp ctxt ctxt
-       | RecBind ((string # exp) list) ctxt
+Theorem demands_exp_eq:
+  ∀d c e e'. exp_eq_in_ctxt c e e' ⇒ e demands (d, c) ⇒ e' demands (d, c)
+Proof
+  PairCases
+  \\ metis_tac [needs_exp_eq, needs_Var_is_demands]
+QED
+
+Theorem Letrec_unfold:
+  ∀lcs i b. i < LENGTH lcs ∧ ALL_DISTINCT (MAP FST lcs)
+            ⇒ (Letrec lcs (Var (FST (EL i lcs))) ≅? Letrec lcs (SND (EL i lcs))) b
+Proof
+  rw [] >> irule eval_IMP_exp_eq >>
+  rw [subst_def, eval_thm, subst_funs_def, MAP_MAP_o, combinTheory.o_DEF, LAMBDA_PROD, bind_def,
+      FLOOKUP_DRESTRICT, FDIFF_def]
+  >- (gvs [MEM_EL] >> rename1 ‘i < LENGTH _’ >>
+      first_x_assum $ qspecl_then [‘i’] assume_tac >> gvs [EL_MAP]) >>
+  rename1 ‘FLOOKUP _ (FST (EL i lcs))’ >> rename1 ‘DRESTRICT f _’ >>
+  qabbrev_tac ‘bind_fun = λp2.
+                            Letrec (MAP  (λ(f',e). (f', subst (DRESTRICT f (COMPL (set (MAP FST lcs)))) e)) lcs)
+                                   (subst (DRESTRICT f (COMPL (set (MAP FST lcs)))) p2)’ >>
+  qspecl_then [‘lcs’, ‘bind_fun’] assume_tac ALL_DISTINCT_FST_MAP >> gvs [] >>
+  drule_then assume_tac fmap_FOLDL_FOLDR >>
+  pop_assum $ qspecl_then [‘FEMPTY’] assume_tac >>
+  drule_then assume_tac $ iffRL FLOOKUP_FOLDR_UPDATE >>
+  pop_assum $ qspecl_then [‘bind_fun (SND (EL i lcs))’, ‘FST (EL i lcs)’, ‘FEMPTY’] assume_tac >>
+  gvs [FUPDATE_LIST, DISJOINT_EMPTY, FDOM_FEMPTY, MEM_EL, PAIR] >>
+  FULL_CASE_TAC >> unabbrev_all_tac >> gvs [] >>
+  rename1 ‘FST (EL i lcs) = EL n (MAP FST lcs)’ >>
+  qspecl_then [‘MAP FST lcs’, ‘n’, ‘i’] assume_tac ALL_DISTINCT_EL_IMP >>
+  gvs [EL_MAP, PULL_EXISTS] >> rename1 ‘EL i _’ >>
+  first_x_assum $ qspecl_then [‘i’] assume_tac >> gvs [EL_MAP] >>
+  qabbrev_tac ‘pair = EL i lcs’ >> PairCases_on ‘pair’ >> gvs [eval_thm, subst_funs_def, bind_def] >>
+  gvs [FUPDATE_LIST, MAP_MAP_o, combinTheory.o_DEF, LAMBDA_PROD] >>
+  rw [] >> gvs []
+QED
+
+Theorem demands_Letrec2:
+  ∀bL ps i e v c. ALL_DISTINCT (MAP FST bL) ∧ i < LENGTH bL
+                  ∧ e demands (([], FST (EL i bL)), RecBind bL c)
+                  ∧ (SND (EL i bL)) demands ((ps, v), Nil)
+                  ∧ ¬MEM v (MAP FST bL)
+                  ⇒ Letrec bL e demands ((ps, v), c)
+Proof
+  rw [demands_def, exp_eq_in_ctxt_def, Projs_def] >>
+  irule exp_eq_in_ctxt_trans >> first_assum $ irule_at Any >>
+  irule exp_eq_in_ctxt_trans >> irule_at (Pos hd) exp_eq_IMP_exp_eq_in_ctxt >> irule_at Any Letrec_Prim >>
+  irule exp_eq_in_ctxt_trans >> irule_at (Pos last) exp_eq_in_ctxt_Prim >> gvs [] >>
+  irule_at (Pos $ el 2) exp_eq_in_ctxt_refl >>
+  irule_at (Pos $ el 3) $ iffLR exp_eq_in_ctxt_sym >> first_x_assum $ irule_at Any >> gvs [] >>
+  irule exp_eq_in_ctxt_trans >> irule_at (Pos last) exp_eq_IMP_exp_eq_in_ctxt >>
+  irule_at Any exp_eq_Prim_cong >> gvs [] >>
+  irule_at (Pos $ el 2) exp_eq_refl >>
+  irule_at (Pos $ el 3) $ iffLR exp_eq_sym >> irule_at Any Letrec_Prim >> gvs [] >>
+  irule exp_eq_in_ctxt_trans >> irule_at (Pos last) exp_eq_IMP_exp_eq_in_ctxt >>
+  irule_at Any Seq_assoc >>
+  irule exp_eq_in_ctxt_Prim >> gvs [exp_eq_in_ctxt_refl] >>
+  irule exp_eq_in_ctxt_trans >> irule_at (Pos hd) exp_eq_IMP_exp_eq_in_ctxt >>
+  irule_at Any Letrec_unfold >> gvs [] >>
+  irule exp_eq_IMP_exp_eq_in_ctxt >>
+  irule exp_eq_trans >> irule_at Any exp_eq_Letrec_cong >> first_x_assum $ irule_at Any >>
+  irule_at Any exp_eq_l_refl >> gvs [] >>
+  irule exp_eq_trans >> irule_at Any Letrec_Prim >>
+  irule exp_eq_Prim_cong >> gvs [] >>
+  irule_at Any Letrec_not_in_freevars >> gvs [freevars_Projs, EVERY_MEM, Once exp_eq_sym, Letrec_unfold]
+QED
+
+Theorem last_Lams:
+  ∀l x e. Lams (l ++ [x]) e = Lams l (Lam x e)
+Proof
+  Induct
+  \\ fs [Lams_def]
+QED
+
+val _ = set_fixity "fdemands" (Infixl 480);
+
+Definition nb_free_def:
+  nb_free Nil = 0 ∧
+  nb_free (IsFree v c) = SUC (nb_free c) ∧
+  nb_free (Bind v e c) = nb_free c ∧
+  nb_free (RecBind b c) = nb_free c
 End
 
-Definition ctxt_size_def:
-  ctxt_size Nil = 0n ∧
-  ctxt_size (IsFree s ctxt) = 1 + ctxt_size ctxt ∧
-  ctxt_size (Bind s e ctxt tl) = 1 + list_size char_size s +  exp_size e + ctxt_size ctxt + ctxt_size tl ∧
-  ctxt_size (RecBind sel ctxt) = 1 + exp1_size sel + ctxt_size ctxt
+Definition fdemands_def:
+  f fdemands ((ps, i), len, Nil) = (i < len ∧ (∀l. LENGTH l = len
+                                             ⇒ Apps f l needs ((ps, EL i l), Nil))) ∧
+  f fdemands (p, len, Bind v e c) = (Let v e f) fdemands (p, len, c) ∧
+  f fdemands (p, len, RecBind b c) = (Letrec b f) fdemands (p, len, c) ∧
+  f fdemands (p, len, IsFree v c) = ∀e. closed e ⇒ (Let v e f) fdemands (p, len, c)
 End
 
-Definition subst_ctxt_def:
-  (subst_ctxt ctxt (App f e) = App (subst_ctxt ctxt f) (subst_ctxt ctxt e)) ∧
-  (subst_ctxt  ctxt (Prim op l) = Prim op (MAP (subst_ctxt ctxt) l)) ∧
-  (subst_ctxt ctxt (Lam v e) = Lam v (subst_ctxt (IsFree v ctxt) e)) ∧
-  (subst_ctxt Nil (Var n) = Var n) ∧
-  (subst_ctxt (IsFree v ctxt) (Var n) = if n = v
-                                        then Var n
-                                        else subst_ctxt ctxt (Var n)) ∧
-  (subst_ctxt (Bind v exp ctxt tl) (Var n) = if n = v
-                                         then subst_ctxt ctxt exp
-                                         else subst_ctxt tl (Var n)) ∧
-  (subst_ctxt (RecBind nel ctxt) (Var n) = if MEM n (MAP FST nel)
-                                                then Var n
-                                                else subst_ctxt ctxt (Var n)) ∧
-  (subst_ctxt ctxt (Letrec nel e) = Letrec nel (subst_ctxt (RecBind nel ctxt) e))
-Termination
-  WF_REL_TAC ‘inv_image ($< LEX $<) (λ(c,e).(exp_size e + ctxt_size c, exp_size e))’
-  \\ rw [ctxt_size_def] \\ fs []
+Theorem fdemands_alt:
+  ∀(c : ctxt) f ps i len. f fdemands ((ps, i), len, c) ⇒ i < len ∧ ∀l. LENGTH l = len ⇒ (Apps f l) needs ((ps, EL i l), c)
+Proof
+  Induct >> gvs [fdemands_def] >> rpt gen_tac >> strip_tac
+  >~[‘IsFree’]
+  >- (rw [needs_def, exp_eq_in_ctxt_def]
+      >- (pop_assum $ qspecl_then [‘Fail’] assume_tac >>
+          gvs [closed_def] >>
+          last_x_assum $ dxrule_then assume_tac >> fs []) >>
+      first_x_assum $ dxrule_then assume_tac >>
+      gvs [needs_def] >>
+      irule exp_eq_in_ctxt_trans >> irule_at Any Let_Apps_in_ctxt >>
+      irule exp_eq_in_ctxt_trans >> last_x_assum $ dxrule_then assume_tac >>
+      fs [] >> first_x_assum $ irule_at Any >> fs [EL_MAP] >>
+      irule exp_eq_IMP_exp_eq_in_ctxt >> irule $ iffLR exp_eq_sym >>
+      irule exp_eq_trans >> irule_at Any Let_Seq >>
+      gvs [Let_Projs, exp_eq_Prim_cong, Let_Apps])
+  >~[‘Bind’]
+  >- (last_x_assum $ dxrule_then assume_tac >> fs [needs_def, exp_eq_in_ctxt_def] >> rw [] >>
+      irule exp_eq_in_ctxt_trans >> irule_at Any Let_Apps_in_ctxt >>
+      irule_at Any exp_eq_in_ctxt_trans >> first_x_assum $ irule_at Any >> fs [EL_MAP] >>
+      irule exp_eq_IMP_exp_eq_in_ctxt >> irule $ iffLR exp_eq_sym >>
+      irule exp_eq_trans >> irule_at Any Let_Seq >>
+      gvs [Let_Projs, exp_eq_Prim_cong, Let_Apps]) >>
+  last_x_assum $ dxrule_then assume_tac >> fs [needs_def, exp_eq_in_ctxt_def] >> rw [] >>
+  irule exp_eq_in_ctxt_trans >> irule_at Any Letrec_Apps_in_ctxt >>
+  irule_at Any exp_eq_in_ctxt_trans >> first_x_assum $ irule_at Any >> fs [EL_MAP] >>
+  irule exp_eq_IMP_exp_eq_in_ctxt >> irule $ iffLR exp_eq_sym >>
+  irule exp_eq_trans >> irule_at Any Letrec_Prim >>
+  gvs [Letrec_Projs, exp_eq_Prim_cong, Letrec_Apps]
+QED
+
+Theorem fdemands_eq_w_app:
+  ∀c p f f' len. eq_when_applied c f f' len ∧ f fdemands (p, len, c) ⇒ f' fdemands (p, len, c)
+Proof
+  Induct
+  >- (PairCases >> rw [fdemands_def, eq_when_applied_def] >>
+      irule needs_exp_eq >> pop_assum $ irule_at Any >>
+      gvs [exp_eq_IMP_exp_eq_in_ctxt])
+  >~[‘IsFree’]
+  >- (rw [fdemands_def] >> last_x_assum irule >>
+      first_x_assum $ irule_at Any >> irule_at Any eq_when_applied_App >>
+      irule_at Any exp_eq_in_ctxt_refl >> irule_at Any eq_when_applied_Lam >>
+      fs []) >>
+  rw [fdemands_def, eq_when_applied_def] >> last_x_assum irule >>
+  rpt $ pop_assum $ irule_at Any
+QED
+
+Theorem fdemands_exp_eq:
+  ∀c p f f' len. exp_eq_in_ctxt c f f' ∧ f fdemands (p, len, c) ⇒ f' fdemands (p, len, c)
+Proof
+  rw [eq_when_applied_0] >>
+  irule fdemands_eq_w_app >>
+  first_assum $ irule_at Any >>
+  irule eq_when_applied_bigger >>
+  first_x_assum $ irule_at Any >> fs []
+QED
+
+Theorem fdemands_Seq:
+  ∀c p len e1 e2. e2 fdemands (p, len, c) ⇒ (Seq e1 e2) fdemands (p, len, c)
+Proof
+  Induct
+  >- (PairCases >> rw [fdemands_def] >>
+      irule needs_exp_eq >> irule_at Any needs_Seq2 >> pop_assum $ irule_at Any >>
+      irule_at Any exp_eq_IMP_exp_eq_in_ctxt >>
+      gvs [Once exp_eq_sym] >> irule_at Any Apps_Seq) >>
+  rw [fdemands_def] >>
+  irule fdemands_exp_eq >> last_x_assum $ irule_at Any >>
+  first_x_assum $ irule_at Any >>
+  once_rewrite_tac [exp_eq_in_ctxt_sym]
+  >~[‘Letrec’]
+  >- (irule_at Any exp_eq_IMP_exp_eq_in_ctxt >>
+      irule_at Any exp_eq_trans >> irule_at Any Letrec_Prim >>
+      gvs [] >> rpt $ irule_at Any exp_eq_refl) >>
+  irule_at Any exp_eq_IMP_exp_eq_in_ctxt >> irule_at Any Let_Seq >> fs []
+QED
+
+Theorem fdemands_IsFree:
+  ∀d c v e len. v ∉ freevars e ∧ e fdemands (d, len, c) ⇒ e fdemands (d, len, IsFree v c)
+Proof
+  rw [fdemands_def] >> irule fdemands_exp_eq >> first_x_assum $ irule_at Any >>
+  irule exp_eq_IMP_exp_eq_in_ctxt >>
+  irule eval_IMP_exp_eq >> dxrule $ GSYM subst_fdomsub >>
+  rw [subst_def, eval_thm, IMP_closed_subst, FRANGE_FLOOKUP, bind1_def]
+QED
+
+Theorem fdemands_Bind:
+  ∀d c v e e2 len. v ∉ freevars e ∧ e fdemands (d, len, c) ⇒ e fdemands (d, len, Bind v e2 c)
+Proof
+  rw [fdemands_def] >> irule fdemands_exp_eq >> first_x_assum $ irule_at Any >>
+  irule exp_eq_IMP_exp_eq_in_ctxt >>
+  irule eval_IMP_exp_eq >> dxrule $ GSYM subst_fdomsub >>
+  rw [subst_def, eval_thm, IMP_closed_subst, FRANGE_FLOOKUP, bind1_def]
+QED
+
+Theorem fdemands_RecBind:
+  ∀c p l e b. e fdemands (p, l, c)
+              ∧ EVERY (λv. v ∉ freevars e) (MAP FST b)
+              ⇒ e fdemands (p, l, RecBind b c)
+Proof
+  rw [fdemands_def] >> irule fdemands_exp_eq >>
+  last_x_assum $ irule_at Any >>
+  irule exp_eq_IMP_exp_eq_in_ctxt >> irule $ iffLR exp_eq_sym >>
+  gvs [Letrec_not_in_freevars]
+QED
+
+Theorem fdemands_App:
+  ∀c e e2 ps i len. e fdemands ((ps, SUC i), SUC len, c) ⇒ App e e2 fdemands  ((ps, i), len, c)
+Proof
+  Induct
+  >- (rw [fdemands_def, GSYM Apps_def] >>
+      rename1 ‘e2::l’ >> pop_assum $ qspecl_then [‘e2::l’] assume_tac >>
+      gvs []) >>
+  rw [fdemands_def] >> irule fdemands_exp_eq >>
+  rpt $ last_x_assum $ irule_at Any >>
+  irule_at Any $ iffLR exp_eq_in_ctxt_sym
+  >~[‘Letrec’] >- (irule_at Any exp_eq_IMP_exp_eq_in_ctxt >> irule_at Any Letrec_App) >>
+  irule_at Any Let_App_in_ctxt
+QED
+
+Theorem fdemands_Apps:
+  ∀eL c e ps i len. e fdemands ((ps, i + LENGTH eL), len + LENGTH eL, c) ⇒ Apps e eL fdemands  ((ps, i), len, c)
+Proof
+  Induct >> gvs [Apps_def] >> rw [] >>
+  last_x_assum irule >> irule fdemands_App >>
+  gvs [SUC_ADD]
+QED
+
+Theorem fdemands_App2:
+  ∀d e e2 eL len c. e fdemands (([], 0), SUC len, c) ∧ e2 demands (d, c) ∧ LENGTH eL = len
+            ⇒ Apps (App e e2) eL demands (d, c)
+Proof
+  PairCases >> rw [] >>
+  dxrule_then assume_tac fdemands_alt >>
+  gvs [fdemands_def, GSYM Apps_def, GSYM needs_Var_is_demands] >>
+  rename1 ‘e2::eL’ >> last_x_assum $ qspecl_then [‘e2::eL’] assume_tac >>
+  irule needs_trans >>
+  pop_assum $ irule_at Any >>
+  gvs []
+QED
+
+Theorem fdemands_subset:
+  ∀fdc fdc'.
+    (∀n l i c2. (n, l) ∈ fdc ∧ i < LENGTH l ∧ EL i l ⇒ Var n fdemands (([], i), LENGTH l, concat_ctxt c c2))
+    ∧ fdc' ⊆ fdc
+    ⇒ (∀n l i. (n, l) ∈ fdc' ∧ i < LENGTH l ∧ EL i l ⇒ Var n fdemands (([], i), LENGTH l, concat_ctxt c c2))
+Proof
+  gvs [SUBSET_DEF]
+QED
+
+Theorem fdemands_set_Bind:
+  ∀fdc v e.
+    (∀n l i c2. (n, l) ∈ fdc ∧ i < LENGTH l ∧ EL i l ⇒ Var n fdemands (([], i), LENGTH l, concat_ctxt c c2))
+    ∧ (∀n l. (n, l) ∈ fdc ⇒ n ≠ v)
+    ⇒ (∀n l i c2. (n, l) ∈ fdc ∧ i < LENGTH l ∧ EL i l
+               ⇒ Var n fdemands (([], i), LENGTH l, concat_ctxt (Bind v e c) c2))
+Proof
+  rw [concat_ctxt_def]
+  \\ irule fdemands_Bind
+  \\ gvs []
+  \\ strip_tac \\ gvs []
+QED
+
+Theorem fdemands_set_IsFree:
+  ∀fdc v.
+    (∀n l i c2. (n, l) ∈ fdc ∧ i < LENGTH l ∧ EL i l ⇒ Var n fdemands (([], i), LENGTH l, concat_ctxt c c2))
+    ∧ (∀l. (v, l) ∉ fdc)
+    ⇒ (∀n l i c2. (n, l) ∈ fdc ∧ i < LENGTH l ∧ EL i l
+               ⇒ Var n fdemands (([], i), LENGTH l, concat_ctxt (IsFree v c) c2))
+Proof
+  rw [concat_ctxt_def]
+  \\ irule fdemands_IsFree
+  \\ gvs []
+  \\ strip_tac \\ gvs []
+QED
+
+Theorem fdemands_set_FOLDL_IsFree:
+  ∀vL fdc c.
+    (∀n l i c2. (n, l) ∈ fdc ∧ i < LENGTH l ∧ EL i l ⇒ Var n fdemands (([], i), LENGTH l, concat_ctxt c c2))
+    ∧ EVERY (λv. ∀argDs. (v, argDs) ∉ fdc) vL
+    ⇒ (∀n l i c2. (n, l) ∈ fdc ∧ i < LENGTH l ∧ EL i l
+               ⇒ Var n fdemands (([], i), LENGTH l, concat_ctxt (FOLDL (λc n. IsFree n c) c vL) c2 ))
+Proof
+  Induct \\ rw [concat_ctxt_def]
+  \\ last_x_assum irule
+  \\ gvs []
+  \\ last_assum $ irule_at Any
+  \\ dxrule_then assume_tac fdemands_set_IsFree
+  \\ pop_assum $ dxrule_then assume_tac
+  \\ fs []
+QED
+
+Theorem fdemands_set_RecBind:
+  ∀fdc c b.
+    (∀n l i c2. (n, l) ∈ fdc ∧ i < LENGTH l ∧ EL i l ⇒ Var n fdemands (([], i), LENGTH l, concat_ctxt c c2))
+    ∧ EVERY (λv. ∀argDs. (v, argDs) ∉ fdc) (MAP FST b)
+    ⇒ (∀n l i c2. (n, l) ∈ fdc ∧ i < LENGTH l ∧ EL i l
+               ⇒ Var n fdemands (([], i), LENGTH l, concat_ctxt (RecBind b c) c2))
+Proof
+  rw [concat_ctxt_def] >> irule fdemands_RecBind >>
+  gvs [EVERY_EL, EL_MAP] >> rw [] >> strip_tac >>
+  first_x_assum $ dxrule_then assume_tac >> gvs []
+QED
+
+(*Theorem fdemands_concat_ctxt:
+  ∀c p len e. e fdemands (p, len, Nil) ⇒ e fdemands (p, len, c)
+Proof
+  Induct >> rw [fdemands_def] >>
+  last_x_assum irule >>
+  rename1 ‘_ fdemands (p, _, _)’ >> PairCases_on ‘p’ >>
+  gvs [fdemands_def] >> rw [] >>
+  completeInduct_on ‘ctxt_size c’ >>
+  Cases >> gvs [FORALL_PROD] >>
+  rpt strip_tac >> rw [fdemands_def] >> last_assum irule >> rw [ctxt_size_def]
+  >~[‘Letrec’]
+  >- cheat >>
+  irule exp_eq_trans >> irule_at Any exp_eq_Apps_cong >>
+  rename1 ‘Apps (Let v e2 e1) l’ >>
+  ‘∃s. s ∉ {v} ∪ freevars e1 ∪ freevars (Apps e1 l)’ by cheat >>
+  irule_at (Pos $ el 2) exp_eq_App_cong >>
+  irule_at (Pos hd) exp_alpha_exp_eq >> irule_at Any exp_alpha_Alpha >>
+  gvs [freevars_Apps] >> first_assum $ irule_at Any >> gvs [] >>
+  irule_at (Pos hd) exp_eq_refl >>
+  irule_at Any exp_eq_trans >> irule_at (Pos hd) $ iffLR exp_eq_sym >> irule_at Any Let_Apps >>
+  irule_at Any exp_eq_trans >> irule_at Any exp_eq_App_cong >>
+  irule_at Any exp_eq_Lam_cong >> last_x_assum $ irule_at Any >>
+  irule_at (Pos $ el 2) exp_eq_refl >>
+  irule_at Any exp_eq_trans >> irule_at Any Let_Seq >>
+  irule_at Any exp_eq_Prim_cong >>
+  cheat
+QED*)
+
+val _ = set_fixity "demands_when_applied" (Infixl 480);
+
+Definition demands_when_applied_def:
+  f demands_when_applied ((ps, v), len, c) = eq_when_applied c f (Seq (Projs ps (Var v)) f) len
 End
 
-Inductive find: (* i i o o *)
+val _ = set_fixity "needs_when_applied" (Infixl 480);
+
+Definition needs_when_applied_def:
+  f needs_when_applied ((ps, e), len, c) = eq_when_applied c f (Seq (Projs ps e) f) len
+End
+
+Theorem needs_when_applied_0:
+  ∀p f c. f needs_when_applied (p, 0, c) = f needs (p, c)
+Proof
+  PairCases >> gvs [needs_when_applied_def, needs_def, eq_when_applied_0]
+QED
+
+Theorem demands_when_applied_0:
+  ∀p f c. f demands_when_applied (p, 0, c) = f demands (p, c)
+Proof
+  PairCases >> gvs [demands_when_applied_def, demands_def, eq_when_applied_0]
+QED
+
+Theorem demands_w_app_is_needs_w_app:
+  ∀f c ps v e len. f demands_when_applied ((ps, v), len, c) = f needs_when_applied ((ps, Var v), len, c)
+Proof
+  rw [demands_when_applied_def, needs_when_applied_def]
+QED
+
+Theorem eq_when_applied_trans_exp_eq:
+  ∀c e1 e2 e3 len.
+    exp_eq_in_ctxt c e1 e2 ∧ eq_when_applied c e2 e3 len
+    ⇒ eq_when_applied c e1 e3 len
+Proof
+  rw [] >> irule eq_when_applied_trans >>
+  first_x_assum $ irule_at Any >>
+  gvs [exp_eq_in_ctxt_IMP_eq_when_applied]
+QED
+
+Theorem fdemands_0_App_needs:
+  ∀c f e d len. e needs (d, c) ∧ f fdemands (([], 0), SUC len, c)
+                ⇒ App f e needs_when_applied (d, len, c)
+Proof
+  Induct >>
+  gvs[FORALL_PROD, needs_when_applied_def, fdemands_def,
+      eq_when_applied_def, exp_eq_in_ctxt_def, Projs_def] >>
+  rw [GSYM Apps_def]
+  >- (irule exp_eq_trans >>
+      irule_at (Pos last) $ iffLR exp_eq_sym >> irule_at Any Apps_Seq >>
+      rename1 ‘Apps f(e::l)’ >> pop_assum $ qspecl_then [‘e::l’] assume_tac >> fs [] >>
+      dxrule_then (dxrule_then assume_tac) needs_trans >>
+      gvs [needs_def, exp_eq_in_ctxt_def, Apps_def])
+  >~[‘Letrec’]
+  >- (irule eq_when_applied_trans_exp_eq >> irule_at Any exp_eq_IMP_exp_eq_in_ctxt >>
+      irule_at Any Letrec_App >>
+      irule_at Any eq_when_applied_trans >> last_x_assum $ irule_at Any >>
+      gvs [needs_def, exp_eq_in_ctxt_def] >>
+      irule_at Any exp_eq_in_ctxt_trans >> first_x_assum $ irule_at Any >>
+      irule_at Any exp_eq_IMP_exp_eq_in_ctxt >> irule_at Any exp_eq_trans >>
+      irule_at Any Letrec_Prim >> irule_at Any exp_eq_Prim_cong >>
+      gvs [exp_eq_refl] >> irule_at Any Letrec_Projs >>
+      irule exp_eq_in_ctxt_IMP_eq_when_applied >> irule exp_eq_IMP_exp_eq_in_ctxt >>
+      irule $ iffLR exp_eq_sym >> irule exp_eq_trans >>
+      irule_at Any Letrec_Prim >> irule_at Any exp_eq_Prim_cong >>
+      gvs [Letrec_App, Letrec_Projs]) >>
+  irule eq_when_applied_trans_exp_eq >> irule_at Any Let_App_in_ctxt >>
+  irule eq_when_applied_trans >> last_x_assum $ irule_at Any
+  >- (gvs [needs_def] >>
+      irule_at Any exp_eq_in_ctxt_trans >> irule_at Any exp_eq_in_ctxt_App >>
+      irule_at Any exp_eq_in_ctxt_Lam >> last_x_assum $ irule_at Any >>
+      irule_at Any exp_eq_in_ctxt_refl >>
+      irule_at Any exp_eq_IMP_exp_eq_in_ctxt >> irule_at Any exp_eq_trans >>
+      irule_at Any Let_Seq >> irule_at Any exp_eq_Prim_cong >>
+      gvs [exp_eq_refl] >> irule_at Any Let_Projs >>
+      irule exp_eq_in_ctxt_IMP_eq_when_applied >> irule exp_eq_IMP_exp_eq_in_ctxt >>
+      irule $ iffLR exp_eq_sym >> irule exp_eq_trans >>
+      irule_at Any Let_Seq >> irule_at Any exp_eq_Prim_cong >>
+      gvs [Let_App, Let_Projs])
+  >- (gvs [needs_def, exp_eq_in_ctxt_def] >>
+      irule_at Any exp_eq_in_ctxt_trans >> last_x_assum $ irule_at Any >> fs [] >>
+      irule_at Any exp_eq_IMP_exp_eq_in_ctxt >> irule_at Any exp_eq_trans >>
+      irule_at Any Let_Seq >> irule_at Any exp_eq_Prim_cong >>
+      gvs [exp_eq_refl] >> irule_at Any Let_Projs >>
+      irule exp_eq_in_ctxt_IMP_eq_when_applied >> irule exp_eq_IMP_exp_eq_in_ctxt >>
+      irule $ iffLR exp_eq_sym >> irule exp_eq_trans >>
+      irule_at Any Let_Seq >> irule_at Any exp_eq_Prim_cong >>
+      gvs [Let_App, Let_Projs])
+QED
+
+Theorem needs_when_applied_App:
+  ∀c p f len e. f needs_when_applied (p, SUC len, c)
+                ⇒ (App f e) needs_when_applied (p, len, c)
+Proof
+  gvs [FORALL_PROD, needs_when_applied_def] >> rw [] >>
+  irule eq_when_applied_trans >> irule_at Any eq_when_applied_App >>
+  irule_at Any exp_eq_in_ctxt_refl >> pop_assum $ irule_at Any >>
+  gvs [exp_eq_IMP_eq_when_applied, App_Seq]
+QED
+
+Theorem demands_when_applied_App:
+  ∀c p f len e. f demands_when_applied (p, SUC len, c)
+                ⇒ (App f e) demands_when_applied (p, len, c)
+Proof
+  gvs [FORALL_PROD, needs_when_applied_App, demands_w_app_is_needs_w_app]
+QED
+
+Theorem demands_when_applied_Apps:
+  ∀eL c p f len. f demands_when_applied (p, len + LENGTH eL, c)
+                ⇒ (Apps f eL) demands_when_applied (p, len, c)
+Proof
+  Induct >> rw [Apps_def] >>
+  last_x_assum irule >> irule demands_when_applied_App >>
+  gvs [SUC_ADD]
+QED
+
+Theorem demands_when_applied_Apps2:
+  ∀eL i c p f len. f fdemands (([], i), len + LENGTH eL, c) ∧ EL i eL demands (p, c) ∧ i < LENGTH eL
+                ⇒ (Apps f eL) demands_when_applied (p, len, c)
+Proof
+  Induct >> gvs [FORALL_PROD] >>
+  gen_tac >> Cases
+  >~[‘EL 0’]
+  >- (rw [Apps_def] >>
+      irule demands_when_applied_Apps >>
+      irule $ iffRL demands_w_app_is_needs_w_app >>
+      irule fdemands_0_App_needs >>
+      gvs [SUC_ADD, needs_Var_is_demands]) >>
+  rw [Apps_def] >>
+  last_x_assum irule >>
+  first_x_assum $ irule_at Any >>
+  gvs [fdemands_App, SUC_ADD]
+QED
+
+Theorem demands_when_applied_Lam_lemma:
+  ∀c p f len e v.
+    eq_when_applied c (Lam v f) (Lam v (Seq p f)) (SUC len) ∧ v ∉ freevars p
+    ⇒ eq_when_applied c (Lam v f) (Seq p (Lam v f)) (SUC len)
+Proof
+  Induct >> gvs [eq_when_applied_def]
+  >- (rpt gen_tac >> strip_tac >> Cases >> rw [] >>
+      irule exp_eq_trans >> last_x_assum $ irule_at Any >>
+      gvs [Apps_def] >>
+      irule exp_eq_Apps_cong >> gvs [exp_eq_l_refl] >>
+      irule exp_eq_trans >> irule_at Any Let_Seq >>
+      irule $ iffLR exp_eq_sym >> irule exp_eq_trans >> irule_at Any App_Seq >>
+      irule exp_eq_Prim_cong >> fs [exp_eq_refl] >>
+      irule eval_IMP_exp_eq >>
+      rw [subst_def, bind1_def, FRANGE_FLOOKUP, IMP_closed_subst, eval_thm, GSYM subst_fdomsub]) >>
+  rw [] >> irule eq_when_applied_trans_exp_eq
+  >~[‘Letrec l (Lam v (Seq p f))’]
+  >- (‘∃s. s ∉ {v} ∪ freevars p ∪ freevars f ∪ set (MAP FST l) ∪ BIGUNION (set (MAP freevars (MAP SND l)))’
+        by (‘INFINITE 𝕌(:string)’ by simp [] \\ dxrule_then assume_tac $ iffLR NOT_IN_FINITE
+             \\ pop_assum $ irule_at Any \\ rw [FINITE_UNION, FINITE_BIGUNION, MEM_EL]
+             \\ gvs [EL_MAP]) >>
+      irule_at Any exp_eq_IMP_exp_eq_in_ctxt >>
+      irule_at Any exp_eq_trans >> irule_at (Pos hd) exp_eq_Letrec_cong >>
+      irule_at Any exp_eq_l_refl >>
+      irule_at (Pos hd) exp_alpha_exp_eq >> irule_at Any exp_alpha_Alpha >>
+      irule_at Any Letrec_Lam_weak >>
+      fs [] >> first_assum $ irule_at Any >> gvs [] >>
+      conj_asm1_tac
+      >- (rw [EVERY_MEM] >>
+          rename1 ‘MEM e (MAP SND l)’ >> first_x_assum $ qspecl_then [‘freevars e’] assume_tac >>
+          gvs [MEM_MAP]) >>
+      irule_at (Pos hd) eq_when_applied_trans >> last_x_assum $ irule_at Any >>
+      irule_at (Pos hd) eq_when_applied_trans_exp_eq >> irule_at Any exp_eq_IMP_exp_eq_in_ctxt >>
+      irule_at (Pos hd) $ iffLR exp_eq_sym >> irule_at Any Letrec_Lam_weak >> fs [] >>
+      irule_at (Pos hd) eq_when_applied_trans_exp_eq >> irule_at Any exp_eq_IMP_exp_eq_in_ctxt >>
+      irule_at Any exp_eq_Letrec_cong >> irule_at Any exp_eq_l_refl >>
+      irule_at Any $ iffLR exp_eq_sym >> irule_at Any exp_alpha_exp_eq >> irule_at Any exp_alpha_Alpha >> fs [] >>
+      irule_at (Pos hd) eq_when_applied_trans >> last_x_assum $ irule_at Any >>
+      rpt $ irule_at Any exp_eq_IMP_eq_when_applied >> irule_at (Pos hd) $ iffLR exp_eq_sym >>
+      irule_at (Pos hd) exp_eq_trans >> irule_at Any Letrec_Prim >>
+      irule_at Any exp_eq_Prim_cong >> fs [] >>
+      irule_at (Pos hd) exp_eq_refl >> fs [] >>
+      irule_at (Pos hd) exp_eq_trans >> irule_at (Pos $ el 2) Letrec_Lam_weak >> fs [] >>
+      irule_at Any exp_eq_Letrec_cong >> fs [exp_eq_l_refl] >>
+      irule_at (Pos hd) exp_alpha_exp_eq >> irule_at Any exp_alpha_Alpha >>
+      gvs [MAP_MAP_o, combinTheory.o_DEF, LAMBDA_PROD] >>
+      irule exp_eq_trans >> irule_at (Pos hd) exp_eq_Letrec_cong >> irule_at Any exp_eq_l_refl >> fs [] >>
+      irule_at (Pos hd) exp_alpha_exp_eq >> irule_at Any exp_alpha_Alpha >>
+      fs [] >> first_assum $ irule_at Any >> fs [] >>
+      irule exp_eq_trans >> irule_at Any Letrec_Lam_weak >> fs [perm_exp_def] >>
+      irule exp_eq_Lam_cong >>
+      irule exp_eq_trans >> irule_at Any Letrec_Prim >>
+      irule exp_eq_Prim_cong >> fs [exp_eq_refl] >>
+      irule exp_eq_Letrec_cong >> fs [exp_eq_l_refl, Once exp_eq_sym] >>
+      irule exp_alpha_exp_eq >> gvs [exp_alpha_perm_irrel]) >>
+  rename1 ‘Let w e (Seq p (Lam v f))’ >>
+  ‘∃s. s ∉ {v} ∪ {w} ∪ freevars p ∪ freevars f ∪ freevars e’
+    by (‘INFINITE 𝕌(:string)’ by simp [] \\ gvs [NOT_IN_FINITE]) >>
+  irule_at Any exp_eq_IMP_exp_eq_in_ctxt >>
+  irule_at Any exp_eq_trans >> irule_at (Pos hd) exp_eq_App_cong >>
+  irule_at (Pos hd) exp_eq_Lam_cong >> irule_at (Pos $ el 2) exp_eq_refl >>
+  irule_at (Pos hd) exp_alpha_exp_eq >> irule_at Any exp_alpha_Alpha >>
+  irule_at Any Let_Lam_weak >>
+  fs [] >> first_assum $ irule_at Any >> gvs [] >>
+  irule_at (Pos hd) eq_when_applied_trans >> last_x_assum $ irule_at Any >>
+  irule_at (Pos hd) eq_when_applied_trans_exp_eq >> irule_at Any exp_eq_IMP_exp_eq_in_ctxt >>
+  irule_at (Pos hd) $ iffLR exp_eq_sym >> irule_at Any Let_Lam_weak >> fs [] >>
+  irule_at (Pos hd) eq_when_applied_trans_exp_eq >> irule_at Any exp_eq_IMP_exp_eq_in_ctxt >>
+  irule_at Any exp_eq_App_cong >> irule_at (Pos hd) exp_eq_Lam_cong >>
+  irule_at (Pos $ el 2) exp_eq_refl >>
+  irule_at Any $ iffLR exp_eq_sym >> irule_at Any exp_alpha_exp_eq >> irule_at Any exp_alpha_Alpha >> fs [] >>
+  irule_at (Pos hd) eq_when_applied_trans >> last_x_assum $ irule_at Any >>
+  rpt $ irule_at Any exp_eq_IMP_eq_when_applied >> irule_at (Pos hd) $ iffLR exp_eq_sym >>
+  irule_at (Pos hd) exp_eq_trans >> irule_at Any Let_Seq >>
+  irule_at Any exp_eq_Prim_cong >> fs [] >>
+  irule_at (Pos hd) exp_eq_refl >> fs [] >>
+  irule_at (Pos hd) exp_eq_trans >> irule_at (Pos $ el 2) Let_Lam_weak >> fs [] >>
+  irule_at Any exp_eq_App_cong >> irule_at Any exp_eq_Lam_cong >> fs [exp_eq_refl] >>
+  irule_at (Pos hd) exp_alpha_exp_eq >> irule_at Any exp_alpha_Alpha >>
+  gvs [MAP_MAP_o, combinTheory.o_DEF, LAMBDA_PROD] >>
+  irule exp_eq_trans >> irule_at Any exp_eq_App_cong >>
+  irule_at (Pos hd) exp_eq_Lam_cong >> irule_at (Pos $ el 2) exp_eq_refl >>
+  irule_at (Pos hd) exp_alpha_exp_eq >> irule_at Any exp_alpha_Alpha >>
+  fs [] >> first_assum $ irule_at Any >> fs [] >>
+  irule exp_eq_trans >> irule_at Any Let_Lam_weak >> fs [perm_exp_def] >>
+  irule exp_eq_Lam_cong >>
+  irule exp_eq_trans >> irule_at Any Let_Seq >>
+  irule exp_eq_Prim_cong >> fs [exp_eq_refl] >>
+  irule exp_eq_App_cong >> irule_at Any exp_eq_Lam_cong >> fs [exp_eq_refl, Once exp_eq_sym] >>
+  irule exp_alpha_exp_eq >> gvs [exp_alpha_perm_irrel]
+QED
+
+Theorem demands_when_applied_Lam:
+  ∀c p f len e v. f demands_when_applied (p, len, IsFree v c) ∧ v ≠ SND p
+                ⇒ (Lam v f) demands_when_applied (p, SUC len, c)
+Proof
+  gvs [FORALL_PROD, demands_when_applied_def] >> rw [] >>
+  irule demands_when_applied_Lam_lemma >>
+  gvs [eq_when_applied_Lam, freevars_Projs]
+QED
+
+Theorem demands_when_applied_Lams:
+  ∀vL c p f len e. f demands_when_applied (p, len, FOLDL (λc n. (IsFree n c)) c vL) ∧ ¬ MEM (SND p) vL
+                ⇒ (Lams vL f) demands_when_applied (p, len + LENGTH vL, c)
+Proof
+  Induct >> gvs [Lams_def] >>
+  rw [GSYM SUC_ADD] >>
+  irule demands_when_applied_Lam >>
+  gvs []
+QED
+
+Theorem needs_when_applied_Seq:
+  ∀c p f len e. f needs_when_applied (p, len, c)
+                ⇒ (Seq e f) needs_when_applied (p, len, c)
+Proof
+  Induct >> gvs [FORALL_PROD, needs_when_applied_def, eq_when_applied_def] >> rw []
+  >- (irule exp_eq_trans >> irule_at Any Apps_Seq >>
+      irule exp_eq_trans >> irule_at Any exp_eq_Apps_cong >>
+      irule_at Any exp_eq_l_refl >>
+      irule_at (Pos hd) exp_eq_trans >> irule_at (Pos $ el 2) Seq_assoc >>
+      irule_at (Pos hd) exp_eq_trans >> irule_at (Pos $ el 2) Seq_comm >>
+      irule_at (Pos hd) $ iffLR exp_eq_sym >> irule_at Any Seq_assoc >>
+      irule exp_eq_trans >> irule_at (Pos last) $ iffLR exp_eq_sym >>
+      irule_at Any Apps_Seq >> irule exp_eq_Prim_cong >>
+      gvs [exp_eq_refl])
+  >~[‘Letrec’]
+  >- (irule eq_when_applied_trans_exp_eq >> irule_at Any exp_eq_IMP_exp_eq_in_ctxt >>
+      irule_at Any Letrec_Prim >> fs [] >>
+      irule eq_when_applied_trans >> last_x_assum $ irule_at Any >>
+      irule_at (Pos hd) eq_when_applied_trans >> first_x_assum $ irule_at Any >>
+      rpt $ irule_at Any exp_eq_in_ctxt_IMP_eq_when_applied >>
+      rpt $ irule_at Any exp_eq_IMP_exp_eq_in_ctxt >>
+      irule_at (Pos hd) exp_eq_trans >> irule_at Any Letrec_Prim >>
+      irule_at Any exp_eq_Prim_cong >> gvs [exp_eq_refl] >>
+      irule_at Any Letrec_Projs >> irule $ iffLR exp_eq_sym >>
+      irule_at Any exp_eq_trans >> irule_at Any Letrec_Prim >> irule exp_eq_Prim_cong >>
+      gvs [Letrec_Projs] >>
+      irule exp_eq_trans >> irule_at Any Letrec_Prim >> gvs [exp_eq_refl]) >>
+  irule eq_when_applied_trans_exp_eq >> irule_at Any exp_eq_IMP_exp_eq_in_ctxt >>
+  irule_at Any Let_Seq >>
+  irule eq_when_applied_trans >> last_x_assum $ irule_at Any >>
+  irule_at (Pos hd) eq_when_applied_trans >> first_x_assum $ irule_at Any >>
+  rpt $ irule_at Any exp_eq_in_ctxt_IMP_eq_when_applied >>
+  rpt $ irule_at Any exp_eq_IMP_exp_eq_in_ctxt >>
+  irule_at (Pos hd) exp_eq_trans >> irule_at Any Let_Seq >>
+  irule_at Any exp_eq_Prim_cong >> gvs [exp_eq_refl] >>
+  irule_at Any Let_Projs >> irule $ iffLR exp_eq_sym >>
+  irule_at Any exp_eq_trans >> irule_at Any Let_Seq >> irule exp_eq_Prim_cong >>
+  gvs [Let_Projs, Let_Seq]
+QED
+
+Theorem demands_when_applied_Seq:
+  ∀p c  f len e. f demands_when_applied (p, len, c)
+                ⇒ (Seq e f) demands_when_applied (p, len, c)
+Proof
+  gvs [FORALL_PROD, demands_w_app_is_needs_w_app, needs_when_applied_Seq]
+QED
+
+Theorem fdemands_0_App_demands:
+  ∀c f e d len. e demands (d, c) ∧ f fdemands (([], 0), SUC len, c)
+                ⇒ App f e demands_when_applied (d, len, c)
+Proof
+  gvs [FORALL_PROD, fdemands_0_App_needs, demands_w_app_is_needs_w_app, needs_Var_is_demands]
+QED
+
+Theorem demands_when_applied_IsFree_Bind:
+  ∀c v e e' d len. e demands_when_applied (d, len, IsFree v c) ∧ SND d ≠ v
+                   ⇒ e demands_when_applied (d, len, Bind v e' c)
+Proof
+  fs [FORALL_PROD] >> rw [] >> simp [demands_when_applied_def, eq_when_applied_def] >>
+  dxrule_then assume_tac demands_when_applied_Lam >> gvs [] >>
+  dxrule_then assume_tac demands_when_applied_App >>
+  gvs [demands_when_applied_def] >>
+  irule eq_when_applied_trans >> first_x_assum $ irule_at Any >>
+  irule exp_eq_IMP_eq_when_applied >> irule $ iffLR exp_eq_sym >>
+  irule exp_eq_trans >> irule_at Any Let_Seq >>
+  irule exp_eq_Prim_cong >> fs [exp_eq_refl] >>
+  irule exp_eq_trans >> irule_at Any Let_Projs >>
+  irule exp_eq_Projs_cong >> irule Let_Var2 >> fs []
+QED
+
+Theorem demands_when_applied_Letrec:
+  ∀b e d len c. e demands_when_applied (d, len, RecBind b c) ∧ (¬MEM (SND d) (MAP FST b))
+                ⇒ Letrec b e demands_when_applied (d, len, c)
+Proof
+  gvs [FORALL_PROD, demands_when_applied_def, eq_when_applied_def] >> rw [] >>
+  irule eq_when_applied_trans >> last_x_assum $ irule_at Any >>
+  irule exp_eq_IMP_eq_when_applied >>
+  irule exp_eq_trans >> irule_at Any Letrec_Prim >>
+  irule exp_eq_Prim_cong >> fs [exp_eq_refl] >>
+  irule Letrec_not_in_freevars >>
+  gvs [freevars_Projs, EVERY_MEM]
+QED
+
+Theorem Lam_fdemands_lemma:
+  ∀c v e ps len. Lam v (Seq (Projs ps (Var v)) e) fdemands ((ps, 0), SUC len, c)
+Proof
+  Induct >> gvs [fdemands_def]
+  >- (rw [] >> rename1 ‘HD l’ >> Cases_on ‘l’ >> gvs [Apps_def, needs_def] >>
+      irule exp_eq_IMP_exp_eq_in_ctxt >>
+      irule exp_eq_trans >> irule_at Any exp_eq_Apps_cong >>
+      irule_at Any exp_eq_l_refl >> irule_at Any Let_Seq >>
+      irule exp_eq_trans >> irule_at Any exp_eq_Prim_cong >> gvs [] >>
+      irule_at Any exp_eq_Apps_cong >> gvs [] >>
+      irule_at Any exp_eq_l_refl >> irule_at (Pos hd) $ iffLR exp_eq_sym >>
+      irule_at Any Let_Seq >> irule_at Any exp_eq_refl >>
+      irule exp_eq_trans >> irule_at Any Apps_Seq >>
+      irule exp_eq_trans >> irule_at (Pos hd) exp_eq_Prim_cong >> gvs [] >>
+      irule_at Any Let_Projs >> irule_at (Pos $ el 3) exp_eq_refl >> gvs [] >>
+      irule exp_eq_trans >> irule_at (Pos hd) exp_eq_Prim_cong >> gvs [] >>
+      irule_at (Pos $ el 2) $ iffLR exp_eq_sym >> irule_at (Pos hd) Seq_id >> gvs [] >>
+      irule_at Any exp_eq_refl >> irule exp_eq_trans >>
+      irule_at Any Seq_assoc >> irule exp_eq_Prim_cong >> gvs [exp_eq_Projs_cong, Let_Var, Once exp_eq_sym] >>
+      irule exp_eq_trans >> irule_at Any Apps_Seq >>
+      irule exp_eq_Prim_cong >> gvs [exp_eq_refl, Let_Projs]) >>
+  rw [] >>
+  irule fdemands_exp_eq >>
+  irule_at Any exp_eq_IMP_exp_eq_in_ctxt
+  >~[‘Letrec lcs (Lam v (Seq _ e))’]
+  >- (irule_at Any $ iffLR exp_eq_sym >> irule_at Any exp_eq_trans >>
+      irule_at (Pos hd) exp_eq_Letrec_cong >> irule_at Any exp_eq_l_refl >>
+      irule_at Any exp_alpha_exp_eq >> irule_at Any exp_alpha_Alpha >>
+      irule_at Any Letrec_Lam_weak >> gvs [perm_exp_def, perm_exp_Projs, perm1_def] >>
+      ‘∃s. s ∉ BIGUNION (set (MAP freevars (MAP SND lcs))) ∪ set (MAP FST lcs)
+             ∪ {v} ∪ freevars e’
+        by (‘INFINITE 𝕌(:string)’ by simp [] >>
+            dxrule_then irule $ iffLR NOT_IN_FINITE >>
+            gvs [NOT_IN_FINITE, FINITE_BIGUNION, MEM_MAP] >> rw [] >> fs [freevars_FINITE]) >>
+      fs [] >> first_assum $ irule_at Any >>
+      gvs [freevars_Projs] >> conj_tac
+      >- (rw [EVERY_MEM] >> rename1 ‘MEM e2 (MAP SND _)’ >>
+          last_x_assum $ qspecl_then [‘freevars e2’] assume_tac >>
+          gvs [MEM_MAP]) >>
+      irule fdemands_exp_eq >>
+      last_x_assum $ irule_at Any >>
+      irule_at Any exp_eq_IMP_exp_eq_in_ctxt >>
+      irule_at Any exp_eq_Lam_cong >>
+      irule_at Any $ iffLR exp_eq_sym >> irule_at Any exp_eq_trans >>
+      irule_at Any Letrec_Prim >> irule_at Any exp_eq_Prim_cong >>
+      fs [] >> irule_at Any exp_eq_refl >>
+      irule exp_eq_trans >> irule_at Any Letrec_Projs >>
+      irule_at Any exp_eq_Projs_cong >>
+      irule Letrec_not_in_freevars >> gvs [EVERY_MEM]) >>
+  rename1 ‘Let w e2 (Lam v (Seq _ e1))’ >>
+  irule_at Any $ iffLR exp_eq_sym >> irule_at Any exp_eq_trans >>
+  irule_at (Pos hd) exp_eq_App_cong >> irule_at (Pos hd) exp_eq_Lam_cong >>
+  irule_at (Pos $ el 2) exp_eq_refl >>
+  irule_at Any exp_alpha_exp_eq >> irule_at Any exp_alpha_Alpha >>
+  irule_at Any Let_Lam_weak >> gvs [perm_exp_def, perm_exp_Projs, perm1_def] >>
+  ‘∃s. s ∉ {w} ∪ freevars e1 ∪ {v} ∪ freevars e2’
+    by (‘INFINITE 𝕌(:string)’ by simp [] >> gvs [NOT_IN_FINITE]) >>
+  fs [] >> first_assum $ irule_at Any >>
+  gvs [freevars_Projs] >>
+  irule fdemands_exp_eq >>
+  last_x_assum $ irule_at Any >>
+  irule_at Any exp_eq_IMP_exp_eq_in_ctxt >>
+  irule_at Any exp_eq_Lam_cong >>
+  irule_at Any $ iffLR exp_eq_sym >> irule_at Any exp_eq_trans >>
+  irule_at Any Let_Seq >> irule_at Any exp_eq_Prim_cong >>
+  fs [] >> irule_at Any exp_eq_refl >>
+  irule exp_eq_trans >> irule_at Any Let_Projs >>
+  irule_at Any exp_eq_Projs_cong >> gvs [Let_Var2]
+QED
+
+Theorem Lam_fdemands:
+  ∀c v e ps len. e demands_when_applied ((ps, v), len, IsFree v c)
+                 ⇒ Lam v e fdemands ((ps, 0), SUC len, c)
+Proof
+  rw [demands_when_applied_def] >>
+  irule fdemands_eq_w_app >>
+  irule_at Any eq_when_applied_Lam >>
+  irule_at Any $ iffLR eq_when_applied_sym >>
+  first_x_assum $ irule_at Any >>
+  gvs [Lam_fdemands_lemma]
+QED
+
+Theorem fdemands_Lam:
+  ∀c v e len ps n. e fdemands ((ps, n), len, IsFree v c) ⇒ Lam v e fdemands ((ps, SUC n), SUC len, c)
+Proof
+  Induct >> rw [fdemands_def]
+  >- (pop_assum $ qspecl_then [‘Fail’] assume_tac >> gvs [])
+  >- (gvs [needs_def, exp_eq_in_ctxt_def] >> irule exp_eq_trans >>
+      rename1 ‘LENGTH l = SUC _’ >> Cases_on ‘l’ >> gvs [Apps_def] >>
+      irule_at Any exp_eq_Apps_cong >> irule_at Any exp_eq_l_refl >>
+      irule_at Any exp_eq_App_cong >> irule_at (Pos hd) exp_alpha_exp_eq >>
+      irule_at Any exp_alpha_Alpha >> rename1 ‘EL n t’ >>
+      ‘∃s. s ∉ freevars e ∪ {v} ∪ BIGUNION (set (MAP freevars t))’
+        by (‘INFINITE 𝕌(:string)’ by simp [] >> dxrule_then assume_tac $ iffLR NOT_IN_FINITE >>
+             pop_assum $ irule_at Any >> rw [FINITE_UNION, FINITE_BIGUNION, MEM_EL] >>
+             gvs [EL_MAP]) >>
+      fs [] >> first_assum $ irule_at Any >> fs [] >>
+      irule_at Any exp_eq_refl >>
+      irule exp_eq_trans >> irule_at (Pos hd) $ iffLR exp_eq_sym >>
+      irule_at (Pos hd) exp_eq_trans >> irule_at (Pos hd) Let_Apps >>
+      irule_at Any exp_eq_Apps_cong >> irule_at Any exp_eq_refl >>
+      irule_at Any $ iffRL LIST_REL_EL_EQN >> irule_at Any LENGTH_MAP >> gvs [EL_MAP] >>
+      conj_asm1_tac
+      >- (rw [EL_MAP] >> irule Let_not_in_freevars >>
+          rename1 ‘freevars (EL n2 t)’ >> last_x_assum $ qspecl_then [‘freevars (EL n2 t)’] assume_tac >>
+          gvs [MEM_MAP] >>
+          pop_assum $ qspecl_then [‘EL n2 t’] assume_tac >> gvs [EL_MEM]) >>
+      irule exp_eq_trans >> irule_at (Pos last) $ iffLR exp_eq_sym >>
+      irule_at (Pos hd) exp_eq_trans >> irule_at (Pos hd) exp_eq_Prim_cong >> gvs [] >>
+      irule_at (Pos $ el 2) $ iffLR exp_eq_sym >>
+      irule_at (Pos hd) exp_eq_trans >> irule_at (Pos hd) Let_Projs >>
+      irule_at (Pos hd) exp_eq_Projs_cong >> first_assum $ irule_at (Pos hd) >> gvs [] >>
+      irule_at (Pos $ el 2) $ iffLR exp_eq_sym >>
+      irule_at (Pos hd) exp_eq_trans >> irule_at (Pos hd) Let_Apps >>
+      irule_at (Pos hd) exp_eq_Apps_cong >> irule_at Any exp_eq_App_cong >>
+      irule_at (Pos hd) $ iffLR exp_eq_sym >> irule_at (Pos hd) exp_alpha_exp_eq >>
+      irule_at (Pos hd) exp_alpha_Alpha >> first_assum $ irule_at Any >> gvs [] >>
+      irule_at Any $ iffRL LIST_REL_EL_EQN >> irule_at Any LENGTH_MAP >>
+      irule_at (Pos $ el 2) exp_eq_refl >> gvs [EL_MAP] >>
+      irule_at (Pos $ el 2) $ iffLR exp_eq_sym >> irule_at Any Let_Seq >>
+      irule_at Any exp_eq_App_cong >> fs [exp_eq_refl] >>
+      irule_at Any $ iffRL exp_eq_Lam_strong >>
+      last_assum $ qspecl_then [‘Fail’] assume_tac >> gvs [] >>
+      rw [] >>
+      irule exp_eq_trans >> irule_at (Pos hd) $ iffLR exp_eq_sym >>
+      irule_at (Pos hd) beta_equality >> fs [] >>
+      irule exp_eq_trans >> irule_at Any Let_Apps >>
+      irule exp_eq_trans >> irule_at Any exp_eq_Apps_cong >>
+      irule_at Any $ iffRL LIST_REL_EL_EQN >> irule_at Any LENGTH_MAP >> gvs [EL_MAP] >>
+      irule_at (Pos $ el 2) $ iffLR exp_eq_sym >> irule_at (Pos hd) exp_eq_App_cong >>
+      irule_at (Pos hd) exp_alpha_exp_eq >> irule_at Any exp_alpha_Alpha >> fs [] >>
+      irule_at (Pos hd) exp_eq_refl >>
+      conj_asm1_tac
+      >- (rw [] >> irule Let_not_in_freevars >>
+          rename1 ‘freevars (EL n2 t)’ >> last_x_assum $ qspecl_then [‘freevars (EL n2 t)’] assume_tac >>
+          gvs [MEM_MAP] >>
+          pop_assum $ qspecl_then [‘EL n2 t’] assume_tac >> gvs [EL_MEM]) >>
+      irule exp_eq_trans >> last_x_assum $ drule_then assume_tac >>
+      pop_assum $ qspecl_then [‘t’] assume_tac >> fs [exp_eq_in_ctxt_def] >> pop_assum $ irule_at Any >>
+      irule exp_eq_trans >> irule_at Any beta_equality >> fs [Once exp_eq_sym] >>
+      irule exp_eq_trans >> irule_at Any Let_Seq >>
+      irule exp_eq_Prim_cong >> fs [] >>
+      irule_at Any Let_not_in_freevars >> gvs [freevars_Projs] >>
+      irule_at Any exp_eq_trans >> irule_at Any Let_Apps >>
+      irule_at Any exp_eq_Apps_cong >> gvs [LIST_REL_EL_EQN, EL_MAP, exp_eq_sym] >>
+      irule_at Any exp_eq_App_cong >> fs [exp_eq_refl] >>
+      irule_at Any exp_alpha_exp_eq >> irule_at Any exp_alpha_Alpha >>
+      rename1 ‘freevars (EL n t)’ >> last_x_assum $ qspecl_then [‘freevars (EL n t)’] assume_tac >>
+      gvs [MEM_MAP] >>
+      pop_assum $ qspecl_then [‘EL n t’] assume_tac >> gvs [EL_MEM])
+  >~[‘Letrec lcs (Lam v e)’]
+  >- (irule fdemands_exp_eq >> irule_at Any exp_eq_IMP_exp_eq_in_ctxt >>
+      irule_at Any $ iffLR exp_eq_sym >> irule_at Any exp_eq_trans >>
+      irule_at (Pos hd) exp_eq_Letrec_cong >> irule_at Any exp_eq_l_refl >>
+      irule_at (Pos hd) exp_alpha_exp_eq >> irule_at Any exp_alpha_Alpha >>
+      irule_at Any Letrec_Lam_weak >>
+      last_x_assum $ irule_at $ Pos last >>
+      ‘∃s. s ∉ {v} ∪ freevars e ∪ set (MAP FST lcs) ∪ BIGUNION (set (MAP freevars (MAP SND lcs)))’
+        by (‘INFINITE 𝕌(:string)’ by simp [] >> dxrule_then assume_tac $ iffLR NOT_IN_FINITE >>
+             pop_assum $ irule_at Any >> rw [FINITE_UNION, FINITE_BIGUNION, MEM_EL] >>
+             gvs [EL_MAP]) >>
+      fs [] >> first_assum $ irule_at Any >> gvs [fdemands_def] >>
+      conj_asm2_tac >> rw [EVERY_MEM]
+      >~[‘MEM e2 (MAP SND lcs)’]
+      >- (first_x_assum $ qspecl_then [‘freevars e2’] assume_tac >>
+          gvs [MEM_MAP]) >>
+      irule fdemands_exp_eq >> last_x_assum $ irule_at Any >>
+      irule_at Any exp_eq_IMP_exp_eq_in_ctxt >>
+      irule_at Any exp_eq_trans >> irule_at Any Letrec_App >>
+      irule_at Any exp_eq_App_cong >> irule_at Any Letrec_not_in_freevars >> gvs [closed_def] >>
+      irule exp_eq_trans >> irule_at (Pos $ el 2) Letrec_Lam_weak >>
+      irule_at Any exp_eq_Letrec_cong >> gvs [exp_eq_l_refl] >>
+      irule exp_alpha_exp_eq >> irule exp_alpha_Alpha >> fs []) >>
+  rename1 ‘Let w e2 (Lam v e1)’ >>
+  irule fdemands_exp_eq >> irule_at Any exp_eq_IMP_exp_eq_in_ctxt >>
+  irule_at Any $ iffLR exp_eq_sym >> irule_at Any exp_eq_trans >>
+  irule_at (Pos hd) exp_eq_App_cong >> irule_at (Pos hd) exp_eq_Lam_cong >>
+  irule_at (Pos $ el 2) exp_eq_refl >>
+  irule_at (Pos hd) exp_alpha_exp_eq >> irule_at Any exp_alpha_Alpha >>
+  irule_at Any Let_Lam_weak >>
+  last_x_assum $ irule_at $ Pos last >>
+  ‘∃s. s ∉ {v} ∪ freevars e1 ∪ freevars e2 ∪ {w}’
+    by (‘INFINITE 𝕌(:string)’ by simp [] >> gvs [NOT_IN_FINITE]) >>
+  fs [] >> first_assum $ irule_at Any >> gvs [fdemands_def] >>
+  rw [] >>
+  irule fdemands_exp_eq >> last_x_assum $ irule_at Any >>
+  irule_at Any exp_eq_IMP_exp_eq_in_ctxt >>
+  irule_at Any exp_eq_trans >> irule_at Any Let_App >>
+  irule_at Any exp_eq_App_cong >> irule_at Any Let_not_in_freevars >> gvs [closed_def] >>
+  irule_at Any exp_eq_trans >> irule_at (Pos $ el 2) Let_Lam_weak >>
+  irule_at Any exp_eq_App_cong >> irule_at Any exp_eq_refl >>
+  irule_at Any exp_eq_Lam_cong >> gvs [] >>
+  irule exp_alpha_exp_eq >> irule exp_alpha_Alpha >> fs []
+QED
+
+Theorem Lams_fdemands_lemma:
+  ∀vl i c e ps len1. i < LENGTH vl ∧ ALL_DISTINCT vl
+                     ∧ e demands_when_applied ((ps, EL i vl), len1, FOLDL (λc n. IsFree n c) c vl)
+                     ⇒ Lams vl e fdemands ((ps, i), len1 + LENGTH vl, c)
+Proof
+  Induct >> gvs [Lams_def, FORALL_PROD] >>
+  gen_tac >> Cases >> rw [GSYM SUC_ADD]
+  >- (irule Lam_fdemands >>
+      irule demands_when_applied_Lams >>
+      gvs [])
+  >- (irule fdemands_Lam >> gvs [])
+QED
+
+Theorem Lams_fdemands:
+  ∀vl i c e ps len1. i < LENGTH vl ∧ ALL_DISTINCT vl
+                     ∧ e demands ((ps, EL i vl), FOLDL (λc n. IsFree n c) c vl)
+                     ⇒ Lams vl e fdemands ((ps, i), LENGTH vl, c)
+Proof
+  rw [GSYM demands_when_applied_0] >>
+  dxrule_then (dxrule_then $ dxrule_then assume_tac) Lams_fdemands_lemma >>
+  gvs []
+QED
+
+(*
+val _ = set_fixity "fdemands_depth" (Infixl 480);
+
+Definition fdemands_depth_def:
+  fexp fdemands_depth ((ps, i), len, k, c)
+  = (i < len
+     ∧ ∃s. FINITE s
+           ∧ ∀l. (set l ∩ s = {} ∧ LENGTH l = len)
+                 ⇒ ∀f. freevars (Apps fexp (MAP Var l)) ⊆ FDOM f
+                       ∧ is_bot (eval_wh_to k (subst f (Var (EL i l))))
+             ⇒  is_bot (eval_wh_to k (subst f (Apps fexp (MAP Var l)))))
+End
+
+Theorem exists_str_not_in_list:
+  ∀l. ∃(s : string). ¬ MEM s l
+Proof
+  qsuff_tac `INFINITE 𝕌(:string)`
+  >- rw[pred_setTheory.NOT_IN_FINITE]
+  >- simp[]
+QED
+
+Theorem exists_l_not_in_s:
+  ∀(s : string -> bool) k. FINITE s ⇒ ∃l. ALL_DISTINCT l ∧ EVERY (λx. x ∉ s) l ∧ LENGTH l = k
+Proof
+  gen_tac
+  \\ Induct
+  \\ rw []
+  \\ first_x_assum drule
+  \\ rw []
+  \\ ‘INFINITE 𝕌(:string)’ by simp []
+  \\ ‘∃hd. hd ∉ s ∪ set l’ by
+    fs [NOT_IN_FINITE, FINITE_UNION, FINITE_LIST_TO_SET]
+  \\ qexists_tac ‘hd::l’
+  \\ gvs []
+QED
+
+Theorem DRESTRICT_DOMSUB_COMM:
+  ∀f v s. DRESTRICT (f \\ v) s = (DRESTRICT f s) \\ v
+Proof
+  fs [EQ_FDOM_SUBMAP]
+  \\ rw [DRESTRICT_DEF, DELETE_INTER, SUBMAP_DEF, DOMSUB_FAPPLY_THM]
+QED
+
+(*
+Theorem subst_does_not_change:
+  ∀e v f. v ∉ freevars e ⇒ subst f e = subst (f \\ v) e
+Proof
+  Induct using freevars_ind
+  \\ rw [subst_def, freevars_def, DOMSUB_FLOOKUP_NEQ, MAP_EQ_f, FDIFF_def]
+  \\ gvs [DOMSUB_COMMUTES]
+  >- (first_x_assum $ irule
+      \\ fs []
+      \\ first_x_assum $ qspecl_then [‘freevars a’] assume_tac
+      \\ fs [MEM_EL]
+      \\ pop_assum $ qspecl_then [‘n’] assume_tac
+      \\ gvs [EL_MAP])
+  >>~[‘subst (DRESTRICT _ _) _ = subst _ _’]
+  >- gvs [DRESTRICT_DOMSUB_COMM]
+  >- (rename1 ‘DRESTRICT f (COMPL (set l))’
+      \\ AP_THM_TAC
+      \\ AP_TERM_TAC
+      \\ gvs [DRESTRICT_EQ_DRESTRICT]
+      \\ irule_at Any DOMSUB_SUBMAP
+      \\ fs [FDOM_DRESTRICT]
+      \\ irule_at Any SUBMAP_TRANS
+      \\ irule_at Any DRESTRICT_SUBMAP
+      \\ fs [DOMSUB_SUBMAP]
+      \\ qspecl_then [‘FDOM f’, ‘COMPL (set l)’, ‘v’] assume_tac DELETE_INTER
+      \\ fs [Once INTER_COMM]
+      \\ fs [GSYM DELETE_NON_ELEMENT])
+  \\ rename1 ‘_ e' = _ e'’
+  \\ PairCases_on ‘e'’
+  \\ fs []
+  >- (last_x_assum drule
+      \\ gvs [DRESTRICT_DOMSUB_COMM]
+      \\ rw []
+      \\ pop_assum irule
+      \\ rename1 ‘MEM (v2, e2) lcs’
+      \\ first_x_assum $ qspecl_then [‘freevars e2’] assume_tac
+      \\ fs [MEM_MAP]
+      \\ pop_assum $ qspecl_then [‘(v2, e2)’] assume_tac
+      \\ fs [])
+  >- (rename1 ‘DRESTRICT f (COMPL (set l))’
+      \\ AP_THM_TAC
+      \\ AP_TERM_TAC
+      \\ gvs [DRESTRICT_EQ_DRESTRICT]
+      \\ irule_at Any DOMSUB_SUBMAP
+      \\ fs [FDOM_DRESTRICT]
+      \\ irule_at Any SUBMAP_TRANS
+      \\ irule_at Any DRESTRICT_SUBMAP
+      \\ fs [DOMSUB_SUBMAP]
+      \\ qspecl_then [‘FDOM f’, ‘COMPL (set l)’, ‘v’] assume_tac DELETE_INTER
+      \\ fs [Once INTER_COMM]
+      \\ fs [GSYM DELETE_NON_ELEMENT])
+QED*)
+
+Theorem closed_subst2:
+  ∀v f e e'. (∀v. v ∈ FRANGE f ⇒ closed v) ⇒ closed e ⇒ freevars e' ⊆ FDOM f ⇒ (closed (subst f e') ∧ closed (subst1 v e (subst (f \\ v) e')))
+Proof
+  rw []
+  \\ rw [closed_def]
+  \\ ‘∀v2. v2 ∈ FRANGE (f \\ v) ⇒ closed v2’
+    by (rw []
+        \\ first_x_assum irule
+        \\ metis_tac [FRANGE_DOMSUB_SUBSET, SUBSET_DEF])
+  \\ dxrule freevars_subst
+  \\ dxrule freevars_subst
+  \\ dxrule freevars_subst1
+  \\ rw []
+  \\ gvs [SUBSET_DIFF_EMPTY, DELETE_DEF, SUBSET_DEF]
+  \\ rw []
+  \\ gvs []
+QED
+
+Theorem App_Let:
+  ∀v e e' e'' b. v ∉ freevars e'' ⇒ (App (Let v e e') e'' ≅? Let v e (App e' e'')) b
+Proof
+  rw []
+  \\ irule eval_wh_IMP_exp_eq
+  \\ rw []
+  \\ gvs [subst_def, eval_wh_thm]
+  \\ ‘∀v. v ∈ FRANGE f ⇒ closed v’ by gvs [FRANGE_FLOOKUP]
+  \\ ‘closed (subst f e)’ by gvs [closed_def, freevars_subst, SUBSET_DIFF_EMPTY]
+  \\ fs [bind1_def, subst1_def, eval_wh_App]
+  \\ IF_CASES_TAC
+  \\ fs []
+  \\ rename1 ‘(subst1 v (subst f e) (subst (f \\ v) e'))’
+  \\ Cases_on ‘dest_wh_Closure (eval_wh (subst1 v (subst f e) (subst (f \\ v) e')))’
+  \\ fs []
+  \\ rename1 ‘SOME x’
+  \\ PairCases_on ‘x’
+  \\ fs []
+  \\ qspecl_then [‘v’, ‘f’, ‘subst f e’, ‘e''’] assume_tac closed_subst2
+  \\ gvs []
+  \\ AP_TERM_TAC
+  \\ AP_THM_TAC
+  \\ AP_TERM_TAC
+  \\ AP_TERM_TAC
+  \\ fs []
+  \\ simp [GSYM subst_fdomsub]
+QED
+
+Theorem Apps_Let:
+  ∀l v e e' b. EVERY (λe. v ∉ freevars e) l ⇒ (Apps (Let v e e') l ≅? Let v e (Apps e' l)) b
+Proof
+  Induct
+  \\ fs [Apps_def, exp_eq_refl]
+  \\ rw []
+  \\ first_x_assum dxrule
+  \\ rw []
+  \\ dxrule App_Let
+  \\ strip_tac
+  \\ irule exp_eq_trans
+  \\ first_x_assum $ irule_at Any
+  \\ irule exp_eq_Apps_cong
+  \\ fs [exp_eq_l_refl]
+QED
+
+Theorem Apps_Lams_fold:
+  ∀l eL e b. EVERY (λx. EVERY (λe. x ∉ freevars e) eL) l ∧ LENGTH l = LENGTH eL ⇒
+             (Apps (Lams l e) eL ≅?  FOLDR (λ (id, e') e. Let id e' e) e (ZIP (l, eL))) b
+Proof
+  Induct
+  \\ fs [Lams_def, Apps_def, exp_eq_refl]
+  \\ gen_tac
+  \\ Cases
+  \\ fs [Apps_def, ZIP_def]
+  \\ rw []
+  \\ irule exp_eq_trans
+  \\ irule_at Any exp_eq_App_cong
+  \\ irule_at Any exp_eq_Lam_cong
+  \\ first_x_assum $ irule_at Any
+  \\ fs []
+  \\ irule_at Any Apps_Let
+  \\ gvs [exp_eq_refl, EVERY_CONJ]
+QED
+
+Theorem LetsSeq_com:
+  ∀l e e' b. (FOLDR (λ (id, e') e. Let id e' e) (Seq e e') l ≅?
+                 Seq (FOLDR (λ (id, e') e. Let id e' e) e l) (FOLDR (λ (id, e') e. Let id e' e) e' l)) b
+Proof
+  Induct
+  \\ fs [exp_eq_refl]
+  \\ Cases
+  \\ rw []
+  \\ irule exp_eq_trans
+  \\ irule_at Any exp_eq_App_cong
+  \\ irule_at Any exp_eq_Lam_cong
+  \\ pop_assum $ irule_at Any
+  \\ irule_at Any exp_eq_refl
+  \\ fs [Let_Seq]
+QED
+
+Theorem Apps_Lams_Seq_strong:
+  ∀l eL e p b. EVERY (λx. EVERY (λe. x ∉ freevars e) eL) l ∧ LENGTH l = LENGTH eL ⇒
+                     (Apps (Lams l (Seq p e)) eL ≅? Seq (Apps (Lams l p) eL) (Apps (Lams l e) eL)) b
+Proof
+  rw []
+  \\ irule exp_eq_trans
+  \\ irule_at Any Apps_Lams_fold
+  \\ fs []
+  \\ irule exp_eq_trans
+  \\ irule_at Any LetsSeq_com
+  \\ irule_at Any exp_eq_Prim_cong
+  \\ gvs [Apps_Lams_fold, exp_eq_sym]
+QED
+
+Theorem FoldLets_Projs:
+  ∀l ps e. FOLDR (λ(id, e1) e2. Let id e1 e2) (Projs ps e) l ≈ Projs ps (FOLDR (λ(id, e1) e2. Let id e1 e2) e l)
+Proof
+  Induct
+  \\ fs [exp_eq_refl]
+  \\ PairCases
+  \\ rw []
+  \\ irule exp_eq_trans
+  \\ irule_at Any Let_Projs
+  \\ irule exp_eq_App_cong
+  \\ gvs [exp_eq_refl, exp_eq_Lam_cong]
+QED
+
+Theorem ALL_DISTINCT_FLOOKUP:
+  ∀l k v. ALL_DISTINCT (MAP FST l) ∧ MEM (k, v) l ⇒ ∀f. FLOOKUP (f |++ l) k = SOME v
+Proof
+  Induct
+  \\ fs []
+  \\ PairCases
+  \\ rw []
+  \\ gvs [FUPDATE_FUPDATE_LIST_COMMUTES, FUPDATE_LIST_THM, FLOOKUP_UPDATE]
+  \\ IF_CASES_TAC
+  >- (gvs [MEM_EL]
+      \\ first_x_assum $ qspecl_then [‘n’] assume_tac
+      \\ qabbrev_tac ‘p = EL n l’
+      \\ PairCases_on ‘p’
+      \\ gvs [EL_MAP])
+  \\ first_x_assum irule
+  \\ fs []
+QED
+
+Theorem eta_red_fold:
+  ∀l f. ALL_DISTINCT (MAP FST l) ∧ EVERY (λv. v ∉ freevars f ∧ EVERY (λe. v ∉ freevars e) (MAP SND l)) (MAP FST l)
+        ⇒ FOLDR (λ (id, e1) e2. Let id e1 e2) (Apps f (MAP (Var o FST) l)) l ≈ Apps f (MAP SND l)
+Proof
+  Induct
+  \\ fs [exp_eq_refl]
+  \\ PairCases
+  \\ rw [Apps_def]
+  \\ irule exp_eq_trans
+  \\ irule_at Any exp_eq_App_cong
+  \\ irule_at Any exp_eq_Lam_cong
+  \\ first_x_assum $ irule_at Any
+  \\ gvs [EVERY_CONJ, EVERY_MEM]
+  \\ irule_at Any exp_eq_refl
+  \\ irule eval_wh_IMP_exp_eq
+  \\ rw [subst_Apps, subst_def, eval_wh_thm]
+  \\ rename1 ‘bind1 _ (subst f2 h1) _’
+  \\ ‘∀v. v ∈ FRANGE f2 ⇒ closed v’
+    by (rw [] \\ first_x_assum irule
+        \\ gvs [FRANGE_FLOOKUP]
+        \\ pop_assum $ irule_at Any)
+  \\ ‘closed (subst f2 h1)’
+    by (irule IMP_closed_subst
+        \\ fs [])
+  \\ qpat_x_assum ‘h0 ∉ freevars f’ assume_tac
+  \\ drule $ GSYM subst_fdomsub
+  \\ strip_tac
+  \\ gvs [bind1_def, subst_Apps, Once subst_subst1_UPDATE, subst_def, FLOOKUP_UPDATE, MAP_MAP_o]
+  \\ AP_TERM_TAC
+  \\ ‘subst1 h0 (subst f2 h1) (subst f2 f) = subst f2 f’
+    by (irule subst1_ignore
+        \\ gvs [freevars_subst])
+  \\ rw []
+  \\ AP_TERM_TAC
+  \\ irule LIST_EQ
+  \\ rw [EL_MAP]
+  \\ rename1 ‘EL n l’
+  \\ ‘h0 ∉ freevars (SND (EL n l))’ by
+    (last_x_assum irule
+     \\ gvs [MEM_EL]
+     \\ first_assum $ irule_at Any
+     \\ fs [EL_MAP])
+  \\ dxrule $ GSYM subst_fdomsub
+  \\ rw []
+  \\ irule subst1_ignore
+  \\ gvs [freevars_subst]
+  \\ DISJ1_TAC
+  \\ last_x_assum $ irule_at Any
+  \\ gvs [MEM_EL]
+  \\ first_assum $ irule_at Any
+  \\ fs [EL_MAP]
+QED
+
+(*Theorem fdemands_every_thing:
+  f fdemands ((ps, i), k, c) ⇔ (i < k ∧ ∀el. LENGTH el = k ⇒ (Apps f el) needs ((ps, EL i el), c))
+Proof
+  eq_tac
+  \\ rw [fdemands_def]
+  >- (rename1 ‘EL i eL’
+      \\ qspecl_then [‘freevars f ∪ s ∪ BIGUNION (set (MAP freevars eL))’, ‘LENGTH eL’] assume_tac exists_l_not_in_s
+      \\ ‘∀s. MEM s (MAP freevars eL) ⇒ FINITE s’ by (rw [MEM_EL] \\ gvs [EL_MAP])
+      \\ gvs [FINITE_UNION, freevars_FINITE, FINITE_BIGUNION]
+      \\ rename1 ‘ALL_DISTINCT l’
+      \\ first_x_assum $ qspecl_then [‘l’] assume_tac
+      \\ irule needs_exp_eq
+      \\ qexists_tac ‘Apps (Lams l (Apps f (MAP Var l))) eL’
+      \\ conj_tac
+      >- (gvs [needs_def, demands_def]
+          \\ irule exp_eq_in_ctxt_trans
+          \\ irule_at Any exp_eq_in_ctxt_Apps
+          \\ irule_at Any exp_eq_in_ctxt_l_refl
+          \\ irule_at Any exp_eq_in_ctxt_Lams
+          \\ pop_assum $ irule_at Any
+          \\ conj_tac
+          >- (irule $ iffLR SUBSET_EMPTY
+              \\ irule $ iffRL SUBSET_DEF
+              \\ gvs [IN_INTER, DISJ_EQ_IMP, EVERY_MEM])
+          \\ irule exp_eq_trans
+          \\ irule_at Any Apps_Lams_Seq_strong
+          \\ irule_at Any exp_eq_Prim_cong
+          \\ gvs [exp_eq_refl]
+          \\ irule_at Any exp_eq_trans
+          \\ irule_at Any Apps_Lams_fold
+          \\ irule_at Any exp_eq_trans
+          \\ irule_at Any FoldLets_Projs
+          \\ irule_at Any exp_eq_Projs_cong
+          \\ irule_at Any exp_eq_trans
+          \\ irule_at Any $ iffLR exp_eq_sym
+          \\ irule_at Any Apps_Lams_fold
+          \\ fs []
+          \\ conj_tac
+          >- (irule eval_wh_IMP_exp_eq
+              \\ gen_tac \\ rpt strip_tac
+              \\ qspecl_then [‘ZIP (l, MAP (subst f') eL)’, ‘subst (FDIFF f' (set l)) (Var (EL i l))’] assume_tac eval_Apps_Lams
+              \\ qabbrev_tac ‘kvl = ZIP (l, MAP (subst f') eL)’
+              \\ ‘ALL_DISTINCT (MAP FST kvl)’
+                by (unabbrev_all_tac
+                    \\ gvs [MAP_ZIP])
+              \\ dxrule ALL_DISTINCT_FLOOKUP
+              \\ strip_tac
+              \\ pop_assum $ qspecl_then [‘EL i l’, ‘subst f' (EL i eL)’, ‘FEMPTY’] assume_tac
+              \\ unabbrev_all_tac
+              \\ ‘MEM (EL i l, subst f' (EL i eL)) (ZIP (l, MAP (subst f') eL))’
+                by (gvs [MEM_EL]
+                    \\ qexists_tac ‘i’
+                    \\ gvs [EL_ZIP, EL_MAP])
+              \\ gvs [MAP_ZIP, subst_Apps, subst_Lams, subst_def, FLOOKUP_FDIFF, EL_MEM,
+                      EVERY_EL, EL_ZIP, BIGUNION_SUBSET, DISJOINT_EMPTY, FUPDATE_LIST, FLOOKUP_EMPTY]
+              \\ first_x_assum irule
+              \\ ‘∀v. v ∈ FRANGE f' ⇒ closed v’ by gvs [FRANGE_FLOOKUP]
+              \\ rw [EL_MAP, closed_def, freevars_subst, SUBSET_DIFF_EMPTY]
+              \\ first_x_assum $ irule_at Any
+              \\ gvs [MEM_MAP]
+              \\ irule_at Any EL_MEM
+              \\ pop_assum $ irule_at Any
+              \\ fs [])
+          \\ gvs [EVERY_MEM]
+          \\ rw []
+          \\ first_x_assum dxrule
+          \\ rw []
+          \\ pop_assum $ qspecl_then [‘freevars e’] assume_tac
+          \\ fs [MEM_MAP]
+          \\ pop_assum $ qspecl_then [‘e’] assume_tac
+          \\ gvs [])
+      \\ qspecl_then [‘ZIP (l, eL)’] assume_tac eta_red_fold
+      \\ irule exp_eq_trans
+      \\ irule_at Any Apps_Lams_fold
+      \\ gvs [MAP_ZIP]
+      \\ pop_assum $ irule_at Any
+      \\ gvs [EVERY_CONJ, EVERY_MEM]
+      \\ rw []
+      \\ first_x_assum drule
+      \\ rpt strip_tac
+      \\ first_x_assum $ qspecl_then [‘freevars e’] assume_tac
+      \\ gvs [MEM_MAP])
+  >- (qexists_tac ‘{}’
+      \\ rw []
+      \\ pop_assum $ qspecl_then [‘MAP Var l’] assume_tac
+      \\ gvs [EL_MAP, needs_Var_is_demands])
+QED*)
+
+Definition find_fdemands_def:
+  find_fdemands (fd: (string # ((string # num) list # num) # num) -> bool) (Var n) = {[], n} ∧
+  find_fdemands fd (Seq e1 e2) = find_fdemands fd e1 ∪ find_fdemands fd e2 ∧
+  find_fdemands fd (If e1 e2 e3) = find_fdemands fd e1 ∪
+                              (find_fdemands fd e2 ∩ find_fdemands fd e3) ∧
+  find_fdemands fd e = {}
+End
+
+(*Theorem find_fdemands_with_eval_to_soundness:
+  ∀e k fd. (∀n p len k2. (n, p, len) ∈ fd ∧ k2 ≤ k ⇒ (Var n) fdemands_depth (p, len, k2))
+           ⇒ ∀ps v. (ps, v) ∈ find_fdemands fd e
+                    ⇒ ∀f. freevars e ⊆ FDOM f ∧ is_bot (eval_wh_to k (subst f (Projs ps (Var v))))
+                          ⇒ is_bot (eval_wh_to k (subst f e))
+Proof
+  Induct using freevars_ind
+  \\ fs [find_fdemands_def, Projs_def]
+  \\ rename1 ‘Prim op es’
+  \\ Cases_on ‘op’
+  \\ Cases_on ‘es’
+  \\ fs [find_fdemands_def]
+  \\ rename1 ‘e1::tl’
+  \\ Cases_on ‘tl’
+  \\ fs [find_fdemands_def]
+  \\ rename1 ‘e1::e2::tl’
+  \\ Cases_on ‘tl’
+  \\ fs [find_fdemands_def]
+  >~ [‘Prim If (e1::e2::e3::t)’]
+  >- (Cases_on ‘t’
+      \\ fs [find_fdemands_def]
+      \\ rw []
+      \\ rename1 ‘(ps, v) ∈ find_fdemands fd e’
+      \\ last_assum $ qspecl_then [‘e’] assume_tac
+      \\ gvs []
+      \\ ‘∀n p len k2. (n, p, len) ∈ fd ∧ k2 ≤ (k - 1) ⇒ Var n fdemands_depth (p, len, k2)’
+        by (rw []
+            \\ first_x_assum irule
+            \\ gvs [])
+      \\ first_x_assum drule
+      \\ strip_tac
+      \\ pop_assum drule
+      \\ strip_tac
+      \\ pop_assum drule
+      \\ strip_tac
+      \\ ‘k - 1 ≤ k’ by fs []
+      \\ drule is_bot_continuous
+      \\ strip_tac
+      \\ pop_assum dxrule
+      \\ strip_tac
+      \\ fs [eval_wh_to_def, is_bot_def, subst_def]
+      \\ IF_CASES_TAC
+      \\ gvs []
+      \\ rename1 ‘_ = ec ∨ _ = et ∨ _ = ee’
+      \\ CASE_TAC \\ fs [] \\ rpt (IF_CASES_TAC \\ fs [])
+      \\ first_x_assum irule
+      \\ gvs []
+      \\ first_x_assum $ irule_at Any
+      \\ rw []
+      \\ first_x_assum $ irule_at Any
+      \\ gvs [])
+  \\ rw []
+  \\ rename1 ‘(ps, v) ∈ find_fdemands fd e’
+  \\ last_x_assum $ qspecl_then [‘e’] assume_tac
+  \\ fs []
+  \\ ‘∀n p len k2. (n, p, len) ∈ fd ∧ k2 ≤ (k - 1) ⇒ Var n fdemands_depth (p, len, k2)’
+        by (rw []
+            \\ first_x_assum irule
+            \\ gvs [])
+  \\ first_x_assum dxrule
+  \\ strip_tac
+  \\ pop_assum dxrule
+  \\ strip_tac
+  \\ pop_assum dxrule
+  \\ strip_tac
+  \\ ‘k - 1 ≤ k’ by fs []
+  \\ dxrule_then assume_tac is_bot_continuous
+  \\ pop_assum $ dxrule_then assume_tac
+  \\ gvs [eval_wh_to_def, is_bot_def, subst_def]
+  \\ Cases_on ‘k’
+  \\ fs []
+  \\ rename1 ‘if p = wh_Diverge ∨ p = wh_Error then _ else _’
+  \\ Cases_on ‘p’
+  \\ fs []
+QED*)
+
+(*Theorem find_fdemands_soundness:
+  ∀e fd. (∀n p k. (n, p, k) ∈ fd ⇒ (Var n) fdemands (p, k)) ⇒ ∀d. d ∈ find_fdemands fd e ⇒ e demands d
+Proof
+  Induct using freevars_ind
+  \\ fs [find_fdemands_def, demands_Var]
+  \\ rename1 ‘Prim op es’
+  \\ Cases_on ‘op’
+  \\ Cases_on ‘es’
+  \\ fs [find_fdemands_def]
+  \\ rename1 ‘e1::tl’
+  \\ Cases_on ‘tl’
+  \\ fs [find_fdemands_def]
+  \\ rename1 ‘e1::e2::tl’
+  \\ Cases_on ‘tl’
+  \\ fs [find_fdemands_def]
+  >~ [‘Prim If (e1::e2::e3::t)’]
+  >- (Cases_on ‘t’
+      \\ fs [find_fdemands_def]
+      \\ rw []
+      \\ rename1 ‘d ∈ find_fdemands fd e’
+      \\ last_assum $ qspecl_then [‘e’] assume_tac
+      \\ fs []
+      \\ pop_assum drule
+      \\ strip_tac
+      \\ pop_assum drule
+      \\ strip_tac
+      \\ fs [demands_If]
+      \\ rename1 ‘If ec et ee’
+      \\ last_x_assum $ qspecl_then [‘et’] assume_tac
+      \\ fs []
+      \\ pop_assum dxrule
+      \\ strip_tac
+      \\ pop_assum dxrule
+      \\ strip_tac
+      \\ fs [demands_If2])
+  \\ rw []
+  \\ rename1 ‘d ∈ find_fdemands fd e’
+  \\ last_x_assum $ qspecl_then [‘e’] assume_tac
+  \\ fs []
+  \\ pop_assum dxrule
+  \\ strip_tac
+  \\ pop_assum dxrule
+  \\ strip_tac
+  \\ fs [demands_Seq, demands_Seq2]
+QED*)
+
+Theorem demands_foldr:
+  ∀l c e ps v. e demands ((ps, v), FOLDL (λc2 (v, e1) . Bind v e1 c2) c l) ∧ ¬MEM v (MAP FST l)
+               ⇒ (FOLDR (λ(v, e1) e2. Let v e1 e2) e l) demands ((ps, v), c)
+Proof
+  Induct
+  \\ fs []
+  \\ PairCases
+  \\ rw []
+  \\ irule demands_Let2
+  \\ fs []
+QED
+
+(*Theorem demands_means_fdemands_lemma:
+  ∀l1 l2 e i ps c. i < LENGTH l1 ∧ LENGTH l1 = LENGTH l2
+    ∧ e demands ((ps, EL i l1), FOLDL (λc (v, e). Bind v e c) c (ZIP (l1, MAP Var l2)))
+    ∧ ALL_DISTINCT l1
+    ∧ EVERY (λv. ¬MEM v l2) l1 ∧ EVERY (λv. ¬MEM v l1) l2
+       ⇒ (FOLDR (λ(v1, e1) e2. Let v1 e1 e2) e (ZIP (l1, MAP Var l2))) demands ((ps, EL i l2), c)
+Proof
+  Induct
+  \\ fs []
+  \\ gen_tac
+  \\ Cases
+  \\ rw []
+  \\ rename1 ‘EL i (hd::tl)’
+  \\ Cases_on ‘i’
+  \\ gvs []
+  >- (irule demands_Let3
+      \\ irule_at Any demands_foldr
+      \\ gvs [MAP_ZIP])
+  \\ irule demands_Let2
+  \\ first_x_assum $ irule_at Any
+  \\ gvs [EL_MEM, EVERY_CONJ]
+  \\ strip_tac
+  \\ qpat_x_assum ‘¬MEM h tl’ irule
+  \\ gvs [EL_MEM]
+QED*)
+
+(*Theorem demands_means_fdemands:
+  ∀l e i ps. i < LENGTH l ∧ e demands ((ps, EL i l), FOLDL (λc v. IsFree v c) c l) ∧ ALL_DISTINCT l
+             ⇒ Lams l e fdemands ((ps, i), LENGTH l, c)
+Proof
+  rw [fdemands_def]
+  \\ qexists_tac ‘set l’
+  \\ fs [FINITE_LIST_TO_SET]
+  \\ rw []
+  \\ irule demands_exp_eq
+  \\ irule_at Any demands_means_fdemands_lemma
+  \\ irule_at Any $ iffLR exp_eq_in_ctxt_sym
+  \\ irule_at Any exp_eq_IMP_exp_eq_in_ctxt
+  \\ irule_at Any Apps_Lams_fold
+  \\ dxrule $ iffRL SUBSET_EMPTY
+  \\ strip_tac
+  \\ dxrule $ iffLR SUBSET_DEF
+  \\ strip_tac
+  \\ gvs [EVERY_MAP, IN_INTER, EVERY_MEM]
+  \\ irule_at Any demands_IsFree_List
+  \\ rw [MAP_ZIP]
+  \\ metis_tac []
+QED*)
+
+(*Theorem find_fdemands_Lambda_soundness:
+  ∀e l fname c. ALL_DISTINCT l ∧ i < LENGTH l ∧ (ps, EL i l) ∈ find_fdemands {} e
+                 ⇒ (Lams l e) fdemands ((ps, i), LENGTH l, c)
+Proof
+  rw []
+  \\ irule demands_means_fdemands
+  \\ fs []
+  \\ irule find_fdemands_soundness
+  \\ pop_assum $ irule_at Any
+  \\ gvs []
+QED*)
+
+Theorem is_bot_eval_wh_to_Apps:
+  ∀eL k f. is_bot (eval_wh_to k f) ⇒ is_bot (eval_wh_to k (Apps f eL))
+Proof
+  Induct
+  \\ rw []
+  \\ fs [Apps_def, eval_wh_to_def, is_bot_def]
+QED
+
+(*
+Theorem find_fdemands_Letrec:
+  ∀k e fd fname vL.ALL_DISTINCT vL ∧
+                   (∀n ps i l. (n, (ps, i), l) ∈ fd ⇒ l = LENGTH vL ∧ n = fname ∧ (ps, EL i vL) ∈ find_fdemands fd e)
+                 ⇒ ∀ps i. (ps, EL i vL) ∈ find_fdemands fd e
+                          ⇒ ∀f eL. is_bot (eval_wh_to k (subst f (Projs ps (EL i eL)))) ∧ LENGTH eL = LENGTH vL
+                                     ⇒ is_bot (eval_wh_to k (subst f (
+                                                              Apps
+                                                                (Letrec [(fname, Lams vL e)] (Var fname))
+                                                                eL)))
+Proof
+  Induct
+  >- (rw [subst_Apps, subst_def, subst_Lams, FLOOKUP_FDIFF]
+      \\ irule is_bot_eval_wh_to_Apps
+      \\ rw [eval_wh_to_def, is_bot_def])
+  \\
+*)
+
+(*Theorem find_fdemands_Letrec_soundness:
+  ∀e fd l fname. ALL_DISTINCT l
+              ∧ (∀n ps i k. (n, (ps, i), k) ∈ fd ∧ n = fname ⇒ k = LENGTH l ∧ (ps, EL i l) ∈ find_fdemands fd e)
+                 ⇒ ∀p k. (fname, p, k) ∈ fd ⇒ (Letrec [(fname, Lams l e)] (Var fname)) fdemands (p, k)
+Proof
+  rw []
+  \\ cheat
+QED*)
+
+Theorem Lam_require:
+  ∀l l' i h c.
+    LENGTH l = LENGTH l' ∧ ¬MEM h l ⇒
+    Apps (Lams l (Var h)) l' demands (([], h), c)
+Proof
+  Induct
+  \\ fs [Apps_def, Lams_def, demands_Var]
+  \\ gen_tac
+  \\ Cases
+  \\ rw [Apps_def]
+  \\ irule demands_exp_eq
+  \\ first_x_assum $ irule_at Any
+  \\ last_x_assum $ irule_at Any
+  \\ fs []
+  \\ irule exp_eq_IMP_exp_eq_in_ctxt
+  \\ irule exp_eq_Apps_cong
+  \\ fs [exp_eq_l_refl]
+  \\ irule eval_wh_IMP_exp_eq
+  \\ rw [subst_def, eval_wh_thm]
+  \\ AP_TERM_TAC
+  \\ ‘∀v. v ∈ FRANGE f ⇒ closed v’ by
+    (rw []
+     \\ first_x_assum irule
+     \\ fs [FRANGE_FLOOKUP]
+     \\ first_x_assum $ irule_at Any)
+  \\ ‘closed (subst f h')’ by gvs [freevars_subst, closed_def, SUBSET_DIFF_EMPTY]
+  \\ fs [bind1_def, subst_Lams, subst1_def, subst_def, FLOOKUP_FDIFF,
+         DOMSUB_FLOOKUP_NEQ, FLOOKUP_DEF]
+QED
+
+Theorem subst1_Lams:
+  ∀l h e e'. ¬ MEM h l ⇒ subst1 h e (Lams l e') = Lams l (subst1 h e e')
+Proof
+  Induct
+  \\ fs [Lams_def]
+  \\ rw [bind1_def, subst1_def]
+QED
+
+(*Theorem Lams_require_arg:
+  ∀l i.
+    ALL_DISTINCT l ∧ i < LENGTH l ⇒
+    Lams l (Var (EL i l)) fdemands (([], i), LENGTH l, c)
+Proof
+  Induct
+  \\ fs [Lams_def, fdemands_def]
+  \\ gen_tac
+  \\ Cases
+  \\ strip_tac
+  \\ gvs []
+  >- (Cases
+      \\ fs [Apps_def]
+      \\ strip_tac
+      \\ irule needs_exp_eq
+      \\ irule_at Any needs_Let1
+      \\ irule_at Any demands_Var
+      \\ irule_at Any Lam_require
+      \\ rename1 ‘MAP Var t’
+      \\ qspecl_then [‘l++t’] assume_tac exists_str_not_in_list
+      \\ fs [MEM_APPEND]
+      \\ qexists_tac ‘l’
+      \\ qexists_tac ‘MAP Var t’
+      \\ rename1 ‘MEM s t’
+      \\ first_assum $ irule_at Any
+      \\ fs [LENGTH_MAP, Once exp_eq_in_ctxt_sym]
+      \\ irule exp_eq_IMP_exp_eq_in_ctxt
+      \\ irule exp_eq_trans
+      \\ irule_at (Pos last) Apps_Let
+      \\ conj_tac
+      >- (rw [EVERY_EL, EL_MAP]
+          \\ strip_tac
+          \\ gvs [MEM_EL])
+      \\ irule exp_eq_Apps_cong
+      \\ fs [exp_eq_l_refl]
+      \\ irule eval_wh_IMP_exp_eq
+      \\ rw [subst_def, subst_Lams, eval_wh_thm, FLOOKUP_DEF]
+      \\ AP_TERM_TAC
+      \\ simp [bind1_def]
+      \\ rw [subst1_Lams, subst1_def])
+  \\ first_x_assum drule
+  \\ strip_tac
+  \\ first_x_assum $ irule_at Any
+  \\ Cases
+  \\ fs [Apps_def]
+  \\ strip_tac
+  \\ irule demands_exp_eq
+  \\ first_x_assum $ irule_at Any
+  \\ rename1 ‘h2 INSERT _’
+  \\ Cases_on ‘h2 ∈ s’
+  \\ gvs [INSERT_INTER]
+  \\ irule exp_eq_IMP_exp_eq_in_ctxt
+  \\ irule exp_eq_Apps_cong
+  \\ fs [exp_eq_l_refl]
+  \\ irule eval_wh_IMP_exp_eq
+  \\ rw []
+  \\ fs [MEM_EL, subst_def, eval_wh_thm, FLOOKUP_DEF, bind1_def]
+  \\ ‘closed (Lams l (Var (EL n' l)))’ by fs [closed_Lams, EL_MEM]
+  \\ fs [closed_subst]
+QED*)
+
+Theorem exists_diff_list_commute:
+  ∀(l : string list) s. FINITE s ⇒ ∃l'. LENGTH l = LENGTH l' ∧ ALL_DISTINCT l' ∧ EVERY (λv. v ∉ s ∧ ¬ MEM v l) l'
+Proof
+  Induct
+  \\ fs []
+  \\ rw []
+  \\ first_x_assum $ qspecl_then [‘s ∪ {h}’] assume_tac
+  \\ fs [FINITE_UNION, FINITE_SING]
+  \\ pop_assum drule
+  \\ rw []
+  \\ ‘INFINITE 𝕌(:string)’ by simp []
+  \\ ‘∃x. x ∉ set l' ∪ set l ∪ s ∪ {h}’ by
+    fs[pred_setTheory.NOT_IN_FINITE, FINITE_UNION, FINITE_SING]
+  \\ qexists_tac ‘x::l'’
+  \\ fs [EVERY_EL]
+QED*)
+
+Definition dest_fd_SND_def:
+  dest_fd_SND NONE = {} ∧
+  dest_fd_SND (SOME (bL, s)) = s
+End
+
+Definition demands_boolList_def:
+  demands_boolList d [] = ([], {}) ∧
+  demands_boolList d (hd::tl) =
+    let (bL, d2) = demands_boolList d tl in
+      (((∃ps. (ps, hd) ∈ d)∧ hd ∉ d2)::bL, d2 ∪ {hd})
+End
+
+Inductive find: (* i i i o o o *)
+[find_Drop_fd:]
+  (∀e e' c fds ds fd.
+     find e c fds ds e' fd ⇒ find e c fds ds e' NONE) ∧
+[find_smaller_fd:]
+  (∀e e' c fds ds bL fd fd'.
+     find e c fds ds e' (SOME (bL, fd)) ∧ fd' ⊆ fd
+     ⇒ find e c fds ds e' (SOME (bL, fd'))) ∧
 [find_Bottom:]
-  (∀e (c:ctxt).
-    find e c {} e) ∧
+  (∀e (c:ctxt) (fdc : (string # (bool list)) -> bool).
+    find e c fdc {} e NONE) ∧
 [find_Seq:]
-  (∀e e' c (p:(string#num) list) ds v.
-    find e c ds e' ∧ (p,v) ∈ ds ⇒
-    find e c ds (Seq (Var v) e')) ∧
+  (∀e e' c (p:(string#num) list) ds v fdc fd.
+    find e c fdc ds e' fd ∧ (p,v) ∈ ds ⇒
+    find e c fdc ds (Seq (Var v) e') fd) ∧
 [find_Seq2:]
-  (∀e e' e2 e2' c ds ds2.
-     find e c ds e' ∧ find e2 c ds2 e2' ⇒
-     find (Seq e e2) c (ds ∪ ds2) (Seq e' e2')) ∧
+  (∀e e' e2 e2' c ds ds2 fdc fd fd2.
+     find e c fdc ds e' fd ∧ find e2 c fdc ds2 e2' fd2 ⇒
+     find (Seq e e2) c fdc (ds ∪ ds2) (Seq e' e2') fd2) ∧
 [find_If:]
-  (∀ec et ee ec' et' ee' c dsc dst dse.
-     find ec c dsc ec' ∧
-     find et c dst et' ∧
-     find ee c dse ee' ⇒
-     find (If ec et ee) c (dsc ∪ (dst ∩ dse)) (If ec' et' ee')) ∧
+  (∀ec et ee ec' et' ee' c dsc dst dse fdc fd fdt fde.
+     find ec c fdc dsc ec' fd
+     ∧ find et c fdc dst et' fdt
+     ∧ find ee c fdc dse ee' fde
+     ⇒ find (If ec et ee) c fdc (dsc ∪ (dst ∩ dse)) (If ec' et' ee') NONE) ∧
 [find_Var:]
-  (∀n c. find (Var n) c {([],n)} (Var n)) ∧
+  (∀n c fdc. find (Var n) c fdc {([],n)} (Var n) NONE) ∧
+[find_Var2:]
+  (∀n c fdc argsDemanded.
+     (n, argsDemanded) ∈ fdc
+     ⇒ find (Var n) c fdc {([],n)} (Var n) (SOME (argsDemanded, {}))) ∧
+[find_No_args:]
+  (∀c fdc e e' ds ds'.
+     find e c fdc ds e' (SOME ([], ds'))
+     ⇒ find e c fdc (ds ∪ ds') e' NONE) ∧
 [find_App:]
-  (∀f f' e e' c ds ds2.
-     find f c ds f' ∧
-     find e c ds2 e' ⇒
-     find (App f e) c ds (App f' e')) ∧
+  (∀f f' e e' fdc c ds ds2 fd1 fd2.
+     find f c fdc ds f' fd1 ∧
+     find e c fdc ds2 e' fd2 ⇒
+     find (App f e) c fdc ds (App f' e') NONE) ∧
+[find_App_arg_strict:]
+  (∀f f' e e' fdc c ds ds2 ds3 fd argD.
+     find f c fdc ds f' (SOME (T::argD, ds3))
+     ∧ find e c fdc ds2 e' fd
+     ⇒ find (App f e) c fdc ds (App f' e') (SOME (argD, ds2 ∪ ds3))) ∧
+[find_App_arg_not_strict:]
+  (∀f f' e e' fdc c ds ds2 ds3 fd argD b.
+     find f c fdc ds f' (SOME (b::argD, ds3))
+     ∧ find e c fdc ds2 e' fd
+     ⇒ find (App f e) c fdc ds (App f' e') (SOME (argD, ds3))) ∧
 [find_Apps:]
-  (∀f f' el el' c ds.
-     LIST_REL (λe e'. ∃ds. find e c ds e') el el' ∧
-     find f c ds f' ⇒ find (Apps f el) c ds (Apps f' el')) ∧
+  (∀f f' el el' c ds fdc fd.
+     LIST_REL (λe e'. ∃ds fd. find e c fdc ds e' fd) el el' ∧
+     find f c fdc ds f' fd ⇒ find (Apps f el) c fdc ds (Apps f' el') NONE) ∧
+[find_Apps_fd:]
+  (∀f f' el el' c ds ds' fdc bL bL' fd dsL.
+     LIST_REL (λe (ds, e'). ∃ fd. find e c fdc ds e' fd) el (ZIP (dsL, el'))
+     ∧ LENGTH el' = LENGTH bL ∧ LENGTH dsL = LENGTH el'
+     ∧ find f c fdc ds f' (SOME (bL ++ bL', fd))
+     ∧ (∀p. p ∈ ds' ⇒ p ∈ fd ∨ ∃i. i < LENGTH bL ∧ p ∈ EL i dsL ∧ EL i bL)
+     ⇒ find (Apps f el) c fdc ds (Apps f' el') (SOME (bL', ds'))) ∧
 [find_Prim:]
-  (∀c el el' ope.
-     LENGTH el = LENGTH el' ∧ (∀k. k < LENGTH el ⇒ ∃ds. find (EL k el) c ds (EL k el') )
-     ⇒ find (Prim ope el) c {} (Prim ope el')) ∧
+  (∀c el el' ope fdc.
+     LENGTH el = LENGTH el' ∧ (∀k. k < LENGTH el ⇒ ∃ds fd. find (EL k el) c fdc ds (EL k el') fd)
+     ⇒ find (Prim ope el) c fdc {} (Prim ope el') NONE) ∧
 [find_Prim1:]
-  (∀c el el' ope ds.
-     LENGTH el = LENGTH el' ∧
-     (∀k. k < LENGTH el ⇒ ∃ds'. find (EL k el) c ds' (EL k el')) (* Rewritte with LIST_REL *)
-     ∧ find (EL 0 el) c ds (EL 0 el') ∧ el ≠ [] ∧ well_formed ope el ⇒ find (Prim ope el) c ds (Prim ope el')) ∧
+  (∀c el el' ope ds fdc fd.
+      LIST_REL (λe e'. ∃ds2 fd2. find e c fdc ds2 e' fd2) el el'
+      ∧ find (EL 0 el) c fdc ds (EL 0 el') fd ∧ el ≠ [] ∧ well_formed ope el
+      ⇒ find (Prim ope el) c fdc ds (Prim ope el') NONE) ∧
 [find_Prim_Fail:]
-  (∀c el ope.
-     ¬ (well_written ope el) ⇒ find (Prim ope el) c {} Fail) ∧
+  (∀c el ope fdc.
+     ¬ (well_written ope el) ⇒ find (Prim ope el) c fdc {} Fail NONE) ∧
 [find_Proj:]
-  (∀e e' n i c ds.
-     find e c ds e' ⇒ find (Proj n i e) c ds (Proj n i e')) ∧
+  (∀e e' n i c ds fdc fd.
+     find e c fdc ds e' fd ⇒ find (Proj n i e) c fdc ds (Proj n i e') NONE) ∧
 [find_IsEq:]
-  (∀e e' n i c ds.
-     find e c ds e' ⇒ find (IsEq n i e) c ds (IsEq n i e')) ∧
+  (∀e e' n i b c ds fdc fd.
+     find e c fdc ds e' fd ⇒ find (IsEq n i b e) c fdc ds (IsEq n i b e') NONE) ∧
 [find_Atom:]
-  (∀el dsl el' c op.
+  (∀el dsl el' fdc c op fd.
      LENGTH dsl = LENGTH el' ∧
-     LIST_REL (λe (ds, e'). find e c ds e') el (ZIP (dsl, el')) ⇒
-     find (Prim (AtomOp op) el) c (BIGUNION (set dsl)) (Prim (AtomOp op) el')) ∧
+     LIST_REL (λe (ds, e'). find e c fdc ds e' fd) el (ZIP (dsl, el')) ⇒
+     find (Prim (AtomOp op) el) c fdc (BIGUNION (set dsl)) (Prim (AtomOp op) el') NONE) ∧
 [find_Subset:]
-  (∀e e' c ds ds'.
-     find e c ds e' ∧ (∀ps v. (ps, v) ∈ ds' ⇒ ∃ps'. (ps++ps', v) ∈ ds) ⇒ find e c ds' e') ∧
+  (∀e e' c ds ds' fdc fdc' fd.
+     find e c fdc' ds e' fd
+     ∧ (∀ps v. (ps, v) ∈ ds' ⇒ ∃ps'. (ps++ps', v) ∈ ds)
+     ∧ fdc' ⊆ fdc
+     ⇒ find e c fdc ds' e' fd) ∧
 [find_Let:]
-  (∀e e' e2 e2' ds ds' c v.
-     find e c ds e' ∧ find e2 (Bind v e c c) ds' e2'
+  (∀e e' e2 e2' ds ds' c v fdc fdc' fd fd'.
+     find e c fdc ds e' fd ∧ find e2 (Bind v e c) fdc' ds' e2' fd'
      ∧ (∀ps. (ps, v) ∉ ds')
-     ⇒ find (Let v e e2) c ds' (Let v e' e2')) ∧
+     ∧ (∀n argDemands. (n, argDemands) ∈ fdc'
+                       ⇒ (n ≠ v ∧ (n, argDemands) ∈ fdc)
+                         ∨ (n = v ∧ ∃dset. SOME (argDemands, dset) = fd))
+     ∧ (∀l. (l, v) ∉ dest_fd_SND fd')
+     ⇒ find (Let v e e2) c fdc ds' (Let v e' e2') fd') ∧
 [find_Let2:]
-  (∀ e e' e2 e2' ds ds' ds'' c v ps.
-     find e c ds e' ∧ find e2 (Bind v e c c) ds' e2'
+  (∀ e e' e2 e2' ds ds' ds'' c v ps fdc fdc' fd fd'.
+     find e c fdc ds e' fd ∧ find e2 (Bind v e c) fdc' ds' e2' fd'
      ∧ (ps,v) ∈ ds'
      ∧ (∀ps' v'. (ps', v') ∈ ds'' ⇒ ((ps', v') ∈ ds' ∧ v' ≠ v) ∨ (ps', v') ∈ ds)
-     ⇒ find (Let v e e2) c ds'' (Let v e' e2')) ∧
+     ∧ (∀n argDemands. (n, argDemands) ∈ fdc'
+                       ⇒ (n ≠ v ∧ (n, argDemands) ∈ fdc)
+                         ∨ (n = v ∧ ∃dset. SOME (argDemands, dset) = fd))
+     ∧ (∀l. (l, v) ∉ dest_fd_SND fd')
+     ⇒ find (Let v e e2) c fdc ds'' (Let v e' e2') fd') ∧
 [find_Lam:]
-  (∀e e' c ds v.
-     find e c ds e' ⇒ find (Lam v e) c {} (Lam v e')) ∧
+  (∀e e' c ds v fdc fd.
+     find e (IsFree v c) fdc ds e' fd ∧ (∀argDs. (v, argDs) ∉ fdc)
+     ⇒ find (Lam v e) c fdc {} (Lam v e') NONE) ∧
 [find_Lams:]
-  (∀e e' c ds vl.
-     find e (FOLDL (λc n. IsFree n c) c vl) ds e' ⇒ find (Lams vl e) c {} (Lams vl e')) ∧
+  (∀e e' c ds vl fdc fd.
+     find e (FOLDL (λc n. IsFree n c) c vl) fdc ds e' fd
+     ∧ EVERY (λv. ∀argDs. (v, argDs) ∉ fdc) vl
+     ⇒ find (Lams vl e) c fdc {} (Lams vl e') NONE ) ∧
+[find_Lams_fd:]
+  (∀e e' c ds vl fdc.
+     find e (FOLDL (λc n. IsFree n c) c vl) fdc ds e' NONE
+     ∧ EVERY (λv. ∀argDs. (v, argDs) ∉ fdc) vl
+     ∧ bL
+     ⇒ find (Lams vl e) c fdc {} (Lams vl e') (SOME (FST (demands_boolList ds vl), {}))) ∧
 [find_Eq:]
-  (∀e e' c. e ≈ e' ⇒ find e c {} e') ∧
+  (∀e1 e2 e3 c fdc ds fd.
+     exp_eq_in_ctxt c e1 e2
+     ∧ find e2 c fdc ds e3 fd
+     ⇒ find e1 c fdc ds e3 fd) ∧
 [find_Letrec:]
-  (∀e e' ds c b b'. LIST_REL (λ(n1, e1) (n2, e2). n1 = n2 ∧ e1 ≈ e2) b b' ∧ find e (RecBind b c) ds e' ⇒ find (Letrec b e) c {} (Letrec b e'))
+  (∀e e' ds ds' c b b' fdc fdc' fd dsL fdL.
+     LENGTH b = LENGTH dsL ∧ LENGTH b = LENGTH b' ∧ LENGTH b = LENGTH fdL
+     ∧ (∀i. i < LENGTH b
+            ⇒ FST (EL i b') = FST (EL i b)
+              ∧ find (SND (EL i b)) Nil {}  (EL i dsL) (SND (EL i b')) (EL i fdL))
+     ∧ find e (RecBind b c) fdc' ds e' fd
+     ∧ EVERY (λv. (∀argDs. (v, argDs) ∉ fdc) ∧ (∀ps. (ps, v) ∉ dest_fd_SND fd)) (MAP FST b)
+     ∧ (∀v argDs. (v, argDs) ∈ fdc' ⇒
+                  (v, argDs) ∈ fdc
+                  ∨ (∃i fdSet. FST (EL i b) = v ∧ i < LENGTH b ∧ EL i fdL = SOME (argDs, fdSet)))
+     ∧ (∀ps v. (ps, v) ∈ ds'
+               ⇒ ¬MEM v (MAP FST b)
+                 ∧ ((ps, v) ∈ ds
+                    ∨ (∃ps' i. i < LENGTH b ∧ (ps', FST (EL i b)) ∈ ds ∧ (ps, v) ∈ EL i dsL)))
+     ∧ ALL_DISTINCT (MAP FST b)
+     ⇒ find (Letrec b e) c fdc ds' (Letrec b' e') fd)
 End
-
 
 fun apply_to_first_n 0 tac = ALL_TAC
   | apply_to_first_n n tac = apply_to_first_n (n-1) tac >- tac;
 
+(*Theorem Let_Let_nothing:
+  ∀e s v b. v ≠ s ∧ s ∉ freevars e ⇒ (Let s (Var v) (Let v (Var s) e) ≅? e) b
+Proof
+  Induct using freevars_ind >> rpt strip_tac
+  >~[‘Let s _ (Let v _ (Var n))’]
+  >- (irule eval_IMP_exp_eq >>
+      rw [Once eval_thm, subst_def] >>
+      Cases_on ‘FLOOKUP f v’
+      >~[‘FLOOKUP f v = NONE’] >- gvs [FLOOKUP_DEF] >>
+      first_assum $ drule_then assume_tac >>
+      Cases_on ‘n = v’ >>
+      gvs [eval_thm, bind1_def, subst1_def, DOMSUB_FLOOKUP, DOMSUB_FLOOKUP_NEQ, FLOOKUP_UPDATE] >>
+      Cases_on ‘FLOOKUP f n’ >> gvs [FLOOKUP_DEF])
+  >~[‘Prim’]
+  >- (irule exp_eq_trans >>
+      irule_at Any exp_eq_App_cong >> irule_at Any exp_eq_Lam_cong >>
+      irule_at Any Let_Prim >> irule_at Any exp_eq_refl >>
+      irule_at Any exp_eq_trans >> irule_at Any Let_Prim >>
+      irule exp_eq_Prim_cong >> rw [LIST_REL_EL_EQN, EL_MAP] >>
+      last_x_assum irule >> gvs [EL_MEM] >>
+      rename1 ‘EL n es’ >> last_x_assum $ qspecl_then [‘freevars (EL n es)’] assume_tac >> fs [] >>
+      strip_tac >> first_x_assum irule >> gvs [MEM_EL] >>
+      first_assum $ irule_at Any >> fs [EL_MAP])
+  >~[‘Let s _ (Let v _ (App _ _))’]
+  >- (irule exp_eq_trans >>
+      irule_at (Pos hd) exp_eq_App_cong >> irule_at Any exp_eq_Lam_cong >>
+      irule_at Any Let_App >> irule_at Any exp_eq_refl >>
+      irule exp_eq_trans >> irule_at Any Let_App >>
+      fs [exp_eq_App_cong])
+  >~[‘Let s _ (Let v _ (Lam n e))’]
+  >- (Cases_on ‘v = n’ >> rw []
+      >~[‘Let _ _ (Let v _ (Lam v e))’]
+      >- (irule exp_eq_trans >>
+          irule_at Any exp_eq_App_cong >> irule_at (Pos hd) exp_eq_Lam_cong >>
+          irule_at (Pos $ el 2) exp_eq_refl >>
+          qexists_tac ‘Lam v e’ >> conj_tac >>
+          irule eval_IMP_exp_eq >> rw [Ntimes subst_def 2] >>
+          rename1 ‘subst (f \\ _)’ >> qspecl_then [‘f’, ‘Lam v e’] assume_tac $ GSYM subst_fdomsub >>
+          gvs [eval_thm, bind1_def, subst1_ignore, IMP_closed_subst, FRANGE_FLOOKUP]) >>
+      ‘∃s2. s2 ∉ freevars (Lam n e) ∪ {n} ∪ {v} ∪ {s} ’
+        by (‘INFINITE 𝕌(:string)’ by simp [] >> gvs [NOT_IN_FINITE]) >>
+      irule exp_eq_trans >> irule_at Any exp_eq_App_cong >>
+      irule_at (Pos hd) exp_alpha_exp_eq >> irule_at Any exp_alpha_Alpha >>
+      qexists_tac ‘s2’ >> once_rewrite_tac [perm_exp_def] >> irule_at Any exp_eq_refl >>
+      irule_at Any exp_eq_trans >> irule_at Any exp_eq_App_cong >>
+      irule_at (Pos hd) exp_eq_Lam_cong >> irule_at (Pos hd) exp_eq_App_cong >>
+      once_rewrite_tac [perm_exp_def] >>
+      irule_at (Pos hd) exp_eq_Lam_cong >> irule_at (Pos hd) $ iffLR exp_eq_sym >>
+      irule_at (Pos hd) exp_alpha_exp_eq >> irule_at (Pos hd) exp_alpha_perm_irrel >>
+      rpt $ irule_at Any exp_eq_refl >> gvs [perm_exp_def, perm1_def] >>
+      irule exp_eq_trans >>
+      irule_at Any exp_eq_App_cong >> irule_at (Pos hd) exp_eq_Lam_cong >>
+      irule_at Any Let_Lam_weak >> irule_at Any exp_eq_refl >>
+      irule_at Any exp_eq_trans >> irule_at Any Let_Lam_weak >>
+      irule_at Any exp_eq_Lam_cong >> last_x_assum $ irule_at Any >>
+      gvs [])
+  >~[‘Let s _ (Let w _ (Letrec lcs _))’]
+  >- (Cases_on ‘MEM w (MAP FST lcs)’
+      >~[‘¬MEM w (MAP FST lcs)’]
+      >- (‘∃s2. s2 ∉ freevars e ∪ BIGUNION (set (MAP freevars (MAP SND lcs)))
+                   ∪ {w} ∪ set (MAP FST lcs) ∪ {s}’
+            by (‘INFINITE 𝕌(:string)’ by simp [] >>
+                dxrule_then irule $ iffLR NOT_IN_FINITE >>
+                gvs [NOT_IN_FINITE, FINITE_BIGUNION, MEM_MAP] >>
+                rw [] >> fs [freevars_FINITE]) >>
+          irule exp_eq_trans >> irule_at Any exp_eq_App_cong >>
+          irule_at (Pos hd) exp_alpha_exp_eq >> irule_at Any exp_alpha_Alpha >>
+          qexists_tac ‘s2’ >> once_rewrite_tac [perm_exp_def] >> irule_at Any exp_eq_refl >>
+          irule_at Any exp_eq_trans >> irule_at Any exp_eq_App_cong >>
+          irule_at (Pos hd) exp_eq_Lam_cong >> irule_at (Pos hd) exp_eq_App_cong >>
+          once_rewrite_tac [perm_exp_def] >>
+          irule_at (Pos hd) exp_eq_Lam_cong >> irule_at (Pos hd) $ iffLR exp_eq_sym >>
+          irule_at (Pos hd) exp_alpha_exp_eq >> irule_at (Pos hd) exp_alpha_perm_irrel >>
+          rpt $ irule_at Any exp_eq_refl >> first_x_assum $ irule_at (Pos hd) >>
+          gvs [perm_exp_def, perm1_def, MAP_MAP_o, combinTheory.o_DEF, LAMBDA_PROD] >>
+          irule exp_eq_trans >>
+          irule_at Any exp_eq_App_cong >> irule_at Any exp_eq_Lam_cong >>
+          irule_at Any Let_Letrec2 >> irule_at Any exp_eq_refl >>
+          irule_at (Pos last) exp_eq_trans >> irule_at (Pos hd) Let_Letrec2 >>
+          irule_at Any exp_eq_Letrec_cong2 >>
+          first_x_assum $ irule_at (Pos $ el 2) >>
+          irule_at Any fmap_rel_FUPDATE_LIST_same >> irule_at Any LIST_EQ >>
+          irule_at Any $ iffRL LIST_REL_EL_EQN >>
+          gvs [EL_MAP, EVERY_EL, MEM_EL] >>
+          rw [] >> rename1 ‘n < LENGTH lcs’ >> qabbrev_tac ‘p = EL n lcs’ >> PairCases_on ‘p’ >> gvs [EL_MAP]
+          >- (last_x_assum irule >> first_assum $ irule_at Any >> gvs [] >>
+              first_x_assum $ qspecl_then [‘freevars p1’] assume_tac >> fs [] >>
+              pop_assum $ qspecl_then [‘n’] assume_tac >> gvs [EL_MAP])
+          >- (strip_tac >> first_x_assum $ qspecl_then [‘n’] assume_tac >> gvs [EL_MAP])
+          >- (strip_tac >> last_x_assum $ qspecl_then [‘n’] assume_tac >> gvs [EL_MAP])
+          >- (strip_tac >> first_x_assum $ qspecl_then [‘n’] assume_tac >> gvs [EL_MAP]))
+      >- (irule exp_eq_trans >> irule_at Any exp_eq_App_cong >> irule_at (Pos hd) exp_eq_Lam_cong >>
+          irule_at (Pos $ el 2) exp_eq_refl >>
+          qexists_tac ‘Letrec lcs e’ >> conj_tac >>
+          irule eval_IMP_exp_eq >> rw [Ntimes subst_def 2] >>
+          rename1 ‘subst (f \\ _ )’ >> qspecl_then [‘f’, ‘Letrec lcs e’] assume_tac $ GSYM subst_fdomsub >>
+          gvs [eval_thm, bind1_def, subst1_ignore, IMP_closed_subst, FRANGE_FLOOKUP]))
+QED
+
+Theorem demands_Apps2:
+  ∀d v e e2 eL v c.
+    (∀eL'. LENGTH eL' = LENGTH eL ⇒ Apps e2 eL' demands (d, Bind v e c)) ∧ v ≠ SND d
+    ⇒ Apps (Let v e e2) eL demands (d, c)
+Proof
+  PairCases >> rw [GSYM needs_Var_is_demands, needs_def, exp_eq_in_ctxt_def] >>
+  ‘∃s. s ∉ freevars (Let v e e2) ∪ {d1} ∪ BIGUNION (set (MAP freevars eL)) ∪ {v}’
+    by (‘INFINITE 𝕌(:string)’ by simp [] >>
+        dxrule_then irule $ iffLR NOT_IN_FINITE >>
+        gvs [NOT_IN_FINITE, FINITE_BIGUNION, MEM_MAP] >> rw [] >> fs [freevars_FINITE]) >>
+  irule exp_eq_in_ctxt_trans >> irule_at Any exp_eq_in_ctxt_Apps >>
+  qexists_tac ‘MAP (λe. Let s (Var v) e) (MAP (λe. Let v (Var s) e) eL)’ >>
+  qexists_tac ‘(Let s (Var v) (Let v e e2))’ >>
+  conj_asm1_tac
+  >- (rw [LIST_REL_EL_EQN, EL_MAP] >>
+      irule exp_eq_IMP_exp_eq_in_ctxt >> irule $ iffLR exp_eq_sym >>
+      irule Let_Let_nothing >> gvs [] >>
+      rename1 ‘EL n eL’ >> first_x_assum $ qspecl_then [‘freevars (EL n eL)’] assume_tac >>
+      gvs [MEM_MAP] >> pop_assum $ qspecl_then [‘EL n eL’] assume_tac >> gvs [MEM_EL]) >>
+  conj_asm1_tac
+  >- (irule exp_eq_IMP_exp_eq_in_ctxt >> irule $ iffLR exp_eq_sym >> irule eval_IMP_exp_eq >>
+      rw [Ntimes subst_def 2] >>
+      rename1 ‘subst (f \\ _ )’ >> qspecl_then [‘f’, ‘Let v e e2’] assume_tac $ GSYM subst_fdomsub >>
+      gvs [eval_thm, bind1_def, subst1_ignore, IMP_closed_subst, FRANGE_FLOOKUP]) >>
+  irule exp_eq_in_ctxt_trans >> irule_at (Pos hd) $ iffLR exp_eq_in_ctxt_sym >>
+  irule_at Any Let_Apps_in_ctxt >>
+QED*)
+
+Theorem concat_Nil:
+  ∀c. concat_ctxt c Nil = c
+Proof
+  Induct >> gvs [concat_ctxt_def]
+QED
+
+Theorem concat_FOLDL_IsFree:
+  ∀vL c1 c2. FOLDL (λc n. IsFree n c) (concat_ctxt c1 c2) vL = concat_ctxt (FOLDL (λc n. IsFree n c) c1 vL) c2
+Proof
+  Induct >> gvs [GSYM concat_ctxt_def]
+QED
+
+Theorem demands_when_applied_exp_eq:
+  ∀d e1 e2 len c. exp_eq_in_ctxt c e1 e2 ∧ e1 demands_when_applied (d, len, c)
+                  ⇒ e2 demands_when_applied (d, len, c)
+Proof
+  PairCases >> rw [demands_when_applied_def] >>
+  irule eq_when_applied_trans_exp_eq >>
+  irule_at Any $ iffLR exp_eq_in_ctxt_sym >> last_assum $ irule_at Any >>
+  irule eq_when_applied_trans >> pop_assum $ irule_at Any >>
+  irule exp_eq_in_ctxt_IMP_eq_when_applied >>
+  irule exp_eq_in_ctxt_Prim >> gvs [exp_eq_in_ctxt_refl]
+QED
+
+Theorem demands_boolList_soundness:
+  ∀vL ds ds2 bL. demands_boolList ds vL = (bL, ds2)
+                 ⇒ (∀h. MEM h vL ⇔ h ∈ ds2) ∧ LENGTH bL = LENGTH vL
+                   ∧ ∀i. i < LENGTH vL ∧ EL i bL ⇒
+                         (∃ps. (ps, EL i vL) ∈ ds)
+                         ∧  ∀e ps c. e demands ((ps, EL i vL), FOLDL (λc n. IsFree n c) c vL)
+                                     ⇒ Lams vL e fdemands ((ps, i), LENGTH vL, c)
+Proof
+  Induct >> gvs [demands_boolList_def, PAIR] >> rw [] >>
+  rename1 ‘demands_boolList ds vL’ >>
+  qabbrev_tac ‘p = demands_boolList ds vL’ >> PairCases_on ‘p’ >> gvs [] >>
+  last_x_assum $ dxrule_then assume_tac >> gvs [Lams_def]
+  >- (eq_tac >> rw [] >> gvs []) >>
+  rename1 ‘i < SUC _’ >> Cases_on ‘i’
+  >>~[‘0 < SUC _’]
+  >- (gvs [] >> first_x_assum $ irule_at Any)
+  >- (irule Lam_fdemands >> gvs [GSYM demands_when_applied_0] >>
+      dxrule_then assume_tac demands_when_applied_Lams >>
+      gvs [])
+  >- gvs []
+  >- (irule fdemands_Lam >> gvs [])
+QED
+
 Theorem find_soundness_lemma:
-  ∀e c ds e'. find e c ds e'  ⇒
-                e ≈ e' ∧
-                (∀d. d ∈ ds ⇒ e demands d)
+  ∀e c fdc ds e' fd. find e c fdc ds e' fd
+    ⇒ (∀n l i c2. (n, l) ∈ fdc ∧ i < LENGTH l ∧ EL i l ⇒ (Var n) fdemands (([], i), LENGTH l, concat_ctxt c c2))
+    ⇒ exp_eq_in_ctxt c e e' ∧ (∀d. d ∈ ds ⇒ e demands (d, c))
+      ∧ (∀argDs ds2.
+           fd = SOME (argDs, ds2)
+           ⇒ (∀i c2. i < LENGTH argDs ∧ EL i argDs ⇒ e' fdemands (([], i), LENGTH argDs, concat_ctxt c c2))
+             ∧ ∀d2. d2 ∈ ds2 ⇒  e' demands_when_applied (d2, LENGTH argDs, c))
+(*           ∧ ∀eL d2. (LENGTH eL = LENGTH argDs ∧ d2 ∈ ds2) ⇒ (Apps e' eL) demands (d2, c))*)
 Proof
   Induct_on ‘find’
   \\ rpt conj_tac
   \\ rpt gen_tac
-  >- fs [exp_eq_refl] (* find_Bottom *)
-  >~[‘e ≈ Seq (Var v) e2’] (* find_Seq *)
+  \\ gvs [exp_eq_in_ctxt_refl, demands_Var]
+  >~[‘exp_eq_in_ctxt c e (Seq (Var v) e2)’] (* find_Seq *)
   >- (strip_tac
       \\ strip_tac
       \\ fs []
       \\ first_x_assum $ drule
+      \\ strip_tac \\ conj_asm1_tac
+      >- (dxrule_then assume_tac demands_empty_Projs
+          \\ fs [demands_def, Projs_def]
+          \\ irule exp_eq_in_ctxt_trans
+          \\ pop_assum $ irule_at Any
+          \\ irule exp_eq_in_ctxt_Prim
+          \\ fs [exp_eq_in_ctxt_refl])
       \\ rw []
-      \\ dxrule_then assume_tac demands_empty_proj
-      \\ fs [demands_def, Projs_def]
-      \\ irule exp_eq_trans
-      \\ first_assum $ irule_at Any
-      \\ irule exp_eq_Prim_cong
-      \\ fs [exp_eq_refl])
-  >~[‘Seq e e2 ≈ Seq e' e2'’] (* find_Seq2 *)
+      >- (first_x_assum $ drule_then assume_tac
+          \\ gvs [fdemands_Seq])
+      >- gvs [demands_when_applied_Seq])
+  >~[‘exp_eq_in_ctxt c (Seq e e2) (Seq e' e2')’] (* find_Seq2 *)
   >- (rw []
-      \\ fs [exp_eq_Prim_cong, demands_Seq, demands_Seq2])
-  >~[‘If ec et ee ≈ If ec' et' ee'’]
-  >- (rw []
-      \\ fs [demands_If, demands_If2, exp_eq_Prim_cong])
-  >~[‘Var n ≈ Var n’] (* find_Var *)
-  >- fs [exp_eq_refl, demands_Var]
-  >~[‘App f e ≈ App f' e'’] (* find_App *)
-  >- (rw []
-      \\ fs [exp_eq_App_cong, demands_App])
-  >~[‘Apps e el' ≈ Apps e' el''’]
+      \\ gvs [exp_eq_in_ctxt_Prim, demands_Seq, demands_Seq2, fdemands_Seq,
+             demands_when_applied_Seq])
+  >~[‘exp_eq_in_ctxt c (If ec et ee) (If ec' et' ee')’]
+  >- (rw [] \\ fs [exp_eq_in_ctxt_Prim, demands_If, demands_If2])
+  >~[‘_ demands_when_applied (_, 0, _)’]
+  >- (rw [] \\ gvs [demands_when_applied_0]
+      \\ irule demands_exp_eq
+      \\ metis_tac [exp_eq_in_ctxt_sym])
+  >~[‘exp_eq_in_ctxt c (App f e) (App f' e')’] (* find_App *)
+  >- (rw [] \\ fs [exp_eq_in_ctxt_App, demands_App])
+  >>~[‘exp_eq_in_ctxt c (Apps e el') (Apps e' el'')’] (* find_Apps *)
   >- (rw []
       \\ fs [Apps_demands]
-      \\ irule exp_eq_Apps_cong
-      \\ fs [LIST_REL_EL_EQN]
-      \\ rw []
+      \\ assume_tac exp_eq_in_ctxt_Apps
+      \\ irule exp_eq_in_ctxt_Apps
+      \\ fs [LIST_REL_EL_EQN] \\ rw []
+      \\ rename1 ‘n < LENGTH _’
       \\ first_x_assum $ qspecl_then [‘n’] assume_tac
       \\ metis_tac [])
-  >~[‘Proj n i e ≈ Proj n i e'’] (* find_Proj *)
+  >- (rw [] (* find_Apps_fd *)
+      >- (irule exp_eq_in_ctxt_Apps
+          \\ fs [LIST_REL_EL_EQN] \\ rw []
+          \\ rename1 ‘n < LENGTH _’ \\ last_x_assum $ qspecl_then [‘n’] assume_tac
+          \\ gvs [EL_ZIP])
+      \\ first_x_assum $ dxrule_then assume_tac
+      \\ gvs [Apps_demands, LIST_REL_EL_EQN, demands_when_applied_Apps]
+      >- (irule fdemands_Apps \\ gvs [Once ADD_SYM]
+          \\ first_x_assum irule
+          \\ gvs [EL_APPEND_EQN])
+      \\ irule demands_when_applied_Apps2
+      \\ rename1 ‘i < LENGTH _’ \\ first_x_assum $ qspecl_then [‘i’, ‘Nil’] assume_tac
+      \\ gvs [EL_ZIP, EL_APPEND_EQN, concat_Nil]
+      \\ first_x_assum $ irule_at Any
+      \\ last_x_assum $ drule_then assume_tac \\ gvs []
+      \\ irule demands_exp_eq
+      \\ rpt $ first_assum $ irule_at $ Pos last)
+  >~[‘exp_eq_in_ctxt c (Proj n i e) (Proj n i e')’] (* find_Proj *)
   >- (strip_tac
-      \\ fs [exp_eq_Prim_cong, demands_Proj])
-  >~[‘IsEq n i e ≈ IsEq n i e'’] (* find_IsEq *)
+      \\ fs [exp_eq_in_ctxt_Prim, demands_Proj])
+  >~[‘exp_eq_in_ctxt c (IsEq n i _ e) (IsEq n i _ e')’] (* find_IsEq *)
   >- (rw []
-      \\ fs [exp_eq_Prim_cong, demands_IsEq])
-  >~[‘Prim (AtomOp op) el1 ≈ Prim (AtomOp op) el2’]
+      \\ fs [exp_eq_in_ctxt_Prim, demands_IsEq])
+  >~[‘exp_eq_in_ctxt c (Prim (AtomOp op) el1) (Prim (AtomOp op) el2)’] (* find_Atom *)
   >- (rw []
-      >- (irule exp_eq_Prim_cong
+      >- (irule exp_eq_in_ctxt_Prim
           \\ fs [LIST_REL_EL_EQN]
           \\ rw []
           \\ rename1 ‘n < LENGTH _’
@@ -1096,84 +4250,218 @@ Proof
       \\ first_x_assum $ qspecl_then [‘n’] assume_tac
       \\ irule demands_AtomOp
       \\ gvs [EL_ZIP, EXISTS_MEM]
-      \\ pop_assum $ irule_at Any
-      \\ fs [MEM_EL]
       \\ first_x_assum $ irule_at Any
-      \\ fs [])
-  >>~[‘Prim ope el1 ≈ Prim ope el2’] (* find_Prim *)
+      \\ fs [EL_MEM])
+  >>~[‘exp_eq_in_ctxt c (Prim ope el1) (Prim ope el2)’] (* find_Prim *)
   >- (rw []
-      \\ irule exp_eq_Prim_cong
+      \\ irule exp_eq_in_ctxt_Prim
       \\ rw [LIST_REL_EL_EQN, EL_MAP]
       \\ rename1 ‘EL n _’
       \\ ‘n < LENGTH el1’ by fs []
       \\ first_x_assum drule
       \\ rw [])
   >- (rw [] (* find_Prim1 *)
-      >- (irule exp_eq_Prim_cong
-          \\ rw [LIST_REL_EL_EQN, EL_MAP]
+      >- (irule exp_eq_in_ctxt_Prim
+          \\ gvs [LIST_REL_EL_EQN, EL_MAP] \\ rw []
           \\ rename1 ‘EL n _’
           \\ ‘n < LENGTH el1’ by fs []
           \\ first_x_assum drule
-          \\ rw []
-          \\ fs [])
-      \\ rw []
+          \\ rw [])
       \\ last_x_assum dxrule
       \\ rw []
       \\ Cases_on ‘el1’
       \\ fs [demands_Prim])
-  >~[‘Prim ope el1 ≈ Fail’] (* find_Prim_Fail *)
+  >~[‘exp_eq_in_ctxt c (Prim ope el1) Fail’] (* find_Prim_Fail *)
   >- (rw []
-      \\ fs [not_well_written_is_fail])
-  >>~[‘Let v e e2 ≈ Let v e' e2'’] (* find_Let *)
-  >- (rw []
-      \\ fs [exp_eq_App_cong, exp_eq_Lam_cong]
-      \\ rename1 ‘_ demands d’
-      \\ PairCases_on ‘d’
-      \\ irule demands_Let2
-      \\ ‘d1 = v ∨ d1 ≠ v’ by fs []
-      \\ fs []
-      \\ last_x_assum irule
-      \\ first_x_assum $ irule_at Any)
-  >- (rw []
-      \\ fs [exp_eq_App_cong, exp_eq_Lam_cong]
-      \\ rename1 ‘_ demands d’
-      \\ PairCases_on ‘d’
-      \\ first_x_assum dxrule
-      \\ rw []
-      >- fs [demands_Let2]
-      \\ irule demands_Let1
-      \\ fs []
-      \\ first_x_assum drule
-      \\ rw []
-      \\ drule demands_empty_proj
+      \\ fs [exp_eq_IMP_exp_eq_in_ctxt, not_well_written_is_fail])
+  >>~[‘exp_eq_in_ctxt c (Let v e e2) (Let v e' e2')’] (* find_Let *)
+  >- (rw [exp_eq_in_ctxt_def]
+      \\ rename1 ‘find _ (Bind _ _ _) fdc2 _ _ _’
+      \\ ‘ (∀n l i c2.
+              (n,l) ∈ fdc2 ∧ i < LENGTH l ∧ EL i l ⇒
+              Var n fdemands (([],i),LENGTH l, concat_ctxt (Bind v e c) c2))’
+        by (rw [] \\ first_x_assum $ dxrule_then assume_tac
+            \\ gvs [fdemands_Bind, fdemands_def, concat_ctxt_def]
+            \\ irule fdemands_exp_eq \\ last_x_assum $ irule_at Any
+            \\ gvs [] \\ irule $ iffLR exp_eq_in_ctxt_sym
+            \\ irule exp_eq_concat_still_eq
+            \\ irule exp_eq_in_ctxt_trans >> last_x_assum $ irule_at Any
+            \\ irule exp_eq_IMP_exp_eq_in_ctxt
+            \\ gvs [GEN_ALL Let_Var])
+      \\ gvs []
+      >- (irule exp_eq_in_ctxt_trans \\ first_x_assum $ irule_at Any
+          \\ gvs [exp_eq_in_ctxt_App, exp_eq_in_ctxt_refl])
+      >~[‘Let _ _ _ demands (d, c)’]
+      >- (PairCases_on ‘d’
+          \\ irule demands_Let2
+          \\ ‘d1 = v ∨ d1 ≠ v’ by fs []
+          \\ gvs [])
+      >~[‘Let _ _ _ fdemands _’]
+      >- (irule fdemands_exp_eq \\ fs [concat_ctxt_def, fdemands_def]
+          \\ irule_at (Pos $ el 2) exp_eq_in_ctxt_App
+          \\ irule_at (Pos hd) exp_eq_in_ctxt_refl
+          \\ irule_at Any exp_eq_concat_still_eq
+          \\ last_x_assum $ irule_at $ Pos hd
+          \\ gvs [])
+      \\ first_x_assum $ drule_then assume_tac
+      \\ rename1 ‘_ demands_when_applied (d2, _, _)’ \\ PairCases_on ‘d2’
+      \\ gvs [demands_when_applied_def, eq_when_applied_def]
+      \\ irule eq_when_applied_trans_exp_eq \\ irule_at Any exp_eq_in_ctxt_App
+      \\ irule_at (Pos hd) exp_eq_in_ctxt_refl
+      \\ irule_at (Pos $ hd) $ iffLR exp_eq_in_ctxt_sym \\ first_assum $ irule_at $ Pos hd
+      \\ irule eq_when_applied_trans \\ pop_assum $ irule_at Any
+      \\ irule exp_eq_in_ctxt_IMP_eq_when_applied \\ irule exp_eq_in_ctxt_trans
+      \\ irule_at (Pos hd) exp_eq_IMP_exp_eq_in_ctxt \\ irule_at Any Let_Seq
+      \\ irule exp_eq_in_ctxt_Prim \\ fs []
+      \\ irule_at Any exp_eq_in_ctxt_App \\ fs [exp_eq_in_ctxt_refl]
+      \\ irule exp_eq_IMP_exp_eq_in_ctxt
+      \\ irule Let_not_in_freevars \\ fs [freevars_Projs]
+      \\ strip_tac \\ gvs [dest_fd_SND_def])
+  >- (rw [exp_eq_in_ctxt_def]
+      \\ rename1 ‘find _ (Bind _ _ _) fdc2 _ _ _’
+      \\ ‘ (∀n l i c2.
+                        (n,l) ∈ fdc2 ∧ i < LENGTH l ∧ EL i l ⇒
+                        Var n fdemands (([],i),LENGTH l, concat_ctxt (Bind v e c) c2))’
+        by (rw [] \\ first_x_assum $ dxrule_then assume_tac
+            \\ gvs [fdemands_Bind, fdemands_def, concat_ctxt_def]
+            \\ irule fdemands_exp_eq
+            \\ irule_at Any exp_eq_concat_still_eq \\ last_x_assum $ irule_at Any
+            \\ gvs [] \\ irule $ iffLR exp_eq_in_ctxt_sym
+            \\ irule exp_eq_in_ctxt_trans >> last_x_assum $ irule_at Any
+            \\ irule exp_eq_IMP_exp_eq_in_ctxt
+            \\ gvs [GEN_ALL Let_Var])
+      \\ gvs []
+      >- (irule exp_eq_in_ctxt_trans
+          \\ first_x_assum $ irule_at Any
+          \\ fs [exp_eq_in_ctxt_App, exp_eq_in_ctxt_refl])
+      >~[‘Let _ _ _ fdemands _’]
+      >- (irule fdemands_exp_eq \\ fs [fdemands_def, concat_ctxt_def]
+          \\ irule_at Any exp_eq_concat_still_eq
+          \\ irule_at (Pos hd) exp_eq_in_ctxt_App
+          \\ irule_at (Pos hd) exp_eq_in_ctxt_refl
+          \\ last_x_assum $ irule_at $ Pos hd
+          \\ gvs [])
+      >~[‘Let _ _ _ demands (d, c)’]
+      >- (rename1 ‘_ demands (d, c)’ \\ PairCases_on ‘d’
+          \\ first_x_assum $ dxrule_then assume_tac
+          \\ fs [demands_Let2]
+          \\ irule demands_Let1
+          \\ first_x_assum $ drule_then assume_tac
+          \\ dxrule_then assume_tac demands_empty_Projs \\ fs [])
+      \\ first_x_assum $ drule_then assume_tac
+      \\ rename1 ‘_ demands_when_applied (d2, _, _)’ \\ PairCases_on ‘d2’
+      \\ gvs [demands_when_applied_def, eq_when_applied_def]
+      \\ irule eq_when_applied_trans_exp_eq \\ irule_at Any exp_eq_in_ctxt_App
+      \\ irule_at (Pos $ el 2) $ iffLR exp_eq_in_ctxt_sym
+      \\ first_assum $ irule_at Any \\ irule_at Any exp_eq_in_ctxt_refl
+      \\ irule eq_when_applied_trans \\ pop_assum $ irule_at Any
+      \\ irule exp_eq_in_ctxt_IMP_eq_when_applied \\ irule exp_eq_in_ctxt_trans
+      \\ irule_at (Pos hd) exp_eq_IMP_exp_eq_in_ctxt \\ irule_at Any Let_Seq
+      \\ irule exp_eq_in_ctxt_Prim \\ fs []
+      \\ irule_at Any exp_eq_in_ctxt_App \\ fs [exp_eq_in_ctxt_refl]
+      \\ irule exp_eq_IMP_exp_eq_in_ctxt \\ irule Let_not_in_freevars
+      \\ fs [freevars_Projs]
+      \\ strip_tac \\ gvs [dest_fd_SND_def])
+  >~[‘SOME (T::argD, ds3)’]
+  >- (rw [] \\ gvs [exp_eq_in_ctxt_App, demands_App, fdemands_App, demands_when_applied_App]
+      >- (rw [Once $ GSYM concat_Nil]
+          \\ irule fdemands_0_App_demands
+          \\ last_assum $ irule_at Any \\ gvs [concat_Nil]
+          \\ irule_at Any demands_exp_eq
+          \\ first_x_assum $ dxrule_then assume_tac
+          \\ pop_assum $ irule_at Any \\ gvs []))
+  >~[‘SOME (b::argD, ds3)’]
+  >- (rw [] \\ gvs [exp_eq_in_ctxt_App, demands_App, fdemands_App, demands_when_applied_App])
+  >~[‘SOME (bL, fd)’]
+  >- (rw [] \\ gvs [SUBSET_DEF])
+  >~ [‘exp_eq_in_ctxt c e1 e2 ∧ find _ _ _ _ _ _ ∧ _’] (* find_Eq *)
+  >- (rw [] >> gvs []
+      >- (irule exp_eq_in_ctxt_trans >> rpt $ first_x_assum $ irule_at Any) >>
+      irule demands_exp_eq >>
+      last_x_assum $ dxrule_then $ irule_at Any >>
+      gvs [exp_eq_in_ctxt_sym])
+  >- (rw [] \\ dxrule_then (dxrule_then assume_tac) fdemands_subset (* find_Subset *)
+      \\ gvs []
+      \\ rename1 ‘e demands (d, c)’ \\ PairCases_on ‘d’
+      \\ gvs []
+      \\ first_x_assum $ drule_then assume_tac \\ fs []
+      \\ first_x_assum $ drule_then assume_tac
+      \\ drule demands_Projs_reduce
       \\ fs [])
-  >- (rw [] (* find_Subset *)
-      \\ rename1 ‘e demands d’ \\ PairCases_on ‘d’
-      \\ first_x_assum drule
-      \\ rw []
-      \\ first_x_assum drule
-      \\ rw []
-      \\ drule demands_projs_reduce
-      \\ fs [])
-  >- (rw [] (* find_Lam *)
-      \\ fs [exp_eq_Lam_cong])
-  >- (rw []
-      \\ fs [exp_eq_Lams_cong])
-  >- (rw []
-      \\ fs [])
-  >- (rw []
-      \\ fs [exp_eq_Letrec_cong, exp_eq_l_refl])
+  >- (rw [] \\ dxrule_then assume_tac fdemands_set_IsFree  (* find_Lam *)
+      \\ pop_assum $ dxrule_then assume_tac
+      \\ last_x_assum $ dxrule_then assume_tac
+      \\ gvs [exp_eq_in_ctxt_Lam])
+  >- (rw [] \\ dxrule_then (dxrule_then assume_tac) fdemands_set_FOLDL_IsFree
+      \\ gvs [exp_eq_in_ctxt_Lams])
+  >- (rw [] \\ dxrule_then (dxrule_then assume_tac) fdemands_set_FOLDL_IsFree
+      \\ gvs [exp_eq_in_ctxt_Lams]
+      \\ rename1 ‘demands_boolList ds vL’
+      \\ qabbrev_tac ‘p = demands_boolList ds vL’ \\ PairCases_on ‘p’ \\ gvs []
+      \\ dxrule_then assume_tac demands_boolList_soundness
+      \\ gvs [] \\ first_x_assum $ drule_then $ dxrule_then assume_tac \\ gvs []
+      \\ first_x_assum irule \\ irule demands_empty_Projs
+      \\ gvs [concat_FOLDL_IsFree]
+      \\ irule_at Any demands_concat
+      \\ irule_at Any demands_exp_eq
+      \\ last_x_assum $ irule_at Any
+      \\ last_x_assum $ dxrule_then $ irule_at Any)
+  >- (rename1 ‘exp_eq_in_ctxt c (Letrec b1 e1) (Letrec b2 e2)’
+      \\ strip_tac \\ strip_tac \\ gvs [EVERY_CONJ]
+      \\ dxrule_then (dxrule_then assume_tac) fdemands_set_RecBind
+      \\ gvs [exp_eq_in_ctxt_def, fdemands_def]
+      \\ ‘∀n l i c2. (n, l) ∈ fdc' ∧ i < LENGTH l ∧ EL i l
+                            ⇒ Letrec b1 (Var n) fdemands (([], i), LENGTH l, concat_ctxt c c2)’
+        by (rw [] \\ first_x_assum $ dxrule_then assume_tac
+            \\ gvs [concat_ctxt_def, fdemands_def]
+            \\ irule fdemands_exp_eq
+            \\ irule_at Any exp_eq_IMP_exp_eq_in_ctxt
+            \\ irule_at Any $ iffLR exp_eq_sym \\ irule_at Any Letrec_unfold
+            \\ last_x_assum $ drule_then assume_tac
+            \\ gvs [GSYM fdemands_def] \\ irule fdemands_exp_eq
+            \\ first_x_assum $ irule_at Any
+            \\ gvs [exp_eq_IMP_exp_eq_in_ctxt, exp_eq_sym])
+      \\ rw [] \\ gvs [fdemands_def, concat_ctxt_def]
+      >~[‘Letrec _ _ demands (d, _)’]
+      >- (PairCases_on ‘d’
+          \\ first_x_assum $ dxrule_then assume_tac
+          \\ gvs [demands_Letrec]
+          \\ irule demands_Letrec2 \\ gvs []
+          \\ first_assum $ irule_at Any
+          \\ last_x_assum $ drule_then assume_tac \\ gvs []
+          \\ last_x_assum $ drule_then assume_tac
+          \\ drule_then irule demands_empty_Projs)
+      >- (irule exp_eq_in_ctxt_trans \\ first_x_assum $ irule_at Any
+          \\ irule exp_eq_IMP_exp_eq_in_ctxt \\ irule exp_eq_Letrec_cong
+          \\ gvs [exp_eq_refl, LIST_REL_EL_EQN] \\ irule_at Any LIST_EQ \\ fs []
+          \\ rw [] \\ last_x_assum $ drule_then assume_tac \\ gvs [EL_MAP])
+      >- (irule fdemands_exp_eq
+          \\ first_x_assum $ irule_at Any \\ gvs []
+          \\ irule exp_eq_concat_still_eq
+          \\ irule exp_eq_IMP_exp_eq_in_ctxt \\ irule exp_eq_Letrec_cong
+          \\ gvs [exp_eq_refl, LIST_REL_EL_EQN] \\ irule_at Any LIST_EQ \\ fs []
+          \\ rw [] \\ last_x_assum $ drule_then assume_tac \\ gvs [EL_MAP])
+      >- (irule demands_when_applied_exp_eq \\ gvs [demands_when_applied_Letrec]
+          \\ first_x_assum $ drule_then assume_tac \\ dxrule_then assume_tac demands_when_applied_Letrec
+          \\ gvs [EVERY_MEM, dest_fd_SND_def]
+          \\ first_x_assum $ irule_at Any \\ gvs []
+          \\ conj_tac
+          >- (strip_tac \\ last_x_assum $ dxrule_then assume_tac
+              \\ rename1 ‘SND d2’ \\ PairCases_on ‘d2’ \\ gvs [])
+          \\ irule exp_eq_IMP_exp_eq_in_ctxt \\ irule exp_eq_Letrec_cong
+          \\ gvs [exp_eq_refl, LIST_REL_EL_EQN] \\ irule_at Any LIST_EQ \\ fs []
+          \\ rw [] \\ last_x_assum $ drule_then assume_tac \\ gvs [EL_MAP]))
 QED
 
 Theorem find_soundness:
-  find e Nil ds e' ⇒ e ≈ e'
+  find e Nil {} ds e' fd ⇒ e ≈ e'
 Proof
   rw []
   \\ dxrule find_soundness_lemma
-  \\ fs []
+  \\ fs [exp_eq_in_ctxt_def]
 QED
 
-Datatype:
+(*Datatype:
   demands_tree = DemandNode bool (((string # num) # demands_tree) list)
 End
 
@@ -1225,7 +4513,7 @@ Definition find_function_def:
   (find_function (Prim op l) c =
   (FEMPTY, Prim op (MAP (λe. SND (find_function e c)) l))) ∧
   (find_function (App (Lam v e2) e) c = let (d, e') = find_function e c in
-                                          let (d2, e2') = find_function e2 (Bind v e c c) in
+                                          let (d2, e2') = find_function e2 (Bind v e c) in
                                            case FLOOKUP d2 v of
                                              | NONE => (d2, App (Lam v e2') e')
                                              | SOME s => (FMERGE merge_dt d (d2 \\ v), Let v e' (Seq (Var v) e2'))) ∧
@@ -1515,7 +4803,7 @@ Proof
        \\ fs [exp_size_def, find_function_def]
        \\ qabbrev_tac ‘ep = find_function e c’
        \\ PairCases_on ‘ep’
-       \\ qabbrev_tac ‘e2p = find_function e2 (Bind s e c c)’
+       \\ qabbrev_tac ‘e2p = find_function e2 (Bind s e c)’
        \\ PairCases_on ‘e2p’
        \\ last_x_assum $ qspecl_then [‘e’] assume_tac
        \\ last_x_assum $ qspecl_then [‘e2’] assume_tac
@@ -1625,7 +4913,7 @@ Proof
   \\ drule find_function_soundness_lemma
   \\ rw []
   \\ first_assum $ irule_at Any
-QED
+QED*)
 
 (*
   let foo = lam (a + 2) in
